@prefix IAO: <http://purl.obolibrary.org/obo/IAO_> .
@prefix linkml: <https://w3id.org/linkml/> .
@prefix odm: <http://www.cdisc.org/ns/odm/v2.0/> .
@prefix owl: <http://www.w3.org/2002/07/owl#> .
@prefix rdf: <http://www.w3.org/1999/02/22-rdf-syntax-ns#> .
@prefix rdfs: <http://www.w3.org/2000/01/rdf-schema#> .
@prefix shex: <http://www.w3.org/ns/shex#> .
@prefix skos: <http://www.w3.org/2004/02/skos/core#> .
@prefix xhtml: <http://www.w3.org/1999/xhtml> .
@prefix xml1: <http://ncicb.nci.nih.gov/xml/odm/EVS/CDISC> .
@prefix xsd: <http://www.w3.org/2001/XMLSchema#> .

<http://www.cdisc.org/ns/odm/v2.0> a owl:Ontology ;
    rdfs:label "odm" ;
    IAO:0000700 odm:AbsoluteTimingConstraint,
        odm:Address,
        odm:AdminData,
        odm:Alias,
        odm:AnnotatedCRF,
        odm:Annotation,
        odm:Arm,
        odm:Association,
        odm:AuditRecord,
        odm:Branching,
        odm:CDISCNotes,
        odm:CRFCompletionInstructions,
        odm:CheckValue,
        odm:City,
        odm:Class,
        odm:ClinicalData,
        odm:Code,
        odm:CodeList,
        odm:CodeListItem,
        odm:CodeListRef,
        odm:Coding,
        odm:Comment,
        odm:CommentDef,
        odm:ConditionDef,
        odm:Country,
        odm:Criterion,
        odm:DateTimeStamp,
        odm:Decode,
        odm:DefaultTransition,
        odm:Definition,
        odm:Description,
        odm:DocumentRef,
        odm:DurationTimingConstraint,
        odm:EntryCriteria,
        odm:Epoch,
        odm:ErrorMessage,
        odm:ExceptionEvent,
        odm:ExclusionCriteria,
        odm:ExitCriteria,
        odm:ExternalCodeLib,
        odm:FamilyName,
        odm:Flag,
        odm:FlagType,
        odm:FlagValue,
        odm:FormalExpression,
        odm:FullName,
        odm:GeoPosition,
        odm:GivenName,
        odm:HouseNumber,
        odm:Image,
        odm:ImplementationNotes,
        odm:Include,
        odm:InclusionCriteria,
        odm:InclusionExclusionCriteria,
        odm:IntercurrentEvent,
        odm:InvestigatorRef,
        odm:ItemData,
        odm:ItemDef,
        odm:ItemGroupData,
        odm:ItemGroupDef,
        odm:ItemGroupRef,
        odm:ItemRef,
        odm:KeySet,
        odm:Leaf,
        odm:LegalReason,
        odm:Location,
        odm:LocationRef,
        odm:Meaning,
        odm:MetaDataVersion,
        odm:MetaDataVersionRef,
        odm:MethodDef,
        odm:MethodSignature,
        odm:ODMFileMetadata,
        odm:Organization,
        odm:Origin,
        odm:OtherText,
        odm:PDFPageRef,
        odm:Parameter,
        odm:ParameterValue,
        odm:PostalCode,
        odm:Prefix,
        odm:Prompt,
        odm:Protocol,
        odm:Query,
        odm:Question,
        odm:RangeCheck,
        odm:ReasonForChange,
        odm:ReferenceData,
        odm:RelativeTimingConstraint,
        odm:Resource,
        odm:ReturnValue,
        odm:Selection,
        odm:Signature,
        odm:SignatureDef,
        odm:SignatureRef,
        odm:SiteRef,
        odm:SourceID,
        odm:SourceItem,
        odm:SourceItems,
        odm:Standard,
        odm:Standards,
        odm:StateProv,
        odm:StreetName,
        odm:Study,
        odm:StudyEndPoint,
        odm:StudyEndPointRef,
        odm:StudyEndPoints,
        odm:StudyEstimand,
        odm:StudyEstimands,
        odm:StudyEventData,
        odm:StudyEventDef,
        odm:StudyEventGroupDef,
        odm:StudyEventGroupRef,
        odm:StudyEventRef,
        odm:StudyIndication,
        odm:StudyIndications,
        odm:StudyIntervention,
        odm:StudyInterventionRef,
        odm:StudyInterventions,
        odm:StudyObjective,
        odm:StudyObjectives,
        odm:StudyParameter,
        odm:StudyStructure,
        odm:StudySummary,
        odm:StudyTargetPopulation,
        odm:StudyTargetPopulationRef,
        odm:StudyTiming,
        odm:StudyTimings,
        odm:SubClass,
        odm:SubjectData,
        odm:Suffix,
        odm:SummaryMeasure,
        odm:SupplementalDoc,
        odm:TargetTransition,
        odm:Telecom,
        odm:Transition,
        odm:TransitionTimingConstraint,
        odm:TranslatedText,
        odm:TrialPhase,
        odm:User,
        odm:UserName,
        odm:UserRef,
        odm:Value,
        odm:ValueListDef,
        odm:ValueListRef,
        odm:WhereClauseDef,
        odm:WhereClauseRef,
        odm:WorkflowDef,
        odm:WorkflowEnd,
        odm:WorkflowRef,
        odm:WorkflowStart ;
    linkml:id "http://www.cdisc.org/ns/odm/v2.0" .

odm:Base64Binary a owl:Class,
        linkml:TypeDefinition ;
    rdfs:label "base64Binary" ;
    rdfs:subClassOf [ a owl:Restriction ;
            owl:onDataRange odm:base64Binary ;
            owl:onProperty linkml:topValue ;
            owl:qualifiedCardinality 1 ] .

odm:Base64Float a owl:Class,
        linkml:TypeDefinition ;
    rdfs:label "base64Float" ;
    rdfs:subClassOf [ a owl:Restriction ;
            owl:onDataRange odm:base64Float ;
            owl:onProperty linkml:topValue ;
            owl:qualifiedCardinality 1 ] .

odm:Boolean a owl:Class,
        linkml:TypeDefinition ;
    rdfs:label "boolean" ;
    rdfs:subClassOf [ a owl:Restriction ;
            owl:onDataRange xsd:boolean ;
            owl:onProperty linkml:topValue ;
            owl:qualifiedCardinality 1 ] .

odm:Curie a owl:Class,
        linkml:TypeDefinition ;
    rdfs:label "curie" ;
    rdfs:subClassOf [ a owl:Restriction ;
            owl:onDataRange xsd:string ;
            owl:onProperty linkml:topValue ;
            owl:qualifiedCardinality 1 ] .

odm:DateOrDatetime a owl:Class,
        linkml:TypeDefinition ;
    rdfs:label "date_or_datetime" ;
    rdfs:subClassOf [ a owl:Restriction ;
            owl:onDataRange linkml:DateOrDatetime ;
            owl:onProperty linkml:topValue ;
            owl:qualifiedCardinality 1 ] .

odm:Dictionary a owl:ObjectProperty,
        linkml:SlotDefinition ;
    rdfs:label "Dictionary" ;
    rdfs:range odm:DictionaryNameType .

odm:Double a owl:Class,
        linkml:TypeDefinition ;
    rdfs:label "double" ;
    rdfs:subClassOf [ a owl:Restriction ;
            owl:onDataRange xsd:double ;
            owl:onProperty linkml:topValue ;
            owl:qualifiedCardinality 1 ] .

odm:EmptyTag a owl:Class,
        linkml:TypeDefinition ;
    rdfs:label "emptyTag" ;
    rdfs:subClassOf [ a owl:Restriction ;
            owl:onDataRange odm:emptyTag ;
            owl:onProperty linkml:topValue ;
            owl:qualifiedCardinality 1 ] .

odm:Float a owl:Class,
        linkml:TypeDefinition ;
    rdfs:label "float" ;
    rdfs:subClassOf [ a owl:Restriction ;
            owl:onDataRange xsd:float ;
            owl:onProperty linkml:topValue ;
            owl:qualifiedCardinality 1 ] .

odm:HexBinary a owl:Class,
        linkml:TypeDefinition ;
    rdfs:label "hexBinary" ;
    rdfs:subClassOf [ a owl:Restriction ;
            owl:onDataRange odm:hexBinary ;
            owl:onProperty linkml:topValue ;
            owl:qualifiedCardinality 1 ] .

odm:HexFloat a owl:Class,
        linkml:TypeDefinition ;
    rdfs:label "hexFloat" ;
    rdfs:subClassOf [ a owl:Restriction ;
            owl:onDataRange odm:hexFloat ;
            owl:onProperty linkml:topValue ;
            owl:qualifiedCardinality 1 ] .

odm:IncompleteDate a owl:Class,
        linkml:TypeDefinition ;
    rdfs:label "incompleteDate" ;
    rdfs:subClassOf [ a owl:Restriction ;
            owl:onDataRange odm:incompleteDate ;
            owl:onProperty linkml:topValue ;
            owl:qualifiedCardinality 1 ] .

odm:IncompleteDatetime a owl:Class,
        linkml:TypeDefinition ;
    rdfs:label "incompleteDatetime" ;
    rdfs:subClassOf [ a owl:Restriction ;
            owl:onDataRange odm:incompleteDatetime ;
            owl:onProperty linkml:topValue ;
            owl:qualifiedCardinality 1 ] .

odm:IncompleteTime a owl:Class,
        linkml:TypeDefinition ;
    rdfs:label "incompleteTime" ;
    rdfs:subClassOf [ a owl:Restriction ;
            owl:onDataRange odm:incompleteTime ;
            owl:onProperty linkml:topValue ;
            owl:qualifiedCardinality 1 ] .

odm:Integer a owl:Class,
        linkml:TypeDefinition ;
    rdfs:label "integer" ;
    rdfs:subClassOf [ a owl:Restriction ;
            owl:onDataRange xsd:integer ;
            owl:onProperty linkml:topValue ;
            owl:qualifiedCardinality 1 ] .

odm:IntervalDatetime a owl:Class,
        linkml:TypeDefinition ;
    rdfs:label "intervalDatetime" ;
    rdfs:subClassOf [ a owl:Restriction ;
            owl:onDataRange odm:intervalDatetime ;
            owl:onProperty linkml:topValue ;
            owl:qualifiedCardinality 1 ] .

odm:ItemGroupTypeTypeEnum a owl:Class,
        linkml:EnumDefinition ;
    rdfs:label "ItemGroupTypeTypeEnum" ;
    owl:unionOf [ rdf:rest () ] .

odm:Ncname a owl:Class,
        linkml:TypeDefinition ;
    rdfs:label "ncname" ;
    rdfs:subClassOf [ a owl:Restriction ;
            owl:onDataRange xsd:string ;
            owl:onProperty linkml:topValue ;
            owl:qualifiedCardinality 1 ] .

odm:Nodeidentifier a owl:Class,
        linkml:TypeDefinition ;
    rdfs:label "nodeidentifier" ;
    rdfs:subClassOf [ a owl:Restriction ;
            owl:onDataRange shex:nonLiteral ;
            owl:onProperty linkml:topValue ;
            owl:qualifiedCardinality 1 ] .

odm:Objectidentifier a owl:Class,
        linkml:TypeDefinition ;
    rdfs:label "objectidentifier" ;
    rdfs:subClassOf [ a owl:Restriction ;
            owl:onDataRange shex:iri ;
            owl:onProperty linkml:topValue ;
            owl:qualifiedCardinality 1 ] .

odm:PartialDate a owl:Class,
        linkml:TypeDefinition ;
    rdfs:label "partialDate" ;
    rdfs:subClassOf [ a owl:Restriction ;
            owl:onDataRange odm:partialDate ;
            owl:onProperty linkml:topValue ;
            owl:qualifiedCardinality 1 ] .

odm:PartialDatetime a owl:Class,
        linkml:TypeDefinition ;
    rdfs:label "partialDatetime" ;
    rdfs:subClassOf [ a owl:Restriction ;
            owl:onDataRange odm:partialDatetime ;
            owl:onProperty linkml:topValue ;
            owl:qualifiedCardinality 1 ] .

odm:PartialTime a owl:Class,
        linkml:TypeDefinition ;
    rdfs:label "partialTime" ;
    rdfs:subClassOf [ a owl:Restriction ;
            owl:onDataRange odm:partialTime ;
            owl:onProperty linkml:topValue ;
            owl:qualifiedCardinality 1 ] .

odm:TDatetime a owl:Class,
        linkml:TypeDefinition ;
    rdfs:label "tDatetime" ;
    rdfs:subClassOf [ a owl:Restriction ;
            owl:onDataRange odm:tDatetime ;
            owl:onProperty linkml:topValue ;
            owl:qualifiedCardinality 1 ] .

odm:TDuration a owl:Class,
        linkml:TypeDefinition ;
    rdfs:label "tDuration" ;
    rdfs:subClassOf [ a owl:Restriction ;
            owl:onDataRange odm:tDuration ;
            owl:onProperty linkml:topValue ;
            owl:qualifiedCardinality 1 ] .

odm:THour a owl:Class,
        linkml:TypeDefinition ;
    rdfs:label "tHour" ;
    rdfs:subClassOf [ a owl:Restriction ;
            owl:onDataRange odm:tHour ;
            owl:onProperty linkml:topValue ;
            owl:qualifiedCardinality 1 ] .

odm:TIncomplete a owl:Class,
        linkml:TypeDefinition ;
    rdfs:label "tIncomplete" ;
    rdfs:subClassOf [ a owl:Restriction ;
            owl:onDataRange odm:tIncomplete ;
            owl:onProperty linkml:topValue ;
            owl:qualifiedCardinality 1 ] .

odm:TIncompleteDate a owl:Class,
        linkml:TypeDefinition ;
    rdfs:label "tIncompleteDate" ;
    rdfs:subClassOf [ a owl:Restriction ;
            owl:onDataRange odm:tIncompleteDate ;
            owl:onProperty linkml:topValue ;
            owl:qualifiedCardinality 1 ] .

odm:TIncompleteTime a owl:Class,
        linkml:TypeDefinition ;
    rdfs:label "tIncompleteTime" ;
    rdfs:subClassOf [ a owl:Restriction ;
            owl:onDataRange odm:tIncompleteTime ;
            owl:onProperty linkml:topValue ;
            owl:qualifiedCardinality 1 ] .

odm:TInterval a owl:Class,
        linkml:TypeDefinition ;
    rdfs:label "tInterval" ;
    rdfs:subClassOf [ a owl:Restriction ;
            owl:onDataRange odm:tInterval ;
            owl:onProperty linkml:topValue ;
            owl:qualifiedCardinality 1 ] .

odm:Time a owl:Class,
        linkml:TypeDefinition ;
    rdfs:label "time" ;
    rdfs:subClassOf [ a owl:Restriction ;
            owl:onDataRange xsd:dateTime ;
            owl:onProperty linkml:topValue ;
            owl:qualifiedCardinality 1 ] .

odm:Uri a owl:Class,
        linkml:TypeDefinition ;
    rdfs:label "uri" ;
    rdfs:subClassOf [ a owl:Restriction ;
            owl:onDataRange xsd:anyURI ;
            owl:onProperty linkml:topValue ;
            owl:qualifiedCardinality 1 ] .

linkml:SubsetDefinition a owl:Class .

odm:AbsoluteTimingConstraintRef a owl:ObjectProperty,
        linkml:SlotDefinition ;
    rdfs:label "AbsoluteTimingConstraintRef" ;
    rdfs:range odm:AbsoluteTimingConstraint ;
    skos:definition "AbsoluteTimingConstraint reference: The element AbsoluteTimingConstraint is used to specify when an activity, represented by either a StudyEventGroup or StudyEvent, can take place." .

odm:AdminDataRef a owl:ObjectProperty,
        linkml:SlotDefinition ;
    rdfs:label "AdminDataRef" ;
    rdfs:range odm:AdminData ;
    skos:definition "AdminData reference: Administrative information about users, locations, organizations, and electronic signatures." .

odm:Altitude a owl:ObjectProperty,
        linkml:SlotDefinition ;
    rdfs:label "Altitude" ;
    rdfs:range odm:Decimal ;
    skos:definition "Height above sea level in meters." .

odm:AnnotatedCRFRef a owl:ObjectProperty,
        linkml:SlotDefinition ;
    rdfs:label "AnnotatedCRFRef" ;
    rdfs:range odm:AnnotatedCRF ;
    skos:definition "AnnotatedCRF reference: An Annotated Case Report Form (CRF) is a Portable File Format (PDF) document that provides the mapping of data collection fields to the variables or discrete variable values contained within the datasets." .

odm:ArchiveLocationID a owl:ObjectProperty,
        linkml:SlotDefinition ;
    rdfs:label "ArchiveLocationID" ;
    rdfs:range odm:Oidref ;
    skos:definition "Reference to the unique ID of a leaf element that provides the actual location and file name of the data file." .

odm:ArmOID a owl:ObjectProperty,
        linkml:SlotDefinition ;
    rdfs:label "ArmOID" ;
    rdfs:range odm:Oidref ;
    skos:definition "Reference to an Arm element defined in the study." .

odm:ArmRef a owl:ObjectProperty,
        linkml:SlotDefinition ;
    rdfs:label "ArmRef" ;
    rdfs:range odm:Arm ;
    skos:definition "Arm reference: An Arm element provides the declaration of a study arm. Arms do not have any ordering relative to one another." .

odm:AsOfDateTime a owl:ObjectProperty,
        linkml:SlotDefinition ;
    rdfs:label "AsOfDateTime" ;
    rdfs:range odm:Datetime ;
    skos:definition "The date/time at which the source database was queried in order to create this document." .

odm:AssociationRef a owl:ObjectProperty,
        linkml:SlotDefinition ;
    rdfs:label "AssociationRef" ;
    rdfs:range odm:Association ;
    skos:definition "Association reference: An association permits an annotation to be placed on an ordered pair of entities rather than on just one. The first and second KeySets identify the start and end of the annotated \"link." .

odm:Attribute a owl:ObjectProperty,
        linkml:SlotDefinition ;
    rdfs:label "Attribute" ;
    rdfs:range odm:Text ;
    skos:definition "Field provided by the Name attribute where the data or information can be obtained. Examples are \"valueQuantity.value\" or \"valueQuantity.unit\" for the case of an HL7-FHIR \"Observation\", \"Repeating\" for the case of an ODM ItemGroupDef element, \"unit\" for the case of an HL7-CDA doseQuantity, \"Code\" or \"Name\" for the case of field 5 (which is composite) of an HL7-v2 OBX message. The Name and Attribute attributes are meant to provide traceability documentation." .

odm:BranchingRef a owl:ObjectProperty,
        linkml:SlotDefinition ;
    rdfs:label "BranchingRef" ;
    rdfs:range odm:Branching ;
    skos:definition "Branching reference: This element describes the branching in a workflow from a source (start) structural element to 2 or more target structural elements, over a Transition element." .

odm:CDISCNotesRef a owl:ObjectProperty,
        linkml:SlotDefinition ;
    rdfs:label "CDISCNotesRef" ;
    rdfs:range odm:CDISCNotes ;
    skos:definition "CDISCNotes reference: Explanatory text for the variable." .

odm:CRFCompletionInstructionsRef a owl:ObjectProperty,
        linkml:SlotDefinition ;
    rdfs:label "CRFCompletionInstructionsRef" ;
    rdfs:range odm:CRFCompletionInstructions ;
    skos:definition "CRFCompletionInstructions reference: Instructions for the clinical site on how to enter collected information on the CRF." .

odm:Category a owl:ObjectProperty,
        linkml:SlotDefinition ;
    rdfs:label "Category" ;
    rdfs:range odm:Text ;
    skos:definition "The Category attribute is typically used to indicate the study phase appropriate to this type of study event. Examples might include screening, pretreatment, treatment, and follow-up." .

odm:CheckValueRef a owl:ObjectProperty,
        linkml:SlotDefinition ;
    rdfs:label "CheckValueRef" ;
    rdfs:range odm:CheckValue ;
    skos:definition "CheckValue reference: A comparison value used in a range check." .

odm:CityRef a owl:ObjectProperty,
        linkml:SlotDefinition ;
    rdfs:label "CityRef" ;
    rdfs:range odm:City ;
    skos:definition "City reference: The city name part of a user's postal address." .

odm:ClassRef a owl:ObjectProperty,
        linkml:SlotDefinition ;
    rdfs:label "ClassRef" ;
    rdfs:range odm:Class ;
    skos:definition "Class reference: None" .

odm:ClinicalDataRef a owl:ObjectProperty,
        linkml:SlotDefinition ;
    rdfs:label "ClinicalDataRef" ;
    rdfs:range odm:ClinicalData ;
    skos:definition "ClinicalData reference: Clinical data for 1 or more subjects." .

odm:CodeListItemRef a owl:ObjectProperty,
        linkml:SlotDefinition ;
    rdfs:label "CodeListItemRef" ;
    rdfs:range odm:CodeListItem ;
    skos:definition "CodeListItem reference: Defines an individual member value of a codelist. It may include a display value in the child Decode element" .

odm:CodedValue a owl:ObjectProperty,
        linkml:SlotDefinition ;
    rdfs:label "CodedValue" ;
    rdfs:range odm:Value ;
    skos:definition "Value of the codelist item (as it would occur in clinical data)." .

odm:CommentDefRef a owl:ObjectProperty,
        linkml:SlotDefinition ;
    rdfs:label "CommentDefRef" ;
    rdfs:range odm:CommentDef ;
    skos:definition "CommentDef reference: The Comment element allows referencing short comments self-contained in the XML document or long comments normally included in external documents. For comments included in external documents, the reference could include specific pages of a document where the comments are included." .

odm:CommentRef a owl:ObjectProperty,
        linkml:SlotDefinition ;
    rdfs:label "CommentRef" ;
    rdfs:range odm:Comment ;
    skos:definition "Comment reference: A free-text (uninterpreted) comment about clinical data. The comment may have come from the sponsor or the clinical site." .

odm:ComparatorRef a owl:ObjectProperty,
        linkml:SlotDefinition ;
    rdfs:label "ComparatorRef" ;
    rdfs:range odm:Comparator ;
    skos:definition "Comparison operator used to compare the item and value(s)." .

odm:ConditionDefRef a owl:ObjectProperty,
        linkml:SlotDefinition ;
    rdfs:label "ConditionDefRef" ;
    rdfs:range odm:ConditionDef ;
    skos:definition "ConditionDef reference: A ConditionDef defines a boolean condition." .

odm:Core a owl:ObjectProperty,
        linkml:SlotDefinition ;
    rdfs:label "Core" ;
    rdfs:range odm:CoreType ;
    skos:definition "CDASH, ADaM, SDTM, and SEND Core designations." .

odm:CountryRef a owl:ObjectProperty,
        linkml:SlotDefinition ;
    rdfs:label "CountryRef" ;
    rdfs:range odm:Country ;
    skos:definition "Country reference: The country name part of a user's postal address. For CDISC SDTM or trial registry applications, this must be represented by an ISO 3166 3-letter or US-GENC country code (e.g., FRA for France, JPN for Japan)." .

odm:CreationDateTime a owl:ObjectProperty,
        linkml:SlotDefinition ;
    rdfs:label "CreationDateTime" ;
    rdfs:range odm:Datetime ;
    skos:definition "Time of creation of the file containing the document." .

odm:DatasetName a owl:ObjectProperty,
        linkml:SlotDefinition ;
    rdfs:label "DatasetName" ;
    rdfs:range odm:Name ;
    skos:definition "Name of a file containing the ItemGroupData for this ItemGroupDef. The name applies to the object itself rather then providing a mapping to a different object." .

odm:DecodeRef a owl:ObjectProperty,
        linkml:SlotDefinition ;
    rdfs:label "DecodeRef" ;
    rdfs:range odm:Decode ;
    skos:definition "Decode reference: The displayed value relating to the CodeListItem/@CodedValue. This is often a label corresponding to a short name or alpha-numeric code. The actual Decode text is provided in a TranslatedText element so that it can be provided in different languages on a case report form or tabular data summary." .

odm:DefaultTransitionRef a owl:ObjectProperty,
        linkml:SlotDefinition ;
    rdfs:label "DefaultTransitionRef" ;
    rdfs:range odm:DefaultTransition ;
    skos:definition "DefaultTransition reference: None" .

odm:DisplayFormat a owl:ObjectProperty,
        linkml:SlotDefinition ;
    rdfs:label "DisplayFormat" ;
    rdfs:range odm:Text ;
    skos:definition "Display format supports data visualization of numeric float and date values." .

odm:Domain a owl:ObjectProperty,
        linkml:SlotDefinition ;
    rdfs:label "Domain" ;
    rdfs:range odm:Text ;
    skos:definition "Identifies the scope or CDISC SDTMIG/SENDIG Domain of the ItemGroup data. The domain applies to the object itself rather then providing a mapping to a different object." .

odm:DurationPostWindow a owl:ObjectProperty,
        linkml:SlotDefinition ;
    rdfs:label "DurationPostWindow" ;
    rdfs:range odm:DurationDatetime ;
    skos:definition "Defines the amount of time by which the targetted duration may be increased." .

odm:DurationPreWindow a owl:ObjectProperty,
        linkml:SlotDefinition ;
    rdfs:label "DurationPreWindow" ;
    rdfs:range odm:DurationDatetime ;
    skos:definition "Defines the amount of time by which the targetted duration may be reduced." .

odm:DurationTarget a owl:ObjectProperty,
        linkml:SlotDefinition ;
    rdfs:label "DurationTarget" ;
    rdfs:range odm:DurationDatetime ;
    skos:definition "Constrains the duration of an activity represented by a Study, Epoch, StudyEventGroupDef, StudyEventDef, ItemGroupDef or ItemDef. Specifies the planned duration of the referenced structural element." .

odm:DurationTimingConstraintRef a owl:ObjectProperty,
        linkml:SlotDefinition ;
    rdfs:label "DurationTimingConstraintRef" ;
    rdfs:range odm:DurationTimingConstraint ;
    skos:definition "DurationTimingConstraint reference: The DurationTimingConstraint constrains the duration of an activity represented by a study, epoch, StudyEventGroupDef, StudyEventDef, ItemGroupDef, or ItemDef. It is used to constrain the duration of the visit, activity, or any other structural element." .

odm:EditPoint a owl:ObjectProperty,
        linkml:SlotDefinition ;
    rdfs:label "EditPoint" ;
    rdfs:range odm:EditPointType ;
    skos:definition "Identifies the phase of data processing in which update action occurred." .

odm:EffectiveDate a owl:ObjectProperty,
        linkml:SlotDefinition ;
    rdfs:label "EffectiveDate" ;
    rdfs:range odm:Date ;
    skos:definition "Datetime stamp when this MetaDataVersion was published at this location." .

odm:EndConditionOID a owl:ObjectProperty,
        linkml:SlotDefinition ;
    rdfs:label "EndConditionOID" ;
    rdfs:range odm:Oidref ;
    skos:definition "The EndConditionOID references a ConditionDef defining the condition under which the transition can be completed. As long as the condition is not met, the transition to the next actitivity or event must be considered to be temporary blocked. When the target structural element can be considered to be a \"visit,\" the condition can be regarded as a visit entry criterion." .

odm:EndOID a owl:ObjectProperty,
        linkml:SlotDefinition ;
    rdfs:label "EndOID" ;
    rdfs:range odm:Oidref ;
    skos:definition "Reference to the definition of the structural element that ends the workflow. It may be a StudyEventGroupDef, StudyEventDef, ItemGroupDef, or ItemDef element." .

odm:EpochOID a owl:ObjectProperty,
        linkml:SlotDefinition ;
    rdfs:label "EpochOID" ;
    rdfs:range odm:Oidref ;
    skos:definition "Reference to an Epoch element defined in the study." .

odm:EpochRef a owl:ObjectProperty,
        linkml:SlotDefinition ;
    rdfs:label "EpochRef" ;
    rdfs:range odm:Epoch ;
    skos:definition "Epoch reference: The planned period of subjects' participation in the trial is divided into sequential epochs. Each epoch is a period of time that serves a purpose in the trial as a whole. Epochs cannot overlap. The sequence of the epoch in the study is provided by the SequenceNumber attribute, the first epoch in the study being assigned the sequence number 1. Sequence numbers are subsequent." .

odm:ErrorMessageRef a owl:ObjectProperty,
        linkml:SlotDefinition ;
    rdfs:label "ErrorMessageRef" ;
    rdfs:range odm:ErrorMessage ;
    skos:definition "ErrorMessage reference: Error message provided to user when the range check fails." .

odm:ExclusionCriteriaRef a owl:ObjectProperty,
        linkml:SlotDefinition ;
    rdfs:label "ExclusionCriteriaRef" ;
    rdfs:range odm:ExclusionCriteria ;
    skos:definition "ExclusionCriteria reference: The ExclusionCriteria is a container element for Criterion elements describing exclusion criteria for subjects in the study. When a list is provided, not meeting any of the criteria in the list may lead to exclusion of enrollment in the study." .

odm:ExtendedValue a owl:ObjectProperty,
        linkml:SlotDefinition ;
    rdfs:label "ExtendedValue" ;
    rdfs:range odm:YesOnly .

odm:ExternalCodeLibRef a owl:ObjectProperty,
        linkml:SlotDefinition ;
    rdfs:label "ExternalCodeLibRef" ;
    rdfs:range odm:ExternalCodeLib ;
    skos:definition "ExternalCodeLib reference: The ExternalCodeLib element references a FormalExpression in an external code library, such as a file or GitHub. The intention is to make it possible to reference existing code libraries where the code is maintained as well as making it simpler to include longer, more complex FormalExpressions. The Library attribute provides the name of the external library, whereas ref or href provides a reference to the repository that can be used to retrieve the code. The Method attribute provides the name of the method in the file referenced for cases where multiple methods are provided in the source code file. The Version element provides the version of the external FormalExpression code referenced." .

odm:FamilyNameRef a owl:ObjectProperty,
        linkml:SlotDefinition ;
    rdfs:label "FamilyNameRef" ;
    rdfs:range odm:FamilyName ;
    skos:definition "FamilyName reference: The user's surname (family name)." .

odm:FileOID a owl:ObjectProperty,
        linkml:SlotDefinition ;
    rdfs:label "FileOID" ;
    rdfs:range odm:Oid ;
    skos:definition "A unique identifier for this file." .

odm:FileTypeRef a owl:ObjectProperty,
        linkml:SlotDefinition ;
    rdfs:label "FileTypeRef" ;
    rdfs:range odm:FileType ;
    skos:definition "Snapshot means that the document contains only the current state of the data and metadata it describes, and no transactional history. Transactional means that the document may contain more than one instance per data point. Query means the document contains only ClinicalData/Query elements." .

odm:FirstPage a owl:ObjectProperty,
        linkml:SlotDefinition ;
    rdfs:label "FirstPage" ;
    rdfs:range odm:PositiveInteger ;
    skos:definition "First page in a range of pages." .

odm:FlagRef a owl:ObjectProperty,
        linkml:SlotDefinition ;
    rdfs:label "FlagRef" ;
    rdfs:range odm:Flag ;
    skos:definition "Flag reference: A machine-processable annotation." .

odm:FlagTypeRef a owl:ObjectProperty,
        linkml:SlotDefinition ;
    rdfs:label "FlagTypeRef" ;
    rdfs:range odm:FlagType ;
    skos:definition "FlagType reference: The type of flag. This determines the purpose and semantics of the flag." .

odm:FlagValueRef a owl:ObjectProperty,
        linkml:SlotDefinition ;
    rdfs:label "FlagValueRef" ;
    rdfs:range odm:FlagValue ;
    skos:definition "FlagValue reference: The value of the flag. The meaning of this value is typically dependent on the associated FlagType. The actual value must be a member of the referenced CodeList" .

odm:FullNameRef a owl:ObjectProperty,
        linkml:SlotDefinition ;
    rdfs:label "FullNameRef" ;
    rdfs:range odm:FullName ;
    skos:definition "FullName reference: The user's full formal name. May be a combination of Prefix, GivenName, FamilyName & Suffix. Intended to be used for display." .

odm:GeoPositionRef a owl:ObjectProperty,
        linkml:SlotDefinition ;
    rdfs:label "GeoPositionRef" ;
    rdfs:range odm:GeoPosition ;
    skos:definition "GeoPosition reference: The geographical position using the World Geodetic System WGS84." .

odm:GivenNameRef a owl:ObjectProperty,
        linkml:SlotDefinition ;
    rdfs:label "GivenNameRef" ;
    rdfs:range odm:GivenName ;
    skos:definition "GivenName reference: The user's initial given name or all given names." .

odm:GranularityRef a owl:ObjectProperty,
        linkml:SlotDefinition ;
    rdfs:label "GranularityRef" ;
    rdfs:range odm:Granularity ;
    skos:definition "Granularity is intended to give the sender a shorthand way to Describes the scope of information in the document, for certain common types of documents. All means the entire study; Metadata means the Study/MetaDataVersion element; AdminData and ReferenceData mean the corresponding elements; AllClinicalData means all of the ClinicalData collected for the study. SingleSite, means all of the Clinical Data for a single study site. SingleSubject means all of the Clinical Data for a single Subject." .

odm:HouseNumberRef a owl:ObjectProperty,
        linkml:SlotDefinition ;
    rdfs:label "HouseNumberRef" ;
    rdfs:range odm:HouseNumber ;
    skos:definition "HouseNumber reference: The house number part of a user's postal address." .

odm:ImageFileName a owl:ObjectProperty,
        linkml:SlotDefinition ;
    rdfs:label "ImageFileName" ;
    rdfs:range odm:FileName ;
    skos:definition "The file name of or file path to the picture" .

odm:ImageRef a owl:ObjectProperty,
        linkml:SlotDefinition ;
    rdfs:label "ImageRef" ;
    rdfs:range odm:Image ;
    skos:definition "Image reference: A visual depiction of the user." .

odm:ImplementationNotesRef a owl:ObjectProperty,
        linkml:SlotDefinition ;
    rdfs:label "ImplementationNotesRef" ;
    rdfs:range odm:ImplementationNotes ;
    skos:definition "ImplementationNotes reference: Further information, such as rationale and implementation instructions, on how to implement the CRF data collection fields." .

odm:IncludeRef a owl:ObjectProperty,
        linkml:SlotDefinition ;
    rdfs:label "IncludeRef" ;
    rdfs:range odm:Include ;
    skos:definition "Include reference: The Include metadata element allows a reference to a prior metadata version." .

odm:InclusionCriteriaRef a owl:ObjectProperty,
        linkml:SlotDefinition ;
    rdfs:label "InclusionCriteriaRef" ;
    rdfs:range odm:InclusionCriteria ;
    skos:definition "InclusionCriteria reference: The InclusionCriteria is a container element for Criterion elements describing inclusion criteria for subjects in the study. When a list is provided, subjects must meet each of the criteria in the list in order to enroll in the study." .

odm:InclusionExclusionCriteriaRef a owl:ObjectProperty,
        linkml:SlotDefinition ;
    rdfs:label "InclusionExclusionCriteriaRef" ;
    rdfs:range odm:InclusionExclusionCriteria ;
    skos:definition "InclusionExclusionCriteria reference: The InclusionExclusionCriteria element can contain 2 lists of Criterion elements, represented by the 2 elements InclusionCriteria and ExclusionCriteria. Together, these criteria determine the eligibility of a subject for the study. The actual condition to be evaluated is contained in an ODM ConditionDef, which is referenced by each Criterion‟s ConditionOID attribute." .

odm:IntercurrentEventRef a owl:ObjectProperty,
        linkml:SlotDefinition ;
    rdfs:label "IntercurrentEventRef" ;
    rdfs:range odm:IntercurrentEvent ;
    skos:definition "IntercurrentEvent reference: None" .

odm:InvestigatorRefRef a owl:ObjectProperty,
        linkml:SlotDefinition ;
    rdfs:label "InvestigatorRefRef" ;
    rdfs:range odm:InvestigatorRef ;
    skos:definition "InvestigatorRef reference: Provides a reference to the user who created the SubjectData record in the source system." .

odm:IsNull a owl:ObjectProperty,
        linkml:SlotDefinition ;
    rdfs:label "IsNull" ;
    rdfs:range odm:YesOnly ;
    skos:definition "Flag specifying that an item's value is to be set to null. In the interest of creating non-verbose XML instances, one should not use ItemData elements with IsNull set to \"Yes\" to indicate uncollected data. The better practice is to transmit only collected data. For use cases where data traceability is important, providing ItemData elements with IsNull=\"Yes\" maybe be useful. It is not necessary to provide an ItemData element with IsNull set to \"Yes\" in cases where the source system would not create a record." .

odm:IsReferenceData a owl:ObjectProperty,
        linkml:SlotDefinition ;
    rdfs:label "IsReferenceData" ;
    rdfs:range odm:YesOrNo ;
    skos:definition "Specifies whether this ItemGroupDef is used for non-subject data." .

odm:ItemDataRef a owl:ObjectProperty,
        linkml:SlotDefinition ;
    rdfs:label "ItemDataRef" ;
    rdfs:range odm:ItemData ;
    skos:definition "ItemData reference: The ItemData element is used for transmission of the clinical data for an item. The model does not support repeating items within a single item group." .

odm:ItemDefRef a owl:ObjectProperty,
        linkml:SlotDefinition ;
    rdfs:label "ItemDefRef" ;
    rdfs:range odm:ItemDef ;
    skos:definition "ItemDef reference: An ItemDef describes a type of item that can occur within a study. Item properties include name, datatype, range, or codelist restrictions, and several other properties." .

odm:ItemGroupDataSeq a owl:ObjectProperty,
        linkml:SlotDefinition ;
    rdfs:label "ItemGroupDataSeq" ;
    rdfs:range odm:PositiveInteger ;
    skos:definition "Unique sequence # for each ItemGroupData child element (record) in the container element. The ItemGroupDataSeq attribute doesn’t have any other meaning than the sequence in which the items are saved and exchanged for each ItemGroupDef. It is equivalent to the observation # in a dataset." .

odm:ItemGroupDefRef a owl:ObjectProperty,
        linkml:SlotDefinition ;
    rdfs:label "ItemGroupDefRef" ;
    rdfs:range odm:ItemGroupDef ;
    skos:definition "ItemGroupDef reference: An ItemGroupDef describes a type of variable or field grouping that can occur within a study." .

odm:KeySequence a owl:ObjectProperty,
        linkml:SlotDefinition ;
    rdfs:label "KeySequence" ;
    rdfs:range odm:PositiveInteger ;
    skos:definition "Indicates that this item is a key for the enclosing element. It also provides an ordering for the keys." .

odm:KeySetRef a owl:ObjectProperty,
        linkml:SlotDefinition ;
    rdfs:label "KeySetRef" ;
    rdfs:range odm:KeySet ;
    skos:definition "KeySet reference: A KeySet references a single entity (e.g., a study, a subject, a study event). Only those attributes needed to specify the particular entity are required, and all others must be omitted (see Section 2.7, Clinical Data Keys)." .

odm:LastPage a owl:ObjectProperty,
        linkml:SlotDefinition ;
    rdfs:label "LastPage" ;
    rdfs:range odm:PositiveInteger ;
    skos:definition "Last page in a range of pages." .

odm:LastUpdateDatetime a owl:ObjectProperty,
        linkml:SlotDefinition ;
    rdfs:label "LastUpdateDatetime" ;
    rdfs:range odm:Datetime ;
    skos:definition "When was this Query updated? Will correspond to the creation date or the last updated date?" .

odm:Latitude a owl:ObjectProperty,
        linkml:SlotDefinition ;
    rdfs:label "Latitude" ;
    rdfs:range odm:Decimal ;
    skos:definition "Latitude component of geoposition coordinate in decimal degrees degrees. May require conversion from degrees, minutes, seconds format." .

odm:LeafID a owl:ObjectProperty,
        linkml:SlotDefinition ;
    rdfs:label "LeafID" ;
    rdfs:range odm:Oid ;
    skos:definition "Unique identifier for the Leaf element with the document location." .

odm:LegalReasonRef a owl:ObjectProperty,
        linkml:SlotDefinition ;
    rdfs:label "LegalReasonRef" ;
    rdfs:range odm:LegalReason ;
    skos:definition "LegalReason reference: The responsibility statement associated with a signature (e.g., \"The signer accepts responsibility for the accuracy of this data.\")." .

odm:Length a owl:ObjectProperty,
        linkml:SlotDefinition ;
    rdfs:label "Length" ;
    rdfs:range odm:PositiveInteger ;
    skos:definition """The Length attribute is optional when DataType is text, string,
                    integer, or float; and should not be used for the other
                    datatypes.""" .

odm:Library a owl:ObjectProperty,
        linkml:SlotDefinition ;
    rdfs:label "Library" ;
    rdfs:range odm:Name ;
    skos:definition "The name of the external library containing the FormalExpression." .

odm:Longitude a owl:ObjectProperty,
        linkml:SlotDefinition ;
    rdfs:label "Longitude" ;
    rdfs:range odm:Decimal ;
    skos:definition "Longitude component of geoposition coordinates in decimal degrees. May require conversion from degrees, minutes, seconds format." .

odm:MeaningRef a owl:ObjectProperty,
        linkml:SlotDefinition ;
    rdfs:label "MeaningRef" ;
    rdfs:range odm:Meaning ;
    skos:definition "Meaning reference: A short name or description for this signature. It should reflect the context of the signature and/or the text that appears when the signature is applied in the user interface." .

odm:Method a owl:ObjectProperty,
        linkml:SlotDefinition ;
    rdfs:label "Method" ;
    rdfs:range odm:Name ;
    skos:definition "The name of the method or function that contains the FormalExpression code." .

odm:MethodDefRef a owl:ObjectProperty,
        linkml:SlotDefinition ;
    rdfs:label "MethodDefRef" ;
    rdfs:range odm:MethodDef ;
    skos:definition "MethodDef reference: A MethodDef defines how a data value can be obtained from a collection of other data values." .

odm:Methodology a owl:ObjectProperty,
        linkml:SlotDefinition ;
    rdfs:label "Methodology" ;
    rdfs:range odm:SignMethod ;
    skos:definition "Defines the type of electronic signature, including the meaning as required by 21 CFR Part 11 ." .

odm:MimeType a owl:ObjectProperty,
        linkml:SlotDefinition ;
    rdfs:label "MimeType" ;
    rdfs:range odm:Text ;
    skos:definition "Media type of the image" .

odm:ODMFileMetadata a owl:Class,
        linkml:ClassDefinition ;
    rdfs:label "ODMFileMetadata" ;
    rdfs:subClassOf [ a owl:Restriction ;
            owl:maxQualifiedCardinality 1 ;
            owl:onClass odm:ODMVersion ;
            owl:onProperty odm:ODMVersionRef ],
        [ a owl:Restriction ;
            owl:maxQualifiedCardinality 1 ;
            owl:onClass odm:Context ;
            owl:onProperty odm:ContextRef ],
        [ a owl:Restriction ;
            owl:onClass odm:FileType ;
            owl:onProperty odm:FileTypeRef ;
            owl:qualifiedCardinality 1 ],
        [ a owl:Restriction ;
            owl:maxQualifiedCardinality 1 ;
            owl:onClass odm:Text ;
            owl:onProperty odm:SourceSystemVersion ],
        [ a owl:Restriction ;
            owl:maxQualifiedCardinality 1 ;
            owl:onClass odm:Text ;
            owl:onProperty odm:Originator ],
        [ a owl:Restriction ;
            owl:maxQualifiedCardinality 1 ;
            owl:onClass odm:Description ;
            owl:onProperty odm:DescriptionRef ],
        [ a owl:Restriction ;
            owl:maxQualifiedCardinality 1 ;
            owl:onClass odm:Datetime ;
            owl:onProperty odm:AsOfDateTime ],
        [ a owl:Restriction ;
            owl:maxQualifiedCardinality 1 ;
            owl:onClass odm:Oidref ;
            owl:onProperty odm:PriorFileOID ],
        [ a owl:Restriction ;
            owl:maxQualifiedCardinality 1 ;
            owl:onClass odm:Granularity ;
            owl:onProperty odm:GranularityRef ],
        [ a owl:Restriction ;
            owl:allValuesFrom odm:Study ;
            owl:onProperty odm:StudyRef ],
        [ a owl:Restriction ;
            owl:allValuesFrom odm:ReferenceData ;
            owl:onProperty odm:ReferenceDataRef ],
        [ a owl:Restriction ;
            owl:maxQualifiedCardinality 1 ;
            owl:onClass odm:Text ;
            owl:onProperty odm:SourceSystem ],
        [ a owl:Restriction ;
            owl:allValuesFrom odm:ClinicalData ;
            owl:onProperty odm:ClinicalDataRef ],
        [ a owl:Restriction ;
            owl:onClass odm:Datetime ;
            owl:onProperty odm:CreationDateTime ;
            owl:qualifiedCardinality 1 ],
        [ a owl:Restriction ;
            owl:allValuesFrom odm:Association ;
            owl:onProperty odm:AssociationRef ],
        [ a owl:Restriction ;
            owl:allValuesFrom odm:AdminData ;
            owl:onProperty odm:AdminDataRef ],
        [ a owl:Restriction ;
            owl:onClass odm:Oid ;
            owl:onProperty odm:FileOID ;
            owl:qualifiedCardinality 1 ] ;
    skos:definition "Root element for ODM Documents. The ODM element is the top-level (root) element of each ODM document." ;
    skos:exactMatch odm:ODM .

odm:ODMVersionRef a owl:ObjectProperty,
        linkml:SlotDefinition ;
    rdfs:label "ODMVersionRef" ;
    rdfs:range odm:ODMVersion ;
    skos:definition "The version of the ODM standard used." .

odm:OrganizationRef a owl:ObjectProperty,
        linkml:SlotDefinition ;
    rdfs:label "OrganizationRef" ;
    rdfs:range odm:Organization ;
    skos:definition "Organization reference: An organization can reference a parent organization. Users may be associated with an Organization. An Organization may be associated with a Location. A User, Location, or Organization may have an address." .

odm:Originator a owl:ObjectProperty,
        linkml:SlotDefinition ;
    rdfs:label "Originator" ;
    rdfs:range odm:Text ;
    skos:definition "The organization that generated the ODM file." .

odm:OtherTextRef a owl:ObjectProperty,
        linkml:SlotDefinition ;
    rdfs:label "OtherTextRef" ;
    rdfs:range odm:OtherText ;
    skos:definition "OtherText reference: Any other text needed as part of a user's postal address." .

odm:PDFPageRefRef a owl:ObjectProperty,
        linkml:SlotDefinition ;
    rdfs:label "PDFPageRefRef" ;
    rdfs:range odm:PDFPageRef ;
    skos:definition "The PDFPageRef element is a container for page references in a PDF file." .

odm:PageRefs a owl:ObjectProperty,
        linkml:SlotDefinition ;
    rdfs:label "PageRefs" ;
    rdfs:range odm:Text ;
    skos:definition "List of PDF pages separated by a space." .

odm:ParameterRef a owl:ObjectProperty,
        linkml:SlotDefinition ;
    rdfs:label "ParameterRef" ;
    rdfs:range odm:Parameter ;
    skos:definition "Parameter reference: The Parameter element represents a method parameter used as part of a MethodSignature in MethodDef, ConditionDef, or RangeCheck." .

odm:ParameterValueRef a owl:ObjectProperty,
        linkml:SlotDefinition ;
    rdfs:label "ParameterValueRef" ;
    rdfs:range odm:ParameterValue ;
    skos:definition "ParameterValue reference: This element contains the value of the study parameter as text content." .

odm:ParentClass a owl:ObjectProperty,
        linkml:SlotDefinition ;
    rdfs:label "ParentClass" ;
    rdfs:range odm:ItemGroupClassSubClass ;
    skos:definition "Parent class of the Sub Class" .

odm:PartOfOrganizationOID a owl:ObjectProperty,
        linkml:SlotDefinition ;
    rdfs:label "PartOfOrganizationOID" ;
    rdfs:range odm:Oidref ;
    skos:definition "Reference to a parent organization." .

odm:Path a owl:ObjectProperty,
        linkml:SlotDefinition ;
    rdfs:label "Path" ;
    rdfs:range odm:Text ;
    skos:definition "Provides the machine-executable instruction or template for it to obtain the data or information from the resource. The value of the Path attribute can either be an absolute path, or a relative path starting from the information in the \"Name\" and \"Attribute\" attributes of the parent Resource element." .

odm:PostalCodeRef a owl:ObjectProperty,
        linkml:SlotDefinition ;
    rdfs:label "PostalCodeRef" ;
    rdfs:range odm:PostalCode ;
    skos:definition "PostalCode reference: The postal code part of a user's postal address." .

odm:PreSpecifiedValue a owl:ObjectProperty,
        linkml:SlotDefinition ;
    rdfs:label "PreSpecifiedValue" ;
    rdfs:range odm:Text ;
    skos:definition "Prefill value or a default value for a field that is automatically populated." .

odm:PredecessorOID a owl:ObjectProperty,
        linkml:SlotDefinition ;
    rdfs:label "PredecessorOID" ;
    rdfs:range odm:Oidref ;
    skos:definition "Identifies a StudyEventGroup, StudyEvent, ItemGroup or Item that occurs immediately before the RelativeTimepointTarget." .

odm:PrefixRef a owl:ObjectProperty,
        linkml:SlotDefinition ;
    rdfs:label "PrefixRef" ;
    rdfs:range odm:Prefix ;
    skos:definition "Prefix reference: Title or other prefix. Maps to FHIR HumanName.prefix (https://www.hl7.org/fhir/datatypes.html#humanname)." .

odm:PriorFileOID a owl:ObjectProperty,
        linkml:SlotDefinition ;
    rdfs:label "PriorFileOID" ;
    rdfs:range odm:Oidref ;
    skos:definition "Reference to the previous file (if any) in a series." .

odm:PromptRef a owl:ObjectProperty,
        linkml:SlotDefinition ;
    rdfs:label "PromptRef" ;
    rdfs:range odm:Prompt ;
    skos:definition "Prompt reference: A prompt text shown to a human user when prompted to provide data for an item on paper or on a screen. The Prompt is a short version of the question." .

odm:ProtocolName a owl:ObjectProperty,
        linkml:SlotDefinition ;
    rdfs:label "ProtocolName" ;
    rdfs:range odm:Name ;
    skos:definition "P rotocol identifier or protocol number assigned to the study . It is used by the regulatory authority or clinical trial registry." .

odm:ProtocolRef a owl:ObjectProperty,
        linkml:SlotDefinition ;
    rdfs:label "ProtocolRef" ;
    rdfs:range odm:Protocol ;
    skos:definition "Protocol reference: The Protocol element lists the kinds of study events that can occur within a specific version of a study. All clinical data must occur within one of these study events." .

odm:PublishingSet a owl:ObjectProperty,
        linkml:SlotDefinition ;
    rdfs:label "PublishingSet" ;
    rdfs:range odm:StandardPublishingSet ;
    skos:definition "Set of published files of Standard when Type=\"CT\" (e.g. SDTM, ADaM, SEND, CDASH, COA)." .

odm:Purpose a owl:ObjectProperty,
        linkml:SlotDefinition ;
    rdfs:label "Purpose" ;
    rdfs:range odm:Text ;
    skos:definition "Purpose of the ItemGroup." .

odm:QuestionRef a owl:ObjectProperty,
        linkml:SlotDefinition ;
    rdfs:label "QuestionRef" ;
    rdfs:range odm:Question ;
    skos:definition "Question reference: A label shown to a human user when prompted to provide data for an item on paper or on a screen." .

odm:Rank a owl:ObjectProperty,
        linkml:SlotDefinition ;
    rdfs:label "Rank" ;
    rdfs:range odm:Decimal ;
    skos:definition "Numeric significance of the CodeListItem relative to others in the CodeList. The Rank attribute may be used where the relative value corresponding to an enumeration cannot or should not be determined by its lexical order. For example, if you have a list of enumerated text values including \"Low\", \"Medium\", and \"High\" and wish to assign these relative numeric values 1, 2, and 3 respectively, you should include a Rank attribute for each CodeListItem defined. Without the applied rank attribute, the normal lexical ordering would be \"High\", \"Low\", and \"Medium\"." .

odm:ReasonForChangeRef a owl:ObjectProperty,
        linkml:SlotDefinition ;
    rdfs:label "ReasonForChangeRef" ;
    rdfs:range odm:ReasonForChange ;
    skos:definition "ReasonForChange reference: A user-supplied reason for a data change." .

odm:ReferenceDataRef a owl:ObjectProperty,
        linkml:SlotDefinition ;
    rdfs:label "ReferenceDataRef" ;
    rdfs:range odm:ReferenceData ;
    skos:definition "ReferenceData reference: Reference data provides information on how to interpret clinical data. For example, reference data might include lab normal ranges. For a study that uses CDISC standards, reference data might include SDTM Trial Design datasets." .

odm:RelativeTimingConstraintRef a owl:ObjectProperty,
        linkml:SlotDefinition ;
    rdfs:label "RelativeTimingConstraintRef" ;
    rdfs:range odm:RelativeTimingConstraint ;
    skos:definition "RelativeTimingConstraint reference: The RelativeTimingConstraint element describes a relative timing constraint between 2 activities or groups of activities, represented by StudyEventGroups, StudyEvents, ItemGroups, or Items." .

odm:Repeat a owl:ObjectProperty,
        linkml:SlotDefinition ;
    rdfs:label "Repeat" ;
    rdfs:range odm:YesOnly ;
    skos:definition "Indicates that the item serves as the item over which repeats are to be performed." .

odm:RepeatingLimit a owl:ObjectProperty,
        linkml:SlotDefinition ;
    rdfs:label "RepeatingLimit" ;
    rdfs:range odm:PositiveInteger ;
    skos:definition "Maximum number of repeats." .

odm:ResourceRef a owl:ObjectProperty,
        linkml:SlotDefinition ;
    rdfs:label "ResourceRef" ;
    rdfs:range odm:Resource ;
    skos:definition "Resource reference: Describes an external resource used as the source for the parent ItemGroup or Item." .

odm:ReturnValueRef a owl:ObjectProperty,
        linkml:SlotDefinition ;
    rdfs:label "ReturnValueRef" ;
    rdfs:range odm:ReturnValue ;
    skos:definition "ReturnValue reference: The ReturnValue element represents a return value used as part of a MethodSignature in MethodDef, ConditionDef, or RangeCheck. A return value identifies values passed from the Method to the calling element. A ReturnValue may be computed by a FormalExpression." .

odm:RoleCodeListOID a owl:ObjectProperty,
        linkml:SlotDefinition ;
    rdfs:label "RoleCodeListOID" ;
    rdfs:range odm:Oidref ;
    skos:definition "Reference to a CodeList that defines the allowable values of Role for the Study." .

odm:SelectionRef a owl:ObjectProperty,
        linkml:SlotDefinition ;
    rdfs:label "SelectionRef" ;
    rdfs:range odm:Selection ;
    skos:definition "Selection reference: Template for machine-readable/executable expression for retrieving the data or information from an external resource." .

odm:SequenceNumber a owl:ObjectProperty,
        linkml:SlotDefinition ;
    rdfs:label "SequenceNumber" ;
    rdfs:range odm:PositiveInteger ;
    skos:definition "Order of the Epoch" .

odm:ShortName a owl:ObjectProperty,
        linkml:SlotDefinition ;
    rdfs:label "ShortName" ;
    rdfs:range odm:Name ;
    skos:definition "Short name or code for the parameter." .

odm:SignatureDefRef a owl:ObjectProperty,
        linkml:SlotDefinition ;
    rdfs:label "SignatureDefRef" ;
    rdfs:range odm:SignatureDef ;
    skos:definition "SignatureDef reference: Provides Metadata for signatures included in the /ODM/ClinicalData." .

odm:SignatureOID a owl:ObjectProperty,
        linkml:SlotDefinition ;
    rdfs:label "SignatureOID" ;
    rdfs:range odm:Oidref ;
    skos:definition "Reference to the SignatureDef ." .

odm:SiteRefRef a owl:ObjectProperty,
        linkml:SlotDefinition ;
    rdfs:label "SiteRefRef" ;
    rdfs:range odm:SiteRef ;
    skos:definition "SiteRef reference: lement NameSiteRefParent ElementsSubjectDataElement XPath(s)/ODM/ClinicalData/SubjectData/SiteRefElement Textual ValueNoneAttributesLocationOIDChild ElementsNoneUsage/Business RulesBusiness Rule(s):Must be provided when the /ODM/FileType is Transactional." .

odm:SoftHard a owl:ObjectProperty,
        linkml:SlotDefinition ;
    rdfs:label "SoftHard" ;
    rdfs:range odm:SoftOrHard ;
    skos:definition "Type of range check. Soft indicates that a warning occurs when the RangeCheck fails. Hard indicates that an error occurs when the RangeCheck fails." .

odm:SourceIDRef a owl:ObjectProperty,
        linkml:SlotDefinition ;
    rdfs:label "SourceIDRef" ;
    rdfs:range odm:SourceID ;
    skos:definition "SourceID reference: Information that identifies the source of the data within an originating system." .

odm:SourceItemRef a owl:ObjectProperty,
        linkml:SlotDefinition ;
    rdfs:label "SourceItemRef" ;
    rdfs:range odm:SourceItem ;
    skos:definition "SourceItem reference: Provides the information needed to identify the source metadata." .

odm:SourceItemsRef a owl:ObjectProperty,
        linkml:SlotDefinition ;
    rdfs:label "SourceItemsRef" ;
    rdfs:range odm:SourceItems ;
    skos:definition "SourceItems reference: Identifies source items as needed to support automated data capture and end-to-end traceability." .

odm:SourceOID a owl:ObjectProperty,
        linkml:SlotDefinition ;
    rdfs:label "SourceOID" ;
    rdfs:range odm:Oidref ;
    skos:definition "References the definition of the source structural element for the transition. The structural element may be a StudyEventGroupDef, StudyEventDef, ItemGroupDef, ItemDef, or Branching element." .

odm:SourceSystem a owl:ObjectProperty,
        linkml:SlotDefinition ;
    rdfs:label "SourceSystem" ;
    rdfs:range odm:Text ;
    skos:definition "The computer system or database management system that is the source of the information in this file." .

odm:SourceSystemVersion a owl:ObjectProperty,
        linkml:SlotDefinition ;
    rdfs:label "SourceSystemVersion" ;
    rdfs:range odm:Text ;
    skos:definition "The version of the \"SourceSystem\" above." .

odm:SponsorOrSite a owl:ObjectProperty,
        linkml:SlotDefinition ;
    rdfs:label "SponsorOrSite" ;
    rdfs:range odm:CommentType ;
    skos:definition "Source of the comment." .

odm:StandardRef a owl:ObjectProperty,
        linkml:SlotDefinition ;
    rdfs:label "StandardRef" ;
    rdfs:range odm:Standard ;
    skos:definition "Definition of a standard referenced in the Define-XML document." .

odm:StandardsRef a owl:ObjectProperty,
        linkml:SlotDefinition ;
    rdfs:label "StandardsRef" ;
    rdfs:range odm:Standards ;
    skos:definition "Standards reference: The Standards element provides a container for the list of Standard elements referenced in the MetaDataVersion for the Study.." .

odm:StartConditionOID a owl:ObjectProperty,
        linkml:SlotDefinition ;
    rdfs:label "StartConditionOID" ;
    rdfs:range odm:Oidref ;
    skos:definition "The StartConditionOID references a ConditionDef specifying a condition that must be met for the transition to start. For example, if the source structural element is a StudyEventGroupDef describing the activities for study screening and the target structural element is a StudyEventGroupDef describing study enrollment, the ConditionDef referenced by the StartConditionOID specifies the criteria that must be met for a subject to transition from screening to enrollment." .

odm:StartOID a owl:ObjectProperty,
        linkml:SlotDefinition ;
    rdfs:label "StartOID" ;
    rdfs:range odm:Oidref ;
    skos:definition "Reference to the definition of the structural element that starts the workflow. It may be a StudyEventGroupDef, StudyEventDef, ItemGroupDef, or ItemDef element." .

odm:State a owl:ObjectProperty,
        linkml:SlotDefinition ;
    rdfs:label "State" ;
    rdfs:range odm:QueryStateType ;
    skos:definition "Status of the Query" .

odm:StateProvRef a owl:ObjectProperty,
        linkml:SlotDefinition ;
    rdfs:label "StateProvRef" ;
    rdfs:range odm:StateProv ;
    skos:definition "StateProv reference: The state or province name part of a user's postal address." .

odm:StreetNameRef a owl:ObjectProperty,
        linkml:SlotDefinition ;
    rdfs:label "StreetNameRef" ;
    rdfs:range odm:StreetName ;
    skos:definition "StreetName reference: The street name part of a user's postal address." .

odm:StructuralElementOID a owl:ObjectProperty,
        linkml:SlotDefinition ;
    rdfs:label "StructuralElementOID" ;
    rdfs:range odm:Oidref ;
    skos:definition "OID of a structural element such as a Study, Epoch, StudyEventGroup, StudyEvent, ItemGroup, Item" .

odm:Structure a owl:ObjectProperty,
        linkml:SlotDefinition ;
    rdfs:label "Structure" ;
    rdfs:range odm:Text ;
    skos:definition "Description of the level of detail represented by individual records in the ItemGroup" .

odm:StudyEndPointOID a owl:ObjectProperty,
        linkml:SlotDefinition ;
    rdfs:label "StudyEndPointOID" ;
    rdfs:range odm:Oidref ;
    skos:definition "Reference to the StudyEndPoint ." .

odm:StudyEndPointsRef a owl:ObjectProperty,
        linkml:SlotDefinition ;
    rdfs:label "StudyEndPointsRef" ;
    rdfs:range odm:StudyEndPoints ;
    skos:definition "StudyEndPoints reference: Go to start of metadata" .

odm:StudyEstimandRef a owl:ObjectProperty,
        linkml:SlotDefinition ;
    rdfs:label "StudyEstimandRef" ;
    rdfs:range odm:StudyEstimand ;
    skos:definition "StudyEstimand reference: None" .

odm:StudyEstimandsRef a owl:ObjectProperty,
        linkml:SlotDefinition ;
    rdfs:label "StudyEstimandsRef" ;
    rdfs:range odm:StudyEstimands ;
    skos:definition "StudyEstimands reference: None" .

odm:StudyEventDataRef a owl:ObjectProperty,
        linkml:SlotDefinition ;
    rdfs:label "StudyEventDataRef" ;
    rdfs:range odm:StudyEventData ;
    skos:definition "StudyEventData reference: Clinical data for a study event (visit). The model supports repeating study events (e.g., when the same set of information is collected for a series of patient visits)." .

odm:StudyEventDefRef a owl:ObjectProperty,
        linkml:SlotDefinition ;
    rdfs:label "StudyEventDefRef" ;
    rdfs:range odm:StudyEventDef ;
    skos:definition "StudyEventDef reference: StudyEventDef represents the definition of an activity in a study where data is collected. For example, a study event may represent a set of item groups that represent data collection instruments to be completed for a subject during a visit in a study. The visit occurs as part of a study workflow, and the workflow is referenced in the study event." .

odm:StudyEventGroupDefRef a owl:ObjectProperty,
        linkml:SlotDefinition ;
    rdfs:label "StudyEventGroupDefRef" ;
    rdfs:range odm:StudyEventGroupDef ;
    skos:definition "StudyEventGroupDef reference: StudyEventGroupDef is a study building block that groups a number of smaller building blocks, which can themselves be StudyEventGroups or StudyEvents. It thus allows nesting of building blocks." .

odm:StudyIndicationRef a owl:ObjectProperty,
        linkml:SlotDefinition ;
    rdfs:label "StudyIndicationRef" ;
    rdfs:range odm:StudyIndication ;
    skos:definition "StudyIndication reference: This element describes a study indication (e.g., condition, disease) for the clinical study. The human-readable description is provided in the Description element. The Coding element can be used to provide a machine-readable code for the indication (e.g., SNOMED-CT code 26929004 for \"Alzheimer's disease\")." .

odm:StudyIndicationsRef a owl:ObjectProperty,
        linkml:SlotDefinition ;
    rdfs:label "StudyIndicationsRef" ;
    rdfs:range odm:StudyIndications ;
    skos:definition "StudyIndications reference: StudyIndications is a container element for individual StudyIndication elements." .

odm:StudyInterventionOID a owl:ObjectProperty,
        linkml:SlotDefinition ;
    rdfs:label "StudyInterventionOID" ;
    rdfs:range odm:Oidref ;
    skos:definition "Reference to a StudyIntervention" .

odm:StudyInterventionsRef a owl:ObjectProperty,
        linkml:SlotDefinition ;
    rdfs:label "StudyInterventionsRef" ;
    rdfs:range odm:StudyInterventions ;
    skos:definition "StudyInterventions reference: The StudyInterventions element is a container element for individual StudyIntervention elements." .

odm:StudyName a owl:ObjectProperty,
        linkml:SlotDefinition ;
    rdfs:label "StudyName" ;
    rdfs:range odm:Name ;
    skos:definition "Sponsoring organization's internal name for the study. If no internal name is available, the value is expected to be the same value as ProtocolName." .

odm:StudyObjectiveRef a owl:ObjectProperty,
        linkml:SlotDefinition ;
    rdfs:label "StudyObjectiveRef" ;
    rdfs:range odm:StudyObjective ;
    skos:definition "StudyObjective reference: None" .

odm:StudyObjectivesRef a owl:ObjectProperty,
        linkml:SlotDefinition ;
    rdfs:label "StudyObjectivesRef" ;
    rdfs:range odm:StudyObjectives ;
    skos:definition "StudyObjectives reference: The StudyObjectives is a container element for individual StudyObjective elements." .

odm:StudyParameterRef a owl:ObjectProperty,
        linkml:SlotDefinition ;
    rdfs:label "StudyParameterRef" ;
    rdfs:range odm:StudyParameter ;
    skos:definition "StudyParameter reference: A StudyParameter defines a study design parameter for which the value or values are delivered in the ParameterValue child element or elements." .

odm:StudyRef a owl:ObjectProperty,
        linkml:SlotDefinition ;
    rdfs:label "StudyRef" ;
    rdfs:range odm:Study ;
    skos:definition "Study reference: This element collects static structural information about an individual study." .

odm:StudyStructureRef a owl:ObjectProperty,
        linkml:SlotDefinition ;
    rdfs:label "StudyStructureRef" ;
    rdfs:range odm:StudyStructure ;
    skos:definition "StudyStructure reference: The StudyStructure element describes the general structure of a clinical study with arms, epochs, and workflows." .

odm:StudySummaryRef a owl:ObjectProperty,
        linkml:SlotDefinition ;
    rdfs:label "StudySummaryRef" ;
    rdfs:range odm:StudySummary ;
    skos:definition "StudySummary reference: The StudyParameter element allows to provide a set of study design parameters such as anticipated number of subjects, minimum and maximum age of the participants, or planned number of arms." .

odm:StudyTargetPopulationOID a owl:ObjectProperty,
        linkml:SlotDefinition ;
    rdfs:label "StudyTargetPopulationOID" ;
    rdfs:range odm:Oidref .

odm:StudyTimingRef a owl:ObjectProperty,
        linkml:SlotDefinition ;
    rdfs:label "StudyTimingRef" ;
    rdfs:range odm:StudyTiming ;
    skos:definition "StudyTiming reference: The StudyTiming element defines a timing constraint within the study, which can be an absolute timing constraint (e.g., start of the screening visit must be between 1 January 2022 and 31 December 2022), a relative timing constraint (e.g., visit 2 must be within 30 days after visit 1 with a window of +/- 1 week), a transition timing constraint (i.e., timing constraint on a transition within a defined workflow), or a duration timing constraint (e.g., the duration of visit 2 is planned to take hours with a window of 30 minutes)." .

odm:StudyTimingsRef a owl:ObjectProperty,
        linkml:SlotDefinition ;
    rdfs:label "StudyTimingsRef" ;
    rdfs:range odm:StudyTimings ;
    skos:definition "StudyTimings reference: The StudyTimings element is a container element for individual StudyTiming elements." .

odm:SubClassRef a owl:ObjectProperty,
        linkml:SlotDefinition ;
    rdfs:label "SubClassRef" ;
    rdfs:range odm:SubClass ;
    skos:definition "SubClass reference: This element contains SubClass definitions." .

odm:SubjectDataRef a owl:ObjectProperty,
        linkml:SlotDefinition ;
    rdfs:label "SubjectDataRef" ;
    rdfs:range odm:SubjectData ;
    skos:definition "SubjectData reference: Clinical data for a single subject." .

odm:SuccessorOID a owl:ObjectProperty,
        linkml:SlotDefinition ;
    rdfs:label "SuccessorOID" ;
    rdfs:range odm:Oidref ;
    skos:definition "Identifies a StudyEventGroup, StudyEvent, ItemGroup or Item tha occurs immediately after the RelativeTimepointTarget." .

odm:SuffixRef a owl:ObjectProperty,
        linkml:SlotDefinition ;
    rdfs:label "SuffixRef" ;
    rdfs:range odm:Suffix ;
    skos:definition "Suffix reference: This element may include credentials, or suffixes (e.g., Jr., III)." .

odm:SummaryMeasureRef a owl:ObjectProperty,
        linkml:SlotDefinition ;
    rdfs:label "SummaryMeasureRef" ;
    rdfs:range odm:SummaryMeasure ;
    skos:definition "SummaryMeasure reference: None" .

odm:SupplementalDocRef a owl:ObjectProperty,
        linkml:SlotDefinition ;
    rdfs:label "SupplementalDocRef" ;
    rdfs:range odm:SupplementalDoc ;
    skos:definition "SupplementalDoc reference: Supplemental data definitions" .

odm:System a owl:ObjectProperty,
        linkml:SlotDefinition ;
    rdfs:label "System" ;
    rdfs:range odm:Uriorcurie ;
    skos:definition "Identifies the code system that defines the code. If the code is taken from a code system resource then the URL for the code system should be used." .

odm:SystemName a owl:ObjectProperty,
        linkml:SlotDefinition ;
    rdfs:label "SystemName" ;
    rdfs:range odm:Text ;
    skos:definition "Human readable name for the code system." .

odm:SystemVersion a owl:ObjectProperty,
        linkml:SlotDefinition ;
    rdfs:label "SystemVersion" ;
    rdfs:range odm:Text ;
    skos:definition "Identifies the version of the code system" .

odm:Target a owl:ObjectProperty,
        linkml:SlotDefinition ;
    rdfs:label "Target" ;
    rdfs:range odm:Text ;
    skos:definition "Element upon which the Query is raised. The parent element is the Target when the Target attribute is omitted." .

odm:TargetOID a owl:ObjectProperty,
        linkml:SlotDefinition ;
    rdfs:label "TargetOID" ;
    rdfs:range odm:Oidref ;
    skos:definition "References the definition of the target structural element for the transition. The structural element may be a StudyEventGroupDef, StudyEventDef, ItemGroupDef, ItemDef, or Branching element. The latter will be used when there is a branching definition necessary as a result of the transition." .

odm:TargetTransitionRef a owl:ObjectProperty,
        linkml:SlotDefinition ;
    rdfs:label "TargetTransitionRef" ;
    rdfs:range odm:TargetTransition ;
    skos:definition "TargetTransition reference: Provides a reference to a Transition element." .

odm:TelecomType a owl:ObjectProperty,
        linkml:SlotDefinition ;
    rdfs:label "TelecomType" ;
    rdfs:range odm:TelecomTypeType .

odm:Term a owl:ObjectProperty,
        linkml:SlotDefinition ;
    rdfs:label "Term" ;
    rdfs:range odm:Name ;
    skos:definition "Longer name. Provides the full name of the parameter." .

odm:TimepointRelativeTarget a owl:ObjectProperty,
        linkml:SlotDefinition ;
    rdfs:label "TimepointRelativeTarget" ;
    rdfs:range odm:DurationDatetime ;
    skos:definition "The relative timing between two activities or groups of activities." .

odm:TransitionOID a owl:ObjectProperty,
        linkml:SlotDefinition ;
    rdfs:label "TransitionOID" ;
    rdfs:range odm:Oidref ;
    skos:definition "References the workflow Transition on which the timing constraint must be executed." .

odm:TransitionRef a owl:ObjectProperty,
        linkml:SlotDefinition ;
    rdfs:label "TransitionRef" ;
    rdfs:range odm:Transition ;
    skos:definition "Transition reference: A Transition defines a link between 2 structural elements in a workflow. When the execution of the transition is dependent upon a timing constraint that is either directly defined or calculated, a TransitionTimingConstraint must be defined, referencing the current Transition." .

odm:TransitionTimingConstraintRef a owl:ObjectProperty,
        linkml:SlotDefinition ;
    rdfs:label "TransitionTimingConstraintRef" ;
    rdfs:range odm:TransitionTimingConstraint ;
    skos:definition "TransitionTimingConstraint reference: The TransitionTimingConstraint element defines a timing constraint on a transition between structural elements as defined in a workflow. As such, it is a non-blocking constraint. This means that the transition is set on hold as long as the timing condition is not fulfilled, and is executed as soon as the timing condition is fulfilled." .

odm:TrialPhaseRef a owl:ObjectProperty,
        linkml:SlotDefinition ;
    rdfs:label "TrialPhaseRef" ;
    rdfs:range odm:TrialPhase ;
    skos:definition "TrialPhase reference: The TrialPhase element designates the phase of the study in the clinical trial." .

odm:UnitsItemOID a owl:ObjectProperty,
        linkml:SlotDefinition ;
    rdfs:label "UnitsItemOID" ;
    rdfs:range odm:Oidref ;
    skos:definition "Reference to a sibling ItemRef element that represents the unit specification for this ItemRef (defines the associated units variable)." .

odm:UsedMethod a owl:ObjectProperty,
        linkml:SlotDefinition ;
    rdfs:label "UsedMethod" ;
    rdfs:range odm:YesOrNo ;
    skos:definition "Indicates that the action was made by the system rather than a data entry form user action." .

odm:UserNameRef a owl:ObjectProperty,
        linkml:SlotDefinition ;
    rdfs:label "UserNameRef" ;
    rdfs:range odm:UserName ;
    skos:definition "UserName reference: The user's login identification in the sender's system." .

odm:UserTypeRef a owl:ObjectProperty,
        linkml:SlotDefinition ;
    rdfs:label "UserTypeRef" ;
    rdfs:range odm:UserType ;
    skos:definition "User's role in the study." .

odm:ValueListDefRef a owl:ObjectProperty,
        linkml:SlotDefinition ;
    rdfs:label "ValueListDefRef" ;
    rdfs:range odm:ValueListDef ;
    skos:definition "ValueListDef reference: The following table specifies the XML structure for valuelist metadata. The ValueListDef element contains ItemRef elements that reference ItemDef elements that provide the value-level metadata details" .

odm:ValueListOID a owl:ObjectProperty,
        linkml:SlotDefinition ;
    rdfs:label "ValueListOID" ;
    rdfs:range odm:Oidref ;
    skos:definition "Reference to the unique ID of a ValueListDef element that provides value-level metadata." .

odm:ValueListRefRef a owl:ObjectProperty,
        linkml:SlotDefinition ;
    rdfs:label "ValueListRefRef" ;
    rdfs:range odm:ValueListRef ;
    skos:definition "ValueListRef reference: The ValueListRef element is the OID of the ValueListDef that contains the valuelist definition associated with the variable. If value-level metadata is required for a variable, a ValueListRef element should be provided as a child element on the ItemDef for the variable definition." .

odm:VariableSet a owl:ObjectProperty,
        linkml:SlotDefinition ;
    rdfs:label "VariableSet" ;
    rdfs:range odm:Text ;
    skos:definition "ADaM variable set, e.g. Dose, Analysis Parameter, Treatment Timing." .

odm:VersionID a owl:ObjectProperty,
        linkml:SlotDefinition ;
    rdfs:label "VersionID" ;
    rdfs:range odm:Name ;
    skos:definition "Identifier for the specific version of the study in the source system that the enclosed Study element metadata refers to." .

odm:VersionName a owl:ObjectProperty,
        linkml:SlotDefinition ;
    rdfs:label "VersionName" ;
    rdfs:range odm:Name ;
    skos:definition "Short descriptive label for the version of the study, e.g. \"Initial go live\" when VersionID = \"<study version ID for Initial go live>\". VersionName may be provided when a VersionID is provided." .

odm:WhereClauseDefRef a owl:ObjectProperty,
        linkml:SlotDefinition ;
    rdfs:label "WhereClauseDefRef" ;
    rdfs:range odm:WhereClauseDef ;
    skos:definition "WhereClauseDef reference: The WhereClauseDef element specifies a condition." .

odm:WhereClauseOID a owl:ObjectProperty,
        linkml:SlotDefinition ;
    rdfs:label "WhereClauseOID" ;
    rdfs:range odm:Oidref ;
    skos:definition "Reference to the unique ID of a WhereClauseDef element" .

odm:WhereClauseRefRef a owl:ObjectProperty,
        linkml:SlotDefinition ;
    rdfs:label "WhereClauseRefRef" ;
    rdfs:range odm:WhereClauseRef ;
    skos:definition "WhereClauseRef reference: The WhereClauseRef references the WhereClauseDef element that describes the conditions under which the variable values are defined by the referenced ItemDef." .

odm:WorkflowDefRef a owl:ObjectProperty,
        linkml:SlotDefinition ;
    rdfs:label "WorkflowDefRef" ;
    rdfs:range odm:WorkflowDef ;
    skos:definition "WorkflowDef reference: A WorkflowDef defines an automated workflow for a study." .

odm:WorkflowEndRef a owl:ObjectProperty,
        linkml:SlotDefinition ;
    rdfs:label "WorkflowEndRef" ;
    rdfs:range odm:WorkflowEnd ;
    skos:definition "WorkflowEnd reference: A WorkflowEnd references a structural element with which the workflows ends." .

odm:WorkflowOID a owl:ObjectProperty,
        linkml:SlotDefinition ;
    rdfs:label "WorkflowOID" ;
    rdfs:range odm:Oidref ;
    skos:definition "Reference to a WorfkflowDef" .

odm:WorkflowStartRef a owl:ObjectProperty,
        linkml:SlotDefinition ;
    rdfs:label "WorkflowStartRef" ;
    rdfs:range odm:WorkflowStart ;
    skos:definition "WorkflowStart reference: WorkflowStart references a structural element that begins the automated workflow." .

odm:_language a owl:ObjectProperty,
        linkml:SlotDefinition ;
    rdfs:label "_language" ;
    rdfs:range odm:LanguageType ;
    skos:definition "language context for internationalisation and localisation" .

odm:leafID a owl:ObjectProperty,
        linkml:SlotDefinition ;
    rdfs:label "leafID" ;
    rdfs:range odm:Oidref ;
    skos:definition "References a leaf element that provides a reference to another ODM document. This is necessary when the source ItemOID references an ItemDef contained in a different ODM document." .

<http://ncicb.nci.nih.gov/xml/odm/EVS/CDISCExtCodeID:C103371> a odm:ItemGroupClass,
        owl:Class ;
    rdfs:label "BASIC DATA STRUCTURE" .

<http://ncicb.nci.nih.gov/xml/odm/EVS/CDISCExtCodeID:C103372> a odm:ItemGroupClass,
        owl:Class ;
    rdfs:label "EVENTS" .

<http://ncicb.nci.nih.gov/xml/odm/EVS/CDISCExtCodeID:C103373> a odm:ItemGroupClass,
        owl:Class ;
    rdfs:label "FINDINGS" .

<http://ncicb.nci.nih.gov/xml/odm/EVS/CDISCExtCodeID:C103374> a odm:ItemGroupClass,
        owl:Class ;
    rdfs:label "INTERVENTIONS" .

<http://ncicb.nci.nih.gov/xml/odm/EVS/CDISCExtCodeID:C103375> a odm:ItemGroupClass,
        owl:Class ;
    rdfs:label "ADAM OTHER" .

<http://ncicb.nci.nih.gov/xml/odm/EVS/CDISCExtCodeID:C103376> a odm:ItemGroupClass,
        owl:Class ;
    rdfs:label "RELATIONSHIP" .

<http://ncicb.nci.nih.gov/xml/odm/EVS/CDISCExtCodeID:C103377> a odm:ItemGroupClass,
        owl:Class ;
    rdfs:label "SPECIAL PURPOSE" .

<http://ncicb.nci.nih.gov/xml/odm/EVS/CDISCExtCodeID:C103378> a odm:ItemGroupClass,
        owl:Class ;
    rdfs:label "SUBJECT LEVEL ANALYSIS DATASET" .

<http://ncicb.nci.nih.gov/xml/odm/EVS/CDISCExtCodeID:C103379> a odm:ItemGroupClass,
        owl:Class ;
    rdfs:label "TRIAL DESIGN" .

<http://ncicb.nci.nih.gov/xml/odm/EVS/CDISCExtCodeID:C123454> a odm:ItemGroupClass,
        owl:Class ;
    rdfs:label "OCCURRENCE DATA STRUCTURE" .

<http://ncicb.nci.nih.gov/xml/odm/EVS/CDISCExtCodeID:C126101> a odm:OriginType,
        owl:Class ;
    rdfs:label "Not Available" .

<http://ncicb.nci.nih.gov/xml/odm/EVS/CDISCExtCodeID:C134003> a odm:DictionaryNameTypeEnum,
        owl:Class ;
    rdfs:label "D-U-N-S NUMBER" .

<http://ncicb.nci.nih.gov/xml/odm/EVS/CDISCExtCodeID:C135396> a odm:ItemGroupClass,
        owl:Class ;
    rdfs:label "FINDINGS ABOUT" .

<http://ncicb.nci.nih.gov/xml/odm/EVS/CDISCExtCodeID:C147271> a odm:ItemGroupClass,
        owl:Class ;
    rdfs:label "STUDY REFERENCE" .

<http://ncicb.nci.nih.gov/xml/odm/EVS/CDISCExtCodeID:C154331> a odm:DictionaryNameTypeEnum,
        owl:Class ;
    rdfs:label "WHO ATC CLASSIFICATION SYSTEM" .

<http://ncicb.nci.nih.gov/xml/odm/EVS/CDISCExtCodeID:C15600> a odm:TrialPhaseTypeEnum,
        owl:Class ;
    rdfs:label "PHASE I TRIAL" .

<http://ncicb.nci.nih.gov/xml/odm/EVS/CDISCExtCodeID:C15601> a odm:TrialPhaseTypeEnum,
        owl:Class ;
    rdfs:label "PHASE II TRIAL" .

<http://ncicb.nci.nih.gov/xml/odm/EVS/CDISCExtCodeID:C15602> a odm:TrialPhaseTypeEnum,
        owl:Class ;
    rdfs:label "PHASE III TRIAL" .

<http://ncicb.nci.nih.gov/xml/odm/EVS/CDISCExtCodeID:C15603> a odm:TrialPhaseTypeEnum,
        owl:Class ;
    rdfs:label "PHASE IV TRIAL" .

<http://ncicb.nci.nih.gov/xml/odm/EVS/CDISCExtCodeID:C15693> a odm:TrialPhaseTypeEnum,
        owl:Class ;
    rdfs:label "PHASE I/II TRIAL" .

<http://ncicb.nci.nih.gov/xml/odm/EVS/CDISCExtCodeID:C15694> a odm:TrialPhaseTypeEnum,
        owl:Class ;
    rdfs:label "PHASE II/III TRIAL" .

<http://ncicb.nci.nih.gov/xml/odm/EVS/CDISCExtCodeID:C163416> a odm:DictionaryNameTypeEnum,
        owl:Class ;
    rdfs:label "MED-RT" .

<http://ncicb.nci.nih.gov/xml/odm/EVS/CDISCExtCodeID:C163417> a odm:DictionaryNameTypeEnum,
        owl:Class ;
    rdfs:label "UNII" .

<http://ncicb.nci.nih.gov/xml/odm/EVS/CDISCExtCodeID:C165637> a odm:ItemGroupSubClass,
        owl:Class ;
    rdfs:label "TIME-TO-EVENT" .

<http://ncicb.nci.nih.gov/xml/odm/EVS/CDISCExtCodeID:C170454> a odm:StandardType,
        owl:Class ;
    rdfs:label "IG" .

<http://ncicb.nci.nih.gov/xml/odm/EVS/CDISCExtCodeID:C170455> a odm:StandardName,
        owl:Class ;
    rdfs:label "SDTMIG" .

<http://ncicb.nci.nih.gov/xml/odm/EVS/CDISCExtCodeID:C170456> a odm:StandardName,
        owl:Class ;
    rdfs:label "SENDIG" .

<http://ncicb.nci.nih.gov/xml/odm/EVS/CDISCExtCodeID:C170547> a odm:OriginType,
        owl:Class ;
    rdfs:label "Assigned" .

<http://ncicb.nci.nih.gov/xml/odm/EVS/CDISCExtCodeID:C170548> a odm:OriginType,
        owl:Class ;
    rdfs:label "Collected" .

<http://ncicb.nci.nih.gov/xml/odm/EVS/CDISCExtCodeID:C170549> a odm:OriginType,
        owl:Class ;
    rdfs:label "Derived" .

<http://ncicb.nci.nih.gov/xml/odm/EVS/CDISCExtCodeID:C170550> a odm:OriginType,
        owl:Class ;
    rdfs:label "Predecessor" .

<http://ncicb.nci.nih.gov/xml/odm/EVS/CDISCExtCodeID:C170551> a odm:OriginType,
        owl:Class ;
    rdfs:label "Protocol" .

<http://ncicb.nci.nih.gov/xml/odm/EVS/CDISCExtCodeID:C170552> a odm:StandardName,
        owl:Class ;
    rdfs:label "ADaMIG" .

<http://ncicb.nci.nih.gov/xml/odm/EVS/CDISCExtCodeID:C170553> a odm:StandardName,
        owl:Class ;
    rdfs:label "SDTMIG-AP" .

<http://ncicb.nci.nih.gov/xml/odm/EVS/CDISCExtCodeID:C170554> a odm:StandardName,
        owl:Class ;
    rdfs:label "SDTMIG-MD" .

<http://ncicb.nci.nih.gov/xml/odm/EVS/CDISCExtCodeID:C170556> a odm:StandardName,
        owl:Class ;
    rdfs:label "SENDIG-DART" .

<http://ncicb.nci.nih.gov/xml/odm/EVS/CDISCExtCodeID:C172452> a odm:ItemGroupSubClass,
        owl:Class ;
    rdfs:label "NON-COMPARTMENTAL ANALYSIS" .

<http://ncicb.nci.nih.gov/xml/odm/EVS/CDISCExtCodeID:C172453> a odm:StandardStatusEnum,
        owl:Class ;
    rdfs:label "Draft" .

<http://ncicb.nci.nih.gov/xml/odm/EVS/CDISCExtCodeID:C172454> a odm:StandardStatusEnum,
        owl:Class ;
    rdfs:label "Provisional" .

<http://ncicb.nci.nih.gov/xml/odm/EVS/CDISCExtCodeID:C172455> a odm:StandardStatusEnum,
        owl:Class ;
    rdfs:label "Final" .

<http://ncicb.nci.nih.gov/xml/odm/EVS/CDISCExtCodeID:C176265> a odm:ItemGroupSubClass,
        owl:Class ;
    rdfs:label "ADVERSE EVENT" .

<http://ncicb.nci.nih.gov/xml/odm/EVS/CDISCExtCodeID:C17649> a odm:OriginType,
        owl:Class ;
    rdfs:label "Other" .

<http://ncicb.nci.nih.gov/xml/odm/EVS/CDISCExtCodeID:C177920> a odm:ItemGroupSubClass,
        owl:Class ;
    rdfs:label "MEDICAL DEVICE TIME-TO-EVENT" .

<http://ncicb.nci.nih.gov/xml/odm/EVS/CDISCExtCodeID:C177921> a odm:ItemGroupClass,
        owl:Class ;
    rdfs:label "DEVICE LEVEL ANALYSIS DATASET" .

<http://ncicb.nci.nih.gov/xml/odm/EVS/CDISCExtCodeID:C177922> a odm:ItemGroupClass,
        owl:Class ;
    rdfs:label "MEDICAL DEVICE BASIC DATA STRUCTURE" .

<http://ncicb.nci.nih.gov/xml/odm/EVS/CDISCExtCodeID:C177923> a odm:ItemGroupClass,
        owl:Class ;
    rdfs:label "MEDICAL DEVICE OCCURRENCE DATA STRUCTURE" .

<http://ncicb.nci.nih.gov/xml/odm/EVS/CDISCExtCodeID:C180548> a odm:StandardPublishingSet,
        owl:Class ;
    rdfs:label "ADaM" .

<http://ncicb.nci.nih.gov/xml/odm/EVS/CDISCExtCodeID:C180549> a odm:StandardPublishingSet,
        owl:Class ;
    rdfs:label "CDASH" .

<http://ncicb.nci.nih.gov/xml/odm/EVS/CDISCExtCodeID:C180550> a odm:StandardPublishingSet,
        owl:Class ;
    rdfs:label "DEFINE-XML" .

<http://ncicb.nci.nih.gov/xml/odm/EVS/CDISCExtCodeID:C180551> a odm:StandardPublishingSet,
        owl:Class ;
    rdfs:label "SDTM" .

<http://ncicb.nci.nih.gov/xml/odm/EVS/CDISCExtCodeID:C180552> a odm:StandardPublishingSet,
        owl:Class ;
    rdfs:label "SEND" .

<http://ncicb.nci.nih.gov/xml/odm/EVS/CDISCExtCodeID:C181230> a odm:StandardName,
        owl:Class ;
    rdfs:label "SENDIG-AR" .

<http://ncicb.nci.nih.gov/xml/odm/EVS/CDISCExtCodeID:C25936> a odm:OriginSource,
        owl:Class ;
    rdfs:label "Investigator" .

<http://ncicb.nci.nih.gov/xml/odm/EVS/CDISCExtCodeID:C41189> a odm:OriginSource,
        owl:Class ;
    rdfs:label "Subject" .

<http://ncicb.nci.nih.gov/xml/odm/EVS/CDISCExtCodeID:C43820> a odm:DictionaryNameTypeEnum,
        owl:Class ;
    rdfs:label "MedDRA" .

<http://ncicb.nci.nih.gov/xml/odm/EVS/CDISCExtCodeID:C47865> a odm:TrialPhaseTypeEnum,
        owl:Class ;
    rdfs:label "PHASE V TRIAL" .

<http://ncicb.nci.nih.gov/xml/odm/EVS/CDISCExtCodeID:C48660> a odm:TrialPhaseTypeEnum,
        owl:Class ;
    rdfs:label "NOT APPLICABLE" .

<http://ncicb.nci.nih.gov/xml/odm/EVS/CDISCExtCodeID:C49468> a odm:DictionaryNameTypeEnum,
        owl:Class ;
    rdfs:label "WHOART" .

<http://ncicb.nci.nih.gov/xml/odm/EVS/CDISCExtCodeID:C49471> a odm:DictionaryNameTypeEnum,
        owl:Class ;
    rdfs:label "COSTART" .

<http://ncicb.nci.nih.gov/xml/odm/EVS/CDISCExtCodeID:C49474> a odm:DictionaryNameTypeEnum,
        owl:Class ;
    rdfs:label "ICD" .

<http://ncicb.nci.nih.gov/xml/odm/EVS/CDISCExtCodeID:C49475> a odm:DictionaryNameTypeEnum,
        owl:Class ;
    rdfs:label "WHODD" .

<http://ncicb.nci.nih.gov/xml/odm/EVS/CDISCExtCodeID:C49476> a odm:DictionaryNameTypeEnum,
        owl:Class ;
    rdfs:label "LOINC" .

<http://ncicb.nci.nih.gov/xml/odm/EVS/CDISCExtCodeID:C49686> a odm:TrialPhaseTypeEnum,
        owl:Class ;
    rdfs:label "PHASE IIA TRIAL" .

<http://ncicb.nci.nih.gov/xml/odm/EVS/CDISCExtCodeID:C49687> a odm:TrialPhaseTypeEnum,
        owl:Class ;
    rdfs:label "PHASE IIIA TRIAL" .

<http://ncicb.nci.nih.gov/xml/odm/EVS/CDISCExtCodeID:C49688> a odm:TrialPhaseTypeEnum,
        owl:Class ;
    rdfs:label "PHASE IIB TRIAL" .

<http://ncicb.nci.nih.gov/xml/odm/EVS/CDISCExtCodeID:C49689> a odm:TrialPhaseTypeEnum,
        owl:Class ;
    rdfs:label "PHASE IIIB TRIAL" .

<http://ncicb.nci.nih.gov/xml/odm/EVS/CDISCExtCodeID:C49704> a odm:DictionaryNameTypeEnum,
        owl:Class ;
    rdfs:label "CTCAE" .

<http://ncicb.nci.nih.gov/xml/odm/EVS/CDISCExtCodeID:C53489> a odm:DictionaryNameTypeEnum,
        owl:Class ;
    rdfs:label "SNOMED" .

<http://ncicb.nci.nih.gov/xml/odm/EVS/CDISCExtCodeID:C54721> a odm:TrialPhaseTypeEnum,
        owl:Class ;
    rdfs:label "PHASE 0 TRIAL" .

<http://ncicb.nci.nih.gov/xml/odm/EVS/CDISCExtCodeID:C68608> a odm:OriginSource,
        owl:Class ;
    rdfs:label "Vendor" .

<http://ncicb.nci.nih.gov/xml/odm/EVS/CDISCExtCodeID:C70793> a odm:OriginSource,
        owl:Class ;
    rdfs:label "Sponsor" .

<http://www.cdisc.org/ns/odm/v2.0/BranchingType#Exclusive> a odm:BranchingType,
        owl:Class ;
    rdfs:label "Exclusive" .

<http://www.cdisc.org/ns/odm/v2.0/BranchingType#Parallel> a odm:BranchingType,
        owl:Class ;
    rdfs:label "Parallel" .

<http://www.cdisc.org/ns/odm/v2.0/CLDataType#decimal> a odm:CLDataType,
        owl:Class ;
    rdfs:label "decimal" .

<http://www.cdisc.org/ns/odm/v2.0/CLDataType#integer> a odm:CLDataType,
        owl:Class ;
    rdfs:label "integer" .

<http://www.cdisc.org/ns/odm/v2.0/CLDataType#string> a odm:CLDataType,
        owl:Class ;
    rdfs:label "string" .

<http://www.cdisc.org/ns/odm/v2.0/CLDataType#text> a odm:CLDataType,
        owl:Class ;
    rdfs:label "text" .

odm:CodeListRefRef a owl:ObjectProperty,
        linkml:SlotDefinition ;
    rdfs:label "CodeListRefRef" ;
    rdfs:range odm:CodeListRef ;
    skos:definition "CodeListRef reference: A reference to a CodeList definition." .

odm:CodeRef a owl:ObjectProperty,
        linkml:SlotDefinition ;
    rdfs:label "CodeRef" ;
    rdfs:range odm:Code ;
    skos:definition "A string pattern that identifies a concept as defined by the code system." .

<http://www.cdisc.org/ns/odm/v2.0/CommentType#Site> a odm:CommentType,
        owl:Class ;
    rdfs:label "Site" .

<http://www.cdisc.org/ns/odm/v2.0/CommentType#Sponsor> a odm:CommentType,
        owl:Class ;
    rdfs:label "Sponsor" .

<http://www.cdisc.org/ns/odm/v2.0/Comparator#EQ> a odm:Comparator,
        owl:Class ;
    rdfs:label "EQ" .

<http://www.cdisc.org/ns/odm/v2.0/Comparator#GE> a odm:Comparator,
        owl:Class ;
    rdfs:label "GE" .

<http://www.cdisc.org/ns/odm/v2.0/Comparator#GT> a odm:Comparator,
        owl:Class ;
    rdfs:label "GT" .

<http://www.cdisc.org/ns/odm/v2.0/Comparator#IN> a odm:Comparator,
        owl:Class ;
    rdfs:label "IN" .

<http://www.cdisc.org/ns/odm/v2.0/Comparator#LE> a odm:Comparator,
        owl:Class ;
    rdfs:label "LE" .

<http://www.cdisc.org/ns/odm/v2.0/Comparator#LT> a odm:Comparator,
        owl:Class ;
    rdfs:label "LT" .

<http://www.cdisc.org/ns/odm/v2.0/Comparator#NE> a odm:Comparator,
        owl:Class ;
    rdfs:label "NE" .

<http://www.cdisc.org/ns/odm/v2.0/Comparator#NOTIN> a odm:Comparator,
        owl:Class ;
    rdfs:label "NOTIN" .

<http://www.cdisc.org/ns/odm/v2.0/Context#Archive> a odm:Context,
        owl:Class ;
    rdfs:label "Archive" .

<http://www.cdisc.org/ns/odm/v2.0/Context#Exchange> a odm:Context,
        owl:Class ;
    rdfs:label "Exchange" .

<http://www.cdisc.org/ns/odm/v2.0/Context#Submission> a odm:Context,
        owl:Class ;
    rdfs:label "Submission" .

<http://www.cdisc.org/ns/odm/v2.0/DataType#URI> a odm:DataType,
        owl:Class ;
    rdfs:label "URI" .

<http://www.cdisc.org/ns/odm/v2.0/DataType#base64Binary> a odm:DataType,
        owl:Class ;
    rdfs:label "base64Binary" .

<http://www.cdisc.org/ns/odm/v2.0/DataType#base64Float> a odm:DataType,
        owl:Class ;
    rdfs:label "base64Float" .

<http://www.cdisc.org/ns/odm/v2.0/DataType#boolean> a odm:DataType,
        owl:Class ;
    rdfs:label "boolean" .

<http://www.cdisc.org/ns/odm/v2.0/DataType#date> a odm:DataType,
        owl:Class ;
    rdfs:label "date" .

<http://www.cdisc.org/ns/odm/v2.0/DataType#datetime> a odm:DataType,
        owl:Class ;
    rdfs:label "datetime" .

<http://www.cdisc.org/ns/odm/v2.0/DataType#decimal> a odm:DataType,
        owl:Class ;
    rdfs:label "decimal" .

<http://www.cdisc.org/ns/odm/v2.0/DataType#double> a odm:DataType,
        owl:Class ;
    rdfs:label "double" .

<http://www.cdisc.org/ns/odm/v2.0/DataType#durationDatetime> a odm:DataType,
        owl:Class ;
    rdfs:label "durationDatetime" .

<http://www.cdisc.org/ns/odm/v2.0/DataType#float> a odm:DataType,
        owl:Class ;
    rdfs:label "float" .

<http://www.cdisc.org/ns/odm/v2.0/DataType#hexBinary> a odm:DataType,
        owl:Class ;
    rdfs:label "hexBinary" .

<http://www.cdisc.org/ns/odm/v2.0/DataType#hexFloat> a odm:DataType,
        owl:Class ;
    rdfs:label "hexFloat" .

<http://www.cdisc.org/ns/odm/v2.0/DataType#incompleteDate> a odm:DataType,
        owl:Class ;
    rdfs:label "incompleteDate" .

<http://www.cdisc.org/ns/odm/v2.0/DataType#incompleteDatetime> a odm:DataType,
        owl:Class ;
    rdfs:label "incompleteDatetime" .

<http://www.cdisc.org/ns/odm/v2.0/DataType#incompleteTime> a odm:DataType,
        owl:Class ;
    rdfs:label "incompleteTime" .

<http://www.cdisc.org/ns/odm/v2.0/DataType#integer> a odm:DataType,
        owl:Class ;
    rdfs:label "integer" .

<http://www.cdisc.org/ns/odm/v2.0/DataType#intervalDatetime> a odm:DataType,
        owl:Class ;
    rdfs:label "intervalDatetime" .

<http://www.cdisc.org/ns/odm/v2.0/DataType#partialDate> a odm:DataType,
        owl:Class ;
    rdfs:label "partialDate" .

<http://www.cdisc.org/ns/odm/v2.0/DataType#partialDatetime> a odm:DataType,
        owl:Class ;
    rdfs:label "partialDatetime" .

<http://www.cdisc.org/ns/odm/v2.0/DataType#partialTime> a odm:DataType,
        owl:Class ;
    rdfs:label "partialTime" .

<http://www.cdisc.org/ns/odm/v2.0/DataType#string> a odm:DataType,
        owl:Class ;
    rdfs:label "string" .

<http://www.cdisc.org/ns/odm/v2.0/DataType#text> a odm:DataType,
        owl:Class ;
    rdfs:label "text" .

<http://www.cdisc.org/ns/odm/v2.0/DataType#time> a odm:DataType,
        owl:Class ;
    rdfs:label "time" .

odm:Date a owl:Class,
        linkml:TypeDefinition ;
    rdfs:label "date" ;
    rdfs:subClassOf [ a owl:Restriction ;
            owl:onDataRange xsd:date ;
            owl:onProperty linkml:topValue ;
            owl:qualifiedCardinality 1 ] .

odm:DateTimeStampRef a owl:ObjectProperty,
        linkml:SlotDefinition ;
    rdfs:label "DateTimeStampRef" ;
    rdfs:range odm:DateTimeStamp ;
    skos:definition "DateTimeStamp reference: None" .

<http://www.cdisc.org/ns/odm/v2.0/DefCoreType#Cond> a odm:DefCoreType,
        owl:Class ;
    rdfs:label "Cond" .

<http://www.cdisc.org/ns/odm/v2.0/DefCoreType#Exp> a odm:DefCoreType,
        owl:Class ;
    rdfs:label "Exp" .

<http://www.cdisc.org/ns/odm/v2.0/DefCoreType#Perm> a odm:DefCoreType,
        owl:Class ;
    rdfs:label "Perm" .

<http://www.cdisc.org/ns/odm/v2.0/DefCoreType#Req> a odm:DefCoreType,
        owl:Class ;
    rdfs:label "Req" .

odm:DictionaryNameType a owl:Class,
        linkml:TypeDefinition ;
    rdfs:label "DictionaryNameType" ;
    rdfs:subClassOf [ a owl:Restriction ;
            owl:onDataRange odm:DictionaryNameType ;
            owl:onProperty linkml:topValue ;
            owl:qualifiedCardinality 1 ] .

<http://www.cdisc.org/ns/odm/v2.0/EditPointType#DBAudit> a odm:EditPointType,
        owl:Class ;
    rdfs:label "DBAudit" .

<http://www.cdisc.org/ns/odm/v2.0/EditPointType#DataManagement> a odm:EditPointType,
        owl:Class ;
    rdfs:label "DataManagement" .

<http://www.cdisc.org/ns/odm/v2.0/EditPointType#Monitoring> a odm:EditPointType,
        owl:Class ;
    rdfs:label "Monitoring" .

odm:EntryCriteria a owl:Class,
        linkml:ClassDefinition ;
    rdfs:label "EntryCriteria" ;
    rdfs:subClassOf [ a owl:Restriction ;
            owl:allValuesFrom odm:Criterion ;
            owl:onProperty odm:CriterionRef ] ;
    skos:exactMatch odm:EntryCriteria .

<http://www.cdisc.org/ns/odm/v2.0/EventType#Common> a odm:EventType,
        owl:Class ;
    rdfs:label "Common" .

<http://www.cdisc.org/ns/odm/v2.0/EventType#Scheduled> a odm:EventType,
        owl:Class ;
    rdfs:label "Scheduled" .

<http://www.cdisc.org/ns/odm/v2.0/EventType#Unscheduled> a odm:EventType,
        owl:Class ;
    rdfs:label "Unscheduled" .

odm:ExceptionEvent a owl:Class,
        linkml:ClassDefinition ;
    rdfs:label "ExceptionEvent" ;
    rdfs:subClassOf [ a owl:Restriction ;
            owl:onClass odm:Name ;
            owl:onProperty odm:Name ;
            owl:qualifiedCardinality 1 ],
        [ a owl:Restriction ;
            owl:onClass odm:WorkflowRef ;
            owl:onProperty odm:WorkflowRefRef ;
            owl:qualifiedCardinality 1 ],
        [ a owl:Restriction ;
            owl:maxQualifiedCardinality 1 ;
            owl:onClass odm:Oidref ;
            owl:onProperty odm:ConditionOID ],
        [ a owl:Restriction ;
            owl:maxQualifiedCardinality 1 ;
            owl:onClass odm:Description ;
            owl:onProperty odm:DescriptionRef ],
        [ a owl:Restriction ;
            owl:onClass odm:Oid ;
            owl:onProperty odm:OID ;
            owl:qualifiedCardinality 1 ],
        [ a owl:Restriction ;
            owl:onClass odm:StudyEventRef ;
            owl:onProperty odm:StudyEventRefRef ;
            owl:qualifiedCardinality 1 ],
        [ a owl:Restriction ;
            owl:onClass odm:StudyEventGroupRef ;
            owl:onProperty odm:StudyEventGroupRefRef ;
            owl:qualifiedCardinality 1 ] ;
    skos:definition "An ExceptionEvent describes an event that occurs suddenly in a study and that was not planned as part of the normal workflow of the study. Examples are adverse events, death of a subject not caused by an adverse event, etc." ;
    skos:exactMatch odm:ExceptionEvent .

odm:ExitCriteria a owl:Class,
        linkml:ClassDefinition ;
    rdfs:label "ExitCriteria" ;
    rdfs:subClassOf [ a owl:Restriction ;
            owl:allValuesFrom odm:Criterion ;
            owl:onProperty odm:CriterionRef ] ;
    skos:exactMatch odm:ExitCriteria .

odm:FileName a owl:Class,
        linkml:TypeDefinition ;
    rdfs:label "fileName" ;
    rdfs:subClassOf [ a owl:Restriction ;
            owl:onDataRange odm:fileName ;
            owl:onProperty linkml:topValue ;
            owl:qualifiedCardinality 1 ] .

<http://www.cdisc.org/ns/odm/v2.0/FileType#Snapshot> a odm:FileType,
        owl:Class ;
    rdfs:label "Snapshot" .

<http://www.cdisc.org/ns/odm/v2.0/FileType#Transactional> a odm:FileType,
        owl:Class ;
    rdfs:label "Transactional" .

<http://www.cdisc.org/ns/odm/v2.0/Granularity#AdminData> a odm:Granularity,
        owl:Class ;
    rdfs:label "AdminData" .

<http://www.cdisc.org/ns/odm/v2.0/Granularity#All> a odm:Granularity,
        owl:Class ;
    rdfs:label "All" .

<http://www.cdisc.org/ns/odm/v2.0/Granularity#AllClinicalData> a odm:Granularity,
        owl:Class ;
    rdfs:label "AllClinicalData" .

<http://www.cdisc.org/ns/odm/v2.0/Granularity#Metadata> a odm:Granularity,
        owl:Class ;
    rdfs:label "Metadata" .

<http://www.cdisc.org/ns/odm/v2.0/Granularity#ReferenceData> a odm:Granularity,
        owl:Class ;
    rdfs:label "ReferenceData" .

<http://www.cdisc.org/ns/odm/v2.0/Granularity#SingleSite> a odm:Granularity,
        owl:Class ;
    rdfs:label "SingleSite" .

<http://www.cdisc.org/ns/odm/v2.0/Granularity#SingleSubject> a odm:Granularity,
        owl:Class ;
    rdfs:label "SingleSubject" .

odm:HasNoData a owl:ObjectProperty,
        linkml:SlotDefinition ;
    rdfs:label "HasNoData" ;
    rdfs:range odm:YesOnly ;
    skos:definition "Used to indicate that an ItemGroupDef has no data. May be used at sponsor's discretion or if required by a regulatory authority" .

odm:ItemGroupRefRef a owl:ObjectProperty,
        linkml:SlotDefinition ;
    rdfs:label "ItemGroupRefRef" ;
    rdfs:range odm:ItemGroupRef ;
    skos:definition "ItemGroupRef reference: ItemGroupRef references an ItemGroupDef as it occurs within a specific StudyEventDef or ItemGroupDef. The list of ItemGroupRefs identifies the types of item groups that are allowed to occur within this type of studyevent or (nested) item group. The ItemGroupRefs within a single StudyEventDef or ItemGroupDef must not have duplicate ItemGroupOID or OrderNumber attribute values." .

odm:ItemGroupRepeatKey a owl:ObjectProperty,
        linkml:SlotDefinition ;
    rdfs:label "ItemGroupRepeatKey" ;
    rdfs:range odm:RepeatKey ;
    skos:definition "A key used to distinguish between repeats of the same type of item group." .

<http://www.cdisc.org/ns/odm/v2.0/ItemGroupRepeatingType#Dynamic> a odm:ItemGroupRepeatingType,
        owl:Class ;
    rdfs:label "Dynamic" .

<http://www.cdisc.org/ns/odm/v2.0/ItemGroupRepeatingType#No> a odm:ItemGroupRepeatingType,
        owl:Class ;
    rdfs:label "No" .

<http://www.cdisc.org/ns/odm/v2.0/ItemGroupRepeatingType#Simple> a odm:ItemGroupRepeatingType,
        owl:Class ;
    rdfs:label "Simple" .

<http://www.cdisc.org/ns/odm/v2.0/ItemGroupRepeatingType#Static> a odm:ItemGroupRepeatingType,
        owl:Class ;
    rdfs:label "Static" .

odm:ItemGroupTypeType a owl:Class,
        linkml:TypeDefinition ;
    rdfs:label "ItemGroupTypeType" ;
    rdfs:subClassOf [ a owl:Restriction ;
            owl:onDataRange odm:ItemGroupTypeType ;
            owl:onProperty linkml:topValue ;
            owl:qualifiedCardinality 1 ] .

odm:ItemRefRef a owl:ObjectProperty,
        linkml:SlotDefinition ;
    rdfs:label "ItemRefRef" ;
    rdfs:range odm:ItemRef ;
    skos:definition "ItemRef reference: A reference to an ItemDef as it occurs within a specific ItemGroupDef. The list of ItemRefs identifies the types of items that are allowed to occur within this type of item group." .

odm:Label a owl:ObjectProperty,
        linkml:SlotDefinition ;
    rdfs:label "Label" ;
    rdfs:range odm:Text ;
    skos:definition "Used to link the value to a named MethodDef parameter." .

odm:LanguageType a owl:Class,
        linkml:TypeDefinition ;
    rdfs:label "_languageType" ;
    rdfs:subClassOf [ a owl:Restriction ;
            owl:onDataRange xml1:lang ;
            owl:onProperty linkml:topValue ;
            owl:qualifiedCardinality 1 ] .

odm:LeafRef a owl:ObjectProperty,
        linkml:SlotDefinition ;
    rdfs:label "LeafRef" ;
    rdfs:range odm:Leaf ;
    skos:definition "Leaf reference: Contains the XLink information referenced by DocumentRef or ArchiveLocationID" .

odm:MetaDataVersionRefRef a owl:ObjectProperty,
        linkml:SlotDefinition ;
    rdfs:label "MetaDataVersionRefRef" ;
    rdfs:range odm:MetaDataVersionRef ;
    skos:definition "MetaDataVersionRef reference: A reference to a MetaDataVersion used at the containing Location. The EffectiveDate reflects the possibility that the metadata may change over the course of the study." .

<http://www.cdisc.org/ns/odm/v2.0/MethodType#Computation> a odm:MethodType,
        owl:Class ;
    rdfs:label "Computation" .

<http://www.cdisc.org/ns/odm/v2.0/MethodType#Imputation> a odm:MethodType,
        owl:Class ;
    rdfs:label "Imputation" .

<http://www.cdisc.org/ns/odm/v2.0/MethodType#Preload> a odm:MethodType,
        owl:Class ;
    rdfs:label "Preload" .

<http://www.cdisc.org/ns/odm/v2.0/MethodType#Transpose> a odm:MethodType,
        owl:Class ;
    rdfs:label "Transpose" .

<http://www.cdisc.org/ns/odm/v2.0/ODMCoreType#HR> a odm:ODMCoreType,
        owl:Class ;
    rdfs:label "HR" .

<http://www.cdisc.org/ns/odm/v2.0/ODMCoreType#O> a odm:ODMCoreType,
        owl:Class ;
    rdfs:label "O" .

<http://www.cdisc.org/ns/odm/v2.0/ODMCoreType#R/C> a odm:ODMCoreType,
        owl:Class ;
    rdfs:label "R/C" .

odm:OrganizationOID a owl:ObjectProperty,
        linkml:SlotDefinition ;
    rdfs:label "OrganizationOID" ;
    rdfs:range odm:Oidref ;
    skos:definition "Reference to an Organization elment." .

<http://www.cdisc.org/ns/odm/v2.0/OrganizationType#CRO> a odm:OrganizationType,
        owl:Class ;
    rdfs:label "CRO" .

<http://www.cdisc.org/ns/odm/v2.0/OrganizationType#Lab> a odm:OrganizationType,
        owl:Class ;
    rdfs:label "Lab" .

<http://www.cdisc.org/ns/odm/v2.0/OrganizationType#Other> a odm:OrganizationType,
        owl:Class ;
    rdfs:label "Other" .

<http://www.cdisc.org/ns/odm/v2.0/OrganizationType#Site> a odm:OrganizationType,
        owl:Class ;
    rdfs:label "Site" .

<http://www.cdisc.org/ns/odm/v2.0/OrganizationType#Sponsor> a odm:OrganizationType,
        owl:Class ;
    rdfs:label "Sponsor" .

<http://www.cdisc.org/ns/odm/v2.0/OrganizationType#TechnologyProvider> a odm:OrganizationType,
        owl:Class ;
    rdfs:label "TechnologyProvider" .

odm:OriginRef a owl:ObjectProperty,
        linkml:SlotDefinition ;
    rdfs:label "OriginRef" ;
    rdfs:range odm:Origin ;
    skos:definition "Origin reference: Origin defines the source metadata, where applicable, for ODM ItemRefs or ItemGroupRefs. Origin as a child element replaces the Origin attribute in ODM v1.3 that exists for the ItemDef and ItemGroupDef elements.The Origin element is based on the def:Origin element in Define-XML v2.1 with the Trace-XML v1.0 extension." .

<http://www.cdisc.org/ns/odm/v2.0/OriginType#EHR> a odm:OriginType,
        owl:Class ;
    rdfs:label "EHR" .

odm:Other a owl:ObjectProperty,
        linkml:SlotDefinition ;
    rdfs:label "Other" ;
    rdfs:range odm:YesOnly ;
    skos:definition "Flag to indicate that the Item represents \"other\" content added to an ItemGroup." .

<http://www.cdisc.org/ns/odm/v2.0/PDFPageType#NamedDestination> a odm:PDFPageType,
        owl:Class ;
    rdfs:label "NamedDestination" .

<http://www.cdisc.org/ns/odm/v2.0/PDFPageType#PhysicalRef> a odm:PDFPageType,
        owl:Class ;
    rdfs:label "PhysicalRef" .

<http://www.cdisc.org/ns/odm/v2.0/QuerySourceType#Coding+System> a odm:QuerySourceType,
        owl:Class ;
    rdfs:label "Coding System" .

<http://www.cdisc.org/ns/odm/v2.0/QuerySourceType#Data+Management> a odm:QuerySourceType,
        owl:Class ;
    rdfs:label "Data Management" .

<http://www.cdisc.org/ns/odm/v2.0/QuerySourceType#Safety+Reviewer> a odm:QuerySourceType,
        owl:Class ;
    rdfs:label "Safety Reviewer" .

<http://www.cdisc.org/ns/odm/v2.0/QuerySourceType#Site+Monitor> a odm:QuerySourceType,
        owl:Class ;
    rdfs:label "Site Monitor" .

<http://www.cdisc.org/ns/odm/v2.0/QuerySourceType#System> a odm:QuerySourceType,
        owl:Class ;
    rdfs:label "System" .

<http://www.cdisc.org/ns/odm/v2.0/QueryStateType#Answered> a odm:QueryStateType,
        owl:Class ;
    rdfs:label "Answered" .

<http://www.cdisc.org/ns/odm/v2.0/QueryStateType#Cancelled> a odm:QueryStateType,
        owl:Class ;
    rdfs:label "Cancelled" .

<http://www.cdisc.org/ns/odm/v2.0/QueryStateType#Candidate> a odm:QueryStateType,
        owl:Class ;
    rdfs:label "Candidate" .

<http://www.cdisc.org/ns/odm/v2.0/QueryStateType#Closed> a odm:QueryStateType,
        owl:Class ;
    rdfs:label "Closed" .

<http://www.cdisc.org/ns/odm/v2.0/QueryStateType#Open> a odm:QueryStateType,
        owl:Class ;
    rdfs:label "Open" .

<http://www.cdisc.org/ns/odm/v2.0/QueryStateType#Resolved> a odm:QueryStateType,
        owl:Class ;
    rdfs:label "Resolved" .

<http://www.cdisc.org/ns/odm/v2.0/QueryType#Manual> a odm:QueryType,
        owl:Class ;
    rdfs:label "Manual" .

<http://www.cdisc.org/ns/odm/v2.0/QueryType#System> a odm:QueryType,
        owl:Class ;
    rdfs:label "System" .

odm:RangeCheckRef a owl:ObjectProperty,
        linkml:SlotDefinition ;
    rdfs:label "RangeCheckRef" ;
    rdfs:range odm:RangeCheck ;
    skos:definition "RangeCheck reference: A RangeCheck defines a constraint on the value of the enclosing item. It represents an expression that evaluates to True when the ItemData value is valid or False when the ItemData value is invalid. The expression is specified using either Comparator and CheckValue or using FormalExpressions." .

<http://www.cdisc.org/ns/odm/v2.0/RelativeTimingConstraintType#FinishToFinish> a odm:RelativeTimingConstraintType,
        owl:Class ;
    rdfs:label "FinishToFinish" .

<http://www.cdisc.org/ns/odm/v2.0/RelativeTimingConstraintType#FinishToStart> a odm:RelativeTimingConstraintType,
        owl:Class ;
    rdfs:label "FinishToStart" .

<http://www.cdisc.org/ns/odm/v2.0/RelativeTimingConstraintType#StartToFinish> a odm:RelativeTimingConstraintType,
        owl:Class ;
    rdfs:label "StartToFinish" .

<http://www.cdisc.org/ns/odm/v2.0/RelativeTimingConstraintType#StartToStart> a odm:RelativeTimingConstraintType,
        owl:Class ;
    rdfs:label "StartToStart" .

odm:Repeating a owl:ObjectProperty,
        linkml:SlotDefinition ;
    rdfs:label "Repeating" ;
    rdfs:range odm:String ;
    skos:definition "The Repeating flag indicates when this type of study event can occur repeatedly within any given subject. When Repeating is \"Yes\" multiple instances of StudyEventData for this StudyEventDef may be collected for a study subject." .

odm:SeqNum a owl:ObjectProperty,
        linkml:SlotDefinition ;
    rdfs:label "SeqNum" ;
    rdfs:range odm:PositiveInteger ;
    skos:definition "When more than 1 Value element exists this attribute uniquely identifies each Value and defines the order of a Value in a list of Values." .

<http://www.cdisc.org/ns/odm/v2.0/SignMethod#Digital> a odm:SignMethod,
        owl:Class ;
    rdfs:label "Digital" .

<http://www.cdisc.org/ns/odm/v2.0/SignMethod#Electronic> a odm:SignMethod,
        owl:Class ;
    rdfs:label "Electronic" .

<http://www.cdisc.org/ns/odm/v2.0/SoftOrHard#Hard> a odm:SoftOrHard,
        owl:Class ;
    rdfs:label "Hard" .

<http://www.cdisc.org/ns/odm/v2.0/SoftOrHard#Soft> a odm:SoftOrHard,
        owl:Class ;
    rdfs:label "Soft" .

odm:Source a owl:ObjectProperty,
        linkml:SlotDefinition ;
    rdfs:label "Source" ;
    rdfs:range odm:String ;
    skos:definition "I ndicates the party responsible for the data's origin type." .

odm:StandardOID a owl:ObjectProperty,
        linkml:SlotDefinition ;
    rdfs:label "StandardOID" ;
    rdfs:range odm:Oidref ;
    skos:definition "Reference to a Standard element." .

odm:StandardStatus a owl:Class,
        linkml:TypeDefinition ;
    rdfs:label "StandardStatus" ;
    rdfs:subClassOf [ a owl:Restriction ;
            owl:onDataRange odm:StandardStatus ;
            owl:onProperty linkml:topValue ;
            owl:qualifiedCardinality 1 ] .

odm:Status a owl:ObjectProperty,
        linkml:SlotDefinition ;
    rdfs:label "Status" ;
    rdfs:range odm:String ;
    skos:definition "Status of Standard." .

<http://www.cdisc.org/ns/odm/v2.0/StudyEndPointType#Composite> a odm:StudyEndPointType,
        owl:Class ;
    rdfs:label "Composite" .

<http://www.cdisc.org/ns/odm/v2.0/StudyEndPointType#Humane> a odm:StudyEndPointType,
        owl:Class ;
    rdfs:label "Humane" .

<http://www.cdisc.org/ns/odm/v2.0/StudyEndPointType#Simple> a odm:StudyEndPointType,
        owl:Class ;
    rdfs:label "Simple" .

<http://www.cdisc.org/ns/odm/v2.0/StudyEndPointType#Surrogate> a odm:StudyEndPointType,
        owl:Class ;
    rdfs:label "Surrogate" .

<http://www.cdisc.org/ns/odm/v2.0/StudyEstimandLevel#Exploratory> a odm:StudyEstimandLevel,
        owl:Class ;
    rdfs:label "Exploratory" .

<http://www.cdisc.org/ns/odm/v2.0/StudyEstimandLevel#Primary> a odm:StudyEstimandLevel,
        owl:Class ;
    rdfs:label "Primary" .

<http://www.cdisc.org/ns/odm/v2.0/StudyEstimandLevel#Secondary> a odm:StudyEstimandLevel,
        owl:Class ;
    rdfs:label "Secondary" .

odm:StudyEventGroupOID a owl:ObjectProperty,
        linkml:SlotDefinition ;
    rdfs:label "StudyEventGroupOID" ;
    rdfs:range odm:Oidref ;
    skos:definition "Reference to the StudyEventGroupDef ." .

odm:StudyEventRefRef a owl:ObjectProperty,
        linkml:SlotDefinition ;
    rdfs:label "StudyEventRefRef" ;
    rdfs:range odm:StudyEventRef ;
    skos:definition "StudyEventRef reference: This element references a StudyEventDef as it occurs within a specific version of a study. The list of StudyEventRefs identifies the types of study events that are allowed to occur within the study." .

odm:StudyEventRepeatKey a owl:ObjectProperty,
        linkml:SlotDefinition ;
    rdfs:label "StudyEventRepeatKey" ;
    rdfs:range odm:RepeatKey ;
    skos:definition "A key used to distinguish between repeats of the same type of study event for a single subject." .

odm:StudyInterventionRefRef a owl:ObjectProperty,
        linkml:SlotDefinition ;
    rdfs:label "StudyInterventionRefRef" ;
    rdfs:range odm:StudyInterventionRef ;
    skos:definition "StudyInterventionRef reference: None" .

<http://www.cdisc.org/ns/odm/v2.0/StudyObjectiveLevel#Exploratory> a odm:StudyObjectiveLevel,
        owl:Class ;
    rdfs:label "Exploratory" .

<http://www.cdisc.org/ns/odm/v2.0/StudyObjectiveLevel#Primary> a odm:StudyObjectiveLevel,
        owl:Class ;
    rdfs:label "Primary" .

<http://www.cdisc.org/ns/odm/v2.0/StudyObjectiveLevel#Secondary> a odm:StudyObjectiveLevel,
        owl:Class ;
    rdfs:label "Secondary" .

odm:StudyTargetPopulationRefRef a owl:ObjectProperty,
        linkml:SlotDefinition ;
    rdfs:label "StudyTargetPopulationRefRef" ;
    rdfs:range odm:StudyTargetPopulationRef ;
    skos:definition "StudyTargetPopulationRef reference: None" .

odm:TargetTransitionOID a owl:ObjectProperty,
        linkml:SlotDefinition ;
    rdfs:label "TargetTransitionOID" ;
    rdfs:range odm:Oidref ;
    skos:definition "Reference to the Transition that is one of the targets of the branching." .

<http://www.cdisc.org/ns/odm/v2.0/TelecomTypeType#Email> a odm:TelecomTypeType,
        owl:Class ;
    rdfs:label "Email" .

<http://www.cdisc.org/ns/odm/v2.0/TelecomTypeType#Fax> a odm:TelecomTypeType,
        owl:Class ;
    rdfs:label "Fax" .

<http://www.cdisc.org/ns/odm/v2.0/TelecomTypeType#Other> a odm:TelecomTypeType,
        owl:Class ;
    rdfs:label "Other" .

<http://www.cdisc.org/ns/odm/v2.0/TelecomTypeType#Pager> a odm:TelecomTypeType,
        owl:Class ;
    rdfs:label "Pager" .

<http://www.cdisc.org/ns/odm/v2.0/TelecomTypeType#Phone> a odm:TelecomTypeType,
        owl:Class ;
    rdfs:label "Phone" .

<http://www.cdisc.org/ns/odm/v2.0/TelecomTypeType#SMS> a odm:TelecomTypeType,
        owl:Class ;
    rdfs:label "SMS" .

<http://www.cdisc.org/ns/odm/v2.0/TelecomTypeType#URL> a odm:TelecomTypeType,
        owl:Class ;
    rdfs:label "URL" .

odm:TimepointTarget a owl:ObjectProperty,
        linkml:SlotDefinition ;
    rdfs:label "TimepointTarget" ;
    rdfs:range odm:String ;
    skos:definition "The planned time between the 2 activities defined by the transition in the workflow." .

odm:Title a owl:ObjectProperty,
        linkml:SlotDefinition ;
    rdfs:label "Title" ;
    rdfs:range odm:Text ;
    skos:definition "Text with the label for the document reference." .

<http://www.cdisc.org/ns/odm/v2.0/TransactionType#Context> a odm:TransactionType,
        owl:Class ;
    rdfs:label "Context" .

<http://www.cdisc.org/ns/odm/v2.0/TransactionType#Insert> a odm:TransactionType,
        owl:Class ;
    rdfs:label "Insert" .

<http://www.cdisc.org/ns/odm/v2.0/TransactionType#Remove> a odm:TransactionType,
        owl:Class ;
    rdfs:label "Remove" .

<http://www.cdisc.org/ns/odm/v2.0/TransactionType#Update> a odm:TransactionType,
        owl:Class ;
    rdfs:label "Update" .

<http://www.cdisc.org/ns/odm/v2.0/TransactionType#Upsert> a odm:TransactionType,
        owl:Class ;
    rdfs:label "Upsert" .

odm:TrialPhaseType a owl:Class,
        linkml:TypeDefinition ;
    rdfs:label "TrialPhaseType" ;
    rdfs:subClassOf [ a owl:Restriction ;
            owl:onDataRange odm:TrialPhaseType ;
            owl:onProperty linkml:topValue ;
            owl:qualifiedCardinality 1 ] .

odm:UserOID a owl:ObjectProperty,
        linkml:SlotDefinition ;
    rdfs:label "UserOID" ;
    rdfs:range odm:Oidref ;
    skos:definition "Reference to a User definition." .

<http://www.cdisc.org/ns/odm/v2.0/UserType#Assessor> a odm:UserType,
        owl:Class ;
    rdfs:label "Assessor" .

<http://www.cdisc.org/ns/odm/v2.0/UserType#Care+provider> a odm:UserType,
        owl:Class ;
    rdfs:label "Care provider" .

<http://www.cdisc.org/ns/odm/v2.0/UserType#Data+analyst> a odm:UserType,
        owl:Class ;
    rdfs:label "Data analyst" .

<http://www.cdisc.org/ns/odm/v2.0/UserType#Investigator> a odm:UserType,
        owl:Class ;
    rdfs:label "Investigator" .

<http://www.cdisc.org/ns/odm/v2.0/UserType#Lab> a odm:UserType,
        owl:Class ;
    rdfs:label "Lab" .

<http://www.cdisc.org/ns/odm/v2.0/UserType#Monitor> a odm:UserType,
        owl:Class ;
    rdfs:label "Monitor" .

<http://www.cdisc.org/ns/odm/v2.0/UserType#Other> a odm:UserType,
        owl:Class ;
    rdfs:label "Other" .

<http://www.cdisc.org/ns/odm/v2.0/UserType#Sponsor> a odm:UserType,
        owl:Class ;
    rdfs:label "Sponsor" .

<http://www.cdisc.org/ns/odm/v2.0/UserType#Subject> a odm:UserType,
        owl:Class ;
    rdfs:label "Subject" .

odm:Version a owl:ObjectProperty,
        linkml:SlotDefinition ;
    rdfs:label "Version" ;
    rdfs:range odm:Text ;
    skos:definition "Version of Standard." .

<http://www.cdisc.org/ns/odm/v2.0/YesOrNo#No> a odm:YesOrNo,
        owl:Class ;
    rdfs:label "No" .

<http://www.cdisc.org/ns/odm/v2.0/YesOrNo#Yes> a odm:YesOrNo,
        owl:Class ;
    rdfs:label "Yes" .

odm:ref a owl:ObjectProperty,
        linkml:SlotDefinition ;
    rdfs:label "ref" ;
    rdfs:range odm:String ;
    skos:definition "Reference to a local instance (e.g. file) of the external library containing the FormalExpression code." .

odm:AddressRef a owl:ObjectProperty,
        linkml:SlotDefinition ;
    rdfs:label "AddressRef" ;
    rdfs:range odm:Address ;
    skos:definition "Address reference: The postal address for a user, location, or organization." .

odm:BranchingType a owl:Class,
        linkml:EnumDefinition ;
    rdfs:label "BranchingType" ;
    owl:unionOf ( <http://www.cdisc.org/ns/odm/v2.0/BranchingType#Exclusive> <http://www.cdisc.org/ns/odm/v2.0/BranchingType#Parallel> ) ;
    linkml:permissible_values <http://www.cdisc.org/ns/odm/v2.0/BranchingType#Exclusive>,
        <http://www.cdisc.org/ns/odm/v2.0/BranchingType#Parallel> .

odm:CodeList a owl:Class,
        linkml:ClassDefinition ;
    rdfs:label "CodeList" ;
    rdfs:subClassOf [ a owl:Restriction ;
            owl:maxQualifiedCardinality 1 ;
            owl:onClass odm:YesOnly ;
            owl:onProperty odm:IsNonStandard ],
        [ a owl:Restriction ;
            owl:allValuesFrom odm:Coding ;
            owl:onProperty odm:CodingRef ],
        [ a owl:Restriction ;
            owl:maxQualifiedCardinality 1 ;
            owl:onClass odm:Oidref ;
            owl:onProperty odm:CommentOID ],
        [ a owl:Restriction ;
            owl:onClass odm:Oid ;
            owl:onProperty odm:OID ;
            owl:qualifiedCardinality 1 ],
        [ a owl:Restriction ;
            owl:allValuesFrom odm:CodeListItem ;
            owl:onProperty odm:CodeListItemRef ],
        [ a owl:Restriction ;
            owl:onClass odm:Name ;
            owl:onProperty odm:Name ;
            owl:qualifiedCardinality 1 ],
        [ a owl:Restriction ;
            owl:onClass odm:CLDataType ;
            owl:onProperty odm:DataTypeRef ;
            owl:qualifiedCardinality 1 ],
        [ a owl:Restriction ;
            owl:allValuesFrom odm:Alias ;
            owl:onProperty odm:AliasRef ],
        [ a owl:Restriction ;
            owl:maxQualifiedCardinality 1 ;
            owl:onClass odm:Description ;
            owl:onProperty odm:DescriptionRef ],
        [ a owl:Restriction ;
            owl:maxQualifiedCardinality 1 ;
            owl:onClass odm:Oidref ;
            owl:onProperty odm:StandardOID ] ;
    skos:definition "Defines a discrete set of permitted values for an item, or provides a reference to a codelist or dictionary maintained by an external organization via the Coding element, or a combination of both. Examples provided under Coding." ;
    skos:exactMatch odm:CodeList .

odm:CodeListOID a owl:ObjectProperty,
        linkml:SlotDefinition ;
    rdfs:label "CodeListOID" ;
    rdfs:range odm:Oidref ;
    skos:definition "Reference to the CodeList definition that provides the allowable values for ItemData that references the ItemDef." .

odm:ConditionOID a owl:ObjectProperty,
        linkml:SlotDefinition ;
    rdfs:label "ConditionOID" ;
    rdfs:range odm:Oidref ;
    skos:definition "Reference to a ConditionDef defining the condition under which the transition must be executed" .

odm:ContextRef a owl:ObjectProperty,
        linkml:SlotDefinition ;
    rdfs:label "ContextRef" ;
    rdfs:range odm:String ;
    skos:definition "Identifies applicable domain or scope of the mapping." .

odm:CoreType a owl:Class,
        linkml:TypeDefinition ;
    rdfs:label "CoreType" ;
    rdfs:subClassOf [ a owl:Restriction ;
            owl:onDataRange odm:CoreType ;
            owl:onProperty linkml:topValue ;
            owl:qualifiedCardinality 1 ] .

odm:DefinitionRef a owl:ObjectProperty,
        linkml:SlotDefinition ;
    rdfs:label "DefinitionRef" ;
    rdfs:range odm:Definition ;
    skos:definition "A free-text definition of the parameter" .

odm:ID a owl:ObjectProperty,
        linkml:SlotDefinition ;
    rdfs:label "ID" ;
    rdfs:range odm:Oid ;
    skos:definition "Unique identifier for the leaf that is referenced." .

odm:IsNonStandard a owl:ObjectProperty,
        linkml:SlotDefinition ;
    rdfs:label "IsNonStandard" ;
    rdfs:range odm:YesOnly ;
    skos:definition "Required for ADaM, SDTM, or SEND if StandardOID is not provided." .

odm:ItemGroupClassSubClass a owl:Class,
        linkml:TypeDefinition ;
    rdfs:label "ItemGroupClassSubClass" ;
    rdfs:subClassOf [ a owl:Restriction ;
            owl:onDataRange odm:ItemGroupClassSubClass ;
            owl:onProperty linkml:topValue ;
            owl:qualifiedCardinality 1 ] .

odm:Level a owl:ObjectProperty,
        linkml:SlotDefinition ;
    rdfs:label "Level" ;
    rdfs:range odm:String ;
    skos:definition "Defined level for the Study Objective" .

odm:Location a owl:Class,
        linkml:ClassDefinition ;
    rdfs:label "Location" ;
    rdfs:subClassOf [ a owl:Restriction ;
            owl:maxQualifiedCardinality 1 ;
            owl:onClass odm:Oidref ;
            owl:onProperty odm:OrganizationOID ],
        [ a owl:Restriction ;
            owl:maxQualifiedCardinality 1 ;
            owl:onClass odm:Text ;
            owl:onProperty odm:Role ],
        [ a owl:Restriction ;
            owl:maxQualifiedCardinality 1 ;
            owl:onClass odm:Description ;
            owl:onProperty odm:DescriptionRef ],
        [ a owl:Restriction ;
            owl:allValuesFrom odm:Telecom ;
            owl:onProperty odm:TelecomRef ],
        [ a owl:Restriction ;
            owl:allValuesFrom odm:Query ;
            owl:onProperty odm:QueryRef ],
        [ a owl:Restriction ;
            owl:allValuesFrom odm:Address ;
            owl:onProperty odm:AddressRef ],
        [ a owl:Restriction ;
            owl:allValuesFrom odm:MetaDataVersionRef ;
            owl:onProperty odm:MetaDataVersionRefRef ],
        [ a owl:Restriction ;
            owl:onClass odm:Name ;
            owl:onProperty odm:Name ;
            owl:qualifiedCardinality 1 ],
        [ a owl:Restriction ;
            owl:onClass odm:Oid ;
            owl:onProperty odm:OID ;
            owl:qualifiedCardinality 1 ] ;
    skos:definition "A physical location associated with data collection and/or treatment of subjects." ;
    skos:exactMatch odm:Location .

odm:LocationRefRef a owl:ObjectProperty,
        linkml:SlotDefinition ;
    rdfs:label "LocationRefRef" ;
    rdfs:range odm:LocationRef ;
    skos:definition "LocationRef reference: A reference to the user's physical location." .

odm:MetaDataVersion a owl:Class,
        linkml:ClassDefinition ;
    rdfs:label "MetaDataVersion" ;
    rdfs:subClassOf [ a owl:Restriction ;
            owl:allValuesFrom odm:Leaf ;
            owl:onProperty odm:LeafRef ],
        [ a owl:Restriction ;
            owl:maxQualifiedCardinality 1 ;
            owl:onClass odm:Standards ;
            owl:onProperty odm:StandardsRef ],
        [ a owl:Restriction ;
            owl:allValuesFrom odm:ConditionDef ;
            owl:onProperty odm:ConditionDefRef ],
        [ a owl:Restriction ;
            owl:maxQualifiedCardinality 1 ;
            owl:onClass odm:Protocol ;
            owl:onProperty odm:ProtocolRef ],
        [ a owl:Restriction ;
            owl:onClass odm:Name ;
            owl:onProperty odm:Name ;
            owl:qualifiedCardinality 1 ],
        [ a owl:Restriction ;
            owl:allValuesFrom odm:WhereClauseDef ;
            owl:onProperty odm:WhereClauseDefRef ],
        [ a owl:Restriction ;
            owl:allValuesFrom odm:WorkflowDef ;
            owl:onProperty odm:WorkflowDefRef ],
        [ a owl:Restriction ;
            owl:onClass odm:Oid ;
            owl:onProperty odm:OID ;
            owl:qualifiedCardinality 1 ],
        [ a owl:Restriction ;
            owl:maxQualifiedCardinality 1 ;
            owl:onClass odm:Include ;
            owl:onProperty odm:IncludeRef ],
        [ a owl:Restriction ;
            owl:allValuesFrom odm:CommentDef ;
            owl:onProperty odm:CommentDefRef ],
        [ a owl:Restriction ;
            owl:maxQualifiedCardinality 1 ;
            owl:onClass odm:Oidref ;
            owl:onProperty odm:CommentOID ],
        [ a owl:Restriction ;
            owl:allValuesFrom odm:StudyEventDef ;
            owl:onProperty odm:StudyEventDefRef ],
        [ a owl:Restriction ;
            owl:maxQualifiedCardinality 1 ;
            owl:onClass odm:SupplementalDoc ;
            owl:onProperty odm:SupplementalDocRef ],
        [ a owl:Restriction ;
            owl:allValuesFrom odm:StudyEventGroupDef ;
            owl:onProperty odm:StudyEventGroupDefRef ],
        [ a owl:Restriction ;
            owl:allValuesFrom odm:ItemDef ;
            owl:onProperty odm:ItemDefRef ],
        [ a owl:Restriction ;
            owl:maxQualifiedCardinality 1 ;
            owl:onClass odm:AnnotatedCRF ;
            owl:onProperty odm:AnnotatedCRFRef ],
        [ a owl:Restriction ;
            owl:allValuesFrom odm:CodeList ;
            owl:onProperty odm:CodeListRefRef ],
        [ a owl:Restriction ;
            owl:allValuesFrom odm:ItemGroupDef ;
            owl:onProperty odm:ItemGroupDefRef ],
        [ a owl:Restriction ;
            owl:allValuesFrom odm:ValueListDef ;
            owl:onProperty odm:ValueListDefRef ],
        [ a owl:Restriction ;
            owl:maxQualifiedCardinality 1 ;
            owl:onClass odm:Description ;
            owl:onProperty odm:DescriptionRef ],
        [ a owl:Restriction ;
            owl:allValuesFrom odm:MethodDef ;
            owl:onProperty odm:MethodDefRef ] ;
    skos:definition "The metadata for a study is defined in a series of MetaDataVersion elements. Through this mechanism (multiple MetaDataVersion elements), the model supports the incremental deployment of \"mid-stream study changes,\" and thus can handle a situation where multiple versions of the metadata are being used simultaneously (e.g., due to delays in IRB approval at various sites)." ;
    skos:exactMatch odm:MetaDataVersion .

odm:MethodOID a owl:ObjectProperty,
        linkml:SlotDefinition ;
    rdfs:label "MethodOID" ;
    rdfs:range odm:Oidref ;
    skos:definition "Reference to a MethodDef that will provide one or more data rows as output. The MethodDef is used to prepopulate items" .

odm:MethodSignatureRef a owl:ObjectProperty,
        linkml:SlotDefinition ;
    rdfs:label "MethodSignatureRef" ;
    rdfs:range odm:MethodSignature ;
    skos:definition "MethodSignature reference: A MethodSignature defines the parameters and return values for a method. The MethodSignature improves traceability while enhancing the ability for automation engines to execute a MethodDef's FormalExpression. Most Methods use one or more input parameters and return one or more values." .

odm:ODMCoreType a owl:Class,
        linkml:EnumDefinition ;
    rdfs:label "ODMCoreType" ;
    owl:unionOf ( <http://www.cdisc.org/ns/odm/v2.0/ODMCoreType#HR> <http://www.cdisc.org/ns/odm/v2.0/ODMCoreType#O> <http://www.cdisc.org/ns/odm/v2.0/ODMCoreType#R/C> ) ;
    linkml:permissible_values <http://www.cdisc.org/ns/odm/v2.0/ODMCoreType#HR>,
        <http://www.cdisc.org/ns/odm/v2.0/ODMCoreType#O>,
        <http://www.cdisc.org/ns/odm/v2.0/ODMCoreType#R/C> .

odm:ODMVersion a owl:Class,
        linkml:TypeDefinition ;
    rdfs:label "ODMVersion" ;
    rdfs:subClassOf [ a owl:Restriction ;
            owl:onDataRange odm:ODMVersion ;
            owl:onProperty linkml:topValue ;
            owl:qualifiedCardinality 1 ] .

odm:PDFPageType a owl:Class,
        linkml:EnumDefinition ;
    rdfs:label "PDFPageType" ;
    owl:unionOf ( <http://www.cdisc.org/ns/odm/v2.0/PDFPageType#NamedDestination> <http://www.cdisc.org/ns/odm/v2.0/PDFPageType#PhysicalRef> ) ;
    linkml:permissible_values <http://www.cdisc.org/ns/odm/v2.0/PDFPageType#NamedDestination>,
        <http://www.cdisc.org/ns/odm/v2.0/PDFPageType#PhysicalRef> .

odm:QueryType a owl:Class,
        linkml:EnumDefinition ;
    rdfs:label "QueryType" ;
    owl:unionOf ( <http://www.cdisc.org/ns/odm/v2.0/QueryType#Manual> <http://www.cdisc.org/ns/odm/v2.0/QueryType#System> ) ;
    linkml:permissible_values <http://www.cdisc.org/ns/odm/v2.0/QueryType#Manual>,
        <http://www.cdisc.org/ns/odm/v2.0/QueryType#System> .

odm:Role a owl:ObjectProperty,
        linkml:SlotDefinition ;
    rdfs:label "Role" ;
    rdfs:range odm:Text ;
    skos:definition "The Role for the referenced ItemDef. The Role attribute provides a single role name describing the use of this data item. If the Role is defined by a standard terminology, RoleCodeListOID may be used to reference a CodeList that defines the full set roles from which the Role attribute value is to be taken." .

odm:StandardStatusEnum a owl:Class,
        linkml:EnumDefinition ;
    rdfs:label "StandardStatusEnum" ;
    owl:unionOf ( <http://ncicb.nci.nih.gov/xml/odm/EVS/CDISCExtCodeID:C172453> <http://ncicb.nci.nih.gov/xml/odm/EVS/CDISCExtCodeID:C172455> <http://ncicb.nci.nih.gov/xml/odm/EVS/CDISCExtCodeID:C172454> ) ;
    linkml:permissible_values <http://ncicb.nci.nih.gov/xml/odm/EVS/CDISCExtCodeID:C172453>,
        <http://ncicb.nci.nih.gov/xml/odm/EVS/CDISCExtCodeID:C172454>,
        <http://ncicb.nci.nih.gov/xml/odm/EVS/CDISCExtCodeID:C172455> .

odm:StandardType a owl:Class,
        linkml:EnumDefinition ;
    rdfs:label "StandardType" ;
    owl:unionOf ( <http://ncicb.nci.nih.gov/xml/odm/EVS/CDISCExtCodeID:C163415> <http://ncicb.nci.nih.gov/xml/odm/EVS/CDISCExtCodeID:C170454> ) ;
    linkml:permissible_values <http://ncicb.nci.nih.gov/xml/odm/EVS/CDISCExtCodeID:C163415>,
        <http://ncicb.nci.nih.gov/xml/odm/EVS/CDISCExtCodeID:C170454> .

odm:StudyEndPoint a owl:Class,
        linkml:ClassDefinition ;
    rdfs:label "StudyEndPoint" ;
    rdfs:subClassOf [ a owl:Restriction ;
            owl:onClass odm:Oid ;
            owl:onProperty odm:OID ;
            owl:qualifiedCardinality 1 ],
        [ a owl:Restriction ;
            owl:allValuesFrom odm:FormalExpression ;
            owl:onProperty odm:FormalExpressionRef ],
        [ a owl:Restriction ;
            owl:maxQualifiedCardinality 1 ;
            owl:onClass odm:StudyEstimandLevel ;
            owl:onProperty odm:Level ],
        [ a owl:Restriction ;
            owl:maxQualifiedCardinality 1 ;
            owl:onClass odm:StudyEndPointType ;
            owl:onProperty odm:Type ],
        [ a owl:Restriction ;
            owl:onClass odm:Name ;
            owl:onProperty odm:Name ;
            owl:qualifiedCardinality 1 ],
        [ a owl:Restriction ;
            owl:maxQualifiedCardinality 1 ;
            owl:onClass odm:Description ;
            owl:onProperty odm:DescriptionRef ] ;
    skos:definition "A study end point reflects an outcome measure of interest that is statistically analyzed to address a particular research question for the study. It typically specifies the type of assessments made; the timing of those assessments; the assessment tools used; and other details, as applicable, such as how multiple assessments within an individual are to be combined." ;
    skos:exactMatch odm:StudyEndPoint .

odm:StudyEndPointRefRef a owl:ObjectProperty,
        linkml:SlotDefinition ;
    rdfs:label "StudyEndPointRefRef" ;
    rdfs:range odm:StudyEndPointRef ;
    skos:definition "StudyEndPointRef reference: Go to start of metadata" .

odm:StudyEventGroupRefRef a owl:ObjectProperty,
        linkml:SlotDefinition ;
    rdfs:label "StudyEventGroupRefRef" ;
    rdfs:range odm:StudyEventGroupRef ;
    skos:definition "StudyEventGroupRef reference: This element references a StudyEventGroupDef as it occurs within a specific version of a study. The list of StudyEventGroupRefs identifies the types of study group events that are allowed to occur within the study." .

odm:StudyIntervention a owl:Class,
        linkml:ClassDefinition ;
    rdfs:label "StudyIntervention" ;
    rdfs:subClassOf [ a owl:Restriction ;
            owl:allValuesFrom odm:Coding ;
            owl:onProperty odm:CodingRef ],
        [ a owl:Restriction ;
            owl:onClass odm:Oid ;
            owl:onProperty odm:OID ;
            owl:qualifiedCardinality 1 ],
        [ a owl:Restriction ;
            owl:maxQualifiedCardinality 1 ;
            owl:onClass odm:Description ;
            owl:onProperty odm:DescriptionRef ] ;
    skos:definition "This element describes a study intervention (e.g., medication, treatment, therapy) for the clinical study. The human-readable description is provided in the Description element. The Coding element can be used to provide a machine-readable code for the indication (e.g., ATC M01AE01 code for \"Ibuprofen\" when used as a nonsteroidal anti-inflammatory drug)." ;
    skos:exactMatch odm:StudyIntervention .

odm:StudyTargetPopulation a owl:Class,
        linkml:ClassDefinition ;
    rdfs:label "StudyTargetPopulation" ;
    rdfs:subClassOf [ a owl:Restriction ;
            owl:maxQualifiedCardinality 1 ;
            owl:onClass odm:Description ;
            owl:onProperty odm:DescriptionRef ],
        [ a owl:Restriction ;
            owl:allValuesFrom odm:Coding ;
            owl:onProperty odm:CodingRef ],
        [ a owl:Restriction ;
            owl:allValuesFrom odm:FormalExpression ;
            owl:onProperty odm:FormalExpressionRef ],
        [ a owl:Restriction ;
            owl:onClass odm:Name ;
            owl:onProperty odm:Name ;
            owl:qualifiedCardinality 1 ],
        [ a owl:Restriction ;
            owl:onClass odm:Oid ;
            owl:onProperty odm:OID ;
            owl:qualifiedCardinality 1 ] ;
    skos:definition "The StudyTargetPopulation describes the population targeted for the clinical study." ;
    skos:exactMatch odm:StudyTargetPopulation .

odm:TelecomRef a owl:ObjectProperty,
        linkml:SlotDefinition ;
    rdfs:label "TelecomRef" ;
    rdfs:range odm:Telecom ;
    skos:definition "Telecom reference: The telecommunication contacts points of a user, a location, or an organization. The Type attribute designates the type of contact." .

odm:TimepointPostWindow a owl:ObjectProperty,
        linkml:SlotDefinition ;
    rdfs:label "TimepointPostWindow" ;
    rdfs:range odm:DurationDatetime ;
    skos:definition "Specifies the amount of time after the TimepointTarget, the time between the two activities, may be lengthened." .

odm:TimepointPreWindow a owl:ObjectProperty,
        linkml:SlotDefinition ;
    rdfs:label "TimepointPreWindow" ;
    rdfs:range odm:DurationDatetime ;
    skos:definition "Specifies the amount of time prior to the TimepointTarget, the time between the two activities, may be shortened." .

odm:User a owl:Class,
        linkml:ClassDefinition ;
    rdfs:label "User" ;
    rdfs:subClassOf [ a owl:Restriction ;
            owl:onClass odm:Oid ;
            owl:onProperty odm:OID ;
            owl:qualifiedCardinality 1 ],
        [ a owl:Restriction ;
            owl:maxQualifiedCardinality 1 ;
            owl:onClass odm:GivenName ;
            owl:onProperty odm:GivenNameRef ],
        [ a owl:Restriction ;
            owl:maxQualifiedCardinality 1 ;
            owl:onClass odm:Image ;
            owl:onProperty odm:ImageRef ],
        [ a owl:Restriction ;
            owl:maxQualifiedCardinality 1 ;
            owl:onClass odm:Oidref ;
            owl:onProperty odm:OrganizationOID ],
        [ a owl:Restriction ;
            owl:maxQualifiedCardinality 1 ;
            owl:onClass odm:FamilyName ;
            owl:onProperty odm:FamilyNameRef ],
        [ a owl:Restriction ;
            owl:maxQualifiedCardinality 1 ;
            owl:onClass odm:UserName ;
            owl:onProperty odm:UserNameRef ],
        [ a owl:Restriction ;
            owl:maxQualifiedCardinality 1 ;
            owl:onClass odm:Suffix ;
            owl:onProperty odm:SuffixRef ],
        [ a owl:Restriction ;
            owl:allValuesFrom odm:Telecom ;
            owl:onProperty odm:TelecomRef ],
        [ a owl:Restriction ;
            owl:maxQualifiedCardinality 1 ;
            owl:onClass odm:UserType ;
            owl:onProperty odm:UserTypeRef ],
        [ a owl:Restriction ;
            owl:maxQualifiedCardinality 1 ;
            owl:onClass odm:Prefix ;
            owl:onProperty odm:PrefixRef ],
        [ a owl:Restriction ;
            owl:maxQualifiedCardinality 1 ;
            owl:onClass odm:FullName ;
            owl:onProperty odm:FullNameRef ],
        [ a owl:Restriction ;
            owl:allValuesFrom odm:Address ;
            owl:onProperty odm:AddressRef ],
        [ a owl:Restriction ;
            owl:maxQualifiedCardinality 1 ;
            owl:onClass odm:Oidref ;
            owl:onProperty odm:LocationOID ] ;
    skos:definition "Information about a specific user of a clinical data collection or data management system." ;
    skos:exactMatch odm:User .

odm:UserRefRef a owl:ObjectProperty,
        linkml:SlotDefinition ;
    rdfs:label "UserRefRef" ;
    rdfs:range odm:UserRef ;
    skos:definition "UserRef reference: None" .

odm:AbsoluteTimingConstraint a owl:Class,
        linkml:ClassDefinition ;
    rdfs:label "AbsoluteTimingConstraint" ;
    rdfs:subClassOf [ a owl:Restriction ;
            owl:onClass odm:Name ;
            owl:onProperty odm:Name ;
            owl:qualifiedCardinality 1 ],
        [ a owl:Restriction ;
            owl:maxQualifiedCardinality 1 ;
            owl:onClass odm:DurationDatetime ;
            owl:onProperty odm:TimepointPostWindow ],
        [ a owl:Restriction ;
            owl:maxQualifiedCardinality 1 ;
            owl:onClass odm:DurationDatetime ;
            owl:onProperty odm:TimepointPreWindow ],
        [ a owl:Restriction ;
            owl:maxQualifiedCardinality 1 ;
            owl:onClass odm:Oidref ;
            owl:onProperty odm:StudyEventGroupOID ],
        [ a owl:Restriction ;
            owl:onClass odm:String ;
            owl:onProperty odm:TimepointTarget ;
            owl:qualifiedCardinality 1 ],
        [ a owl:Restriction ;
            owl:maxQualifiedCardinality 1 ;
            owl:onClass odm:Oidref ;
            owl:onProperty odm:StudyEventOID ],
        [ a owl:Restriction ;
            owl:maxQualifiedCardinality 1 ;
            owl:onClass odm:Description ;
            owl:onProperty odm:DescriptionRef ],
        [ a owl:Restriction ;
            owl:onClass odm:Oid ;
            owl:onProperty odm:OID ;
            owl:qualifiedCardinality 1 ] ;
    skos:definition "The element AbsoluteTimingConstraint is used to specify when an activity, represented by either a StudyEventGroup or StudyEvent, can take place." ;
    skos:exactMatch odm:AbsoluteTimingConstraint .

odm:AdminData a owl:Class,
        linkml:ClassDefinition ;
    rdfs:label "AdminData" ;
    rdfs:subClassOf [ a owl:Restriction ;
            owl:maxQualifiedCardinality 1 ;
            owl:onClass odm:Oidref ;
            owl:onProperty odm:StudyOID ],
        [ a owl:Restriction ;
            owl:allValuesFrom odm:Location ;
            owl:onProperty odm:LocationRefRef ],
        [ a owl:Restriction ;
            owl:allValuesFrom odm:User ;
            owl:onProperty odm:UserRefRef ],
        [ a owl:Restriction ;
            owl:allValuesFrom odm:SignatureDef ;
            owl:onProperty odm:SignatureDefRef ],
        [ a owl:Restriction ;
            owl:allValuesFrom odm:Organization ;
            owl:onProperty odm:OrganizationRef ] ;
    skos:definition "Administrative information about users, locations, organizations, and electronic signatures." ;
    skos:exactMatch odm:AdminData .

odm:AnnotatedCRF a owl:Class,
        linkml:ClassDefinition ;
    rdfs:label "AnnotatedCRF" ;
    rdfs:subClassOf [ a owl:Restriction ;
            owl:allValuesFrom odm:DocumentRef ;
            owl:onProperty odm:DocumentRefRef ] ;
    skos:definition "An Annotated Case Report Form (CRF) is a Portable File Format (PDF) document that provides the mapping of data collection fields to the variables or discrete variable values contained within the datasets." ;
    skos:exactMatch odm:AnnotatedCRF .

odm:Arm a owl:Class,
        linkml:ClassDefinition ;
    rdfs:label "Arm" ;
    rdfs:subClassOf [ a owl:Restriction ;
            owl:maxQualifiedCardinality 1 ;
            owl:onClass odm:Description ;
            owl:onProperty odm:DescriptionRef ],
        [ a owl:Restriction ;
            owl:onClass odm:Oid ;
            owl:onProperty odm:OID ;
            owl:qualifiedCardinality 1 ],
        [ a owl:Restriction ;
            owl:onClass odm:Name ;
            owl:onProperty odm:Name ;
            owl:qualifiedCardinality 1 ],
        [ a owl:Restriction ;
            owl:maxQualifiedCardinality 1 ;
            owl:onClass odm:WorkflowRef ;
            owl:onProperty odm:WorkflowRefRef ] ;
    skos:definition "An Arm element provides the declaration of a study arm. Arms do not have any ordering relative to one another." ;
    skos:exactMatch odm:Arm .

odm:Association a owl:Class,
        linkml:ClassDefinition ;
    rdfs:label "Association" ;
    rdfs:subClassOf [ a owl:Restriction ;
            owl:maxQualifiedCardinality 1 ;
            owl:onClass odm:Annotation ;
            owl:onProperty odm:AnnotationRef ],
        [ a owl:Restriction ;
            owl:maxQualifiedCardinality 1 ;
            owl:onClass odm:KeySet ;
            owl:onProperty odm:KeySetRef ],
        [ a owl:Restriction ;
            owl:onClass odm:Oidref ;
            owl:onProperty odm:StudyOID ;
            owl:qualifiedCardinality 1 ],
        [ a owl:Restriction ;
            owl:onClass odm:Oidref ;
            owl:onProperty odm:MetaDataVersionOID ;
            owl:qualifiedCardinality 1 ] ;
    skos:definition "An association permits an annotation to be placed on an ordered pair of entities rather than on just one. The first and second KeySets identify the start and end of the annotated \"link." ;
    skos:exactMatch odm:Association .

odm:Branching a owl:Class,
        linkml:ClassDefinition ;
    rdfs:label "Branching" ;
    rdfs:subClassOf [ a owl:Restriction ;
            owl:onClass odm:BranchingType ;
            owl:onProperty odm:Type ;
            owl:qualifiedCardinality 1 ],
        [ a owl:Restriction ;
            owl:allValuesFrom odm:TargetTransition ;
            owl:onProperty odm:TargetTransitionRef ],
        [ a owl:Restriction ;
            owl:onClass odm:Oid ;
            owl:onProperty odm:OID ;
            owl:qualifiedCardinality 1 ],
        [ a owl:Restriction ;
            owl:allValuesFrom odm:DefaultTransition ;
            owl:onProperty odm:DefaultTransitionRef ],
        [ a owl:Restriction ;
            owl:onClass odm:Name ;
            owl:onProperty odm:Name ;
            owl:qualifiedCardinality 1 ] ;
    skos:definition "This element describes the branching in a workflow from a source (start) structural element to 2 or more target structural elements, over a Transition element." ;
    skos:exactMatch odm:Branching .

odm:CDISCNotes a owl:Class,
        linkml:ClassDefinition ;
    rdfs:label "CDISCNotes" ;
    rdfs:subClassOf [ a owl:Restriction ;
            owl:allValuesFrom odm:TranslatedText ;
            owl:onProperty odm:TranslatedTextRef ] ;
    skos:definition "Explanatory text for the variable." ;
    skos:exactMatch odm:CDISCNotes .

odm:CRFCompletionInstructions a owl:Class,
        linkml:ClassDefinition ;
    rdfs:label "CRFCompletionInstructions" ;
    rdfs:subClassOf [ a owl:Restriction ;
            owl:allValuesFrom odm:TranslatedText ;
            owl:onProperty odm:TranslatedTextRef ] ;
    skos:definition "Instructions for the clinical site on how to enter collected information on the CRF." ;
    skos:exactMatch odm:CRFCompletionInstructions .

odm:CheckValue a owl:Class,
        linkml:ClassDefinition ;
    rdfs:label "CheckValue" ;
    rdfs:subClassOf [ a owl:Restriction ;
            owl:maxQualifiedCardinality 1 ;
            owl:onClass odm:ContentType ;
            owl:onProperty odm:_content ],
        [ a owl:Restriction ;
            owl:maxQualifiedCardinality 1 ;
            owl:onClass odm:String ;
            owl:onProperty odm:range ] ;
    skos:definition "A comparison value used in a range check." ;
    skos:exactMatch odm:CheckValue .

odm:City a owl:Class,
        linkml:ClassDefinition ;
    rdfs:label "City" ;
    rdfs:subClassOf [ a owl:Restriction ;
            owl:maxQualifiedCardinality 1 ;
            owl:onClass odm:ContentType ;
            owl:onProperty odm:_content ],
        [ a owl:Restriction ;
            owl:maxQualifiedCardinality 1 ;
            owl:onClass odm:String ;
            owl:onProperty odm:range ] ;
    skos:definition "The city name part of a user's postal address." ;
    skos:exactMatch odm:City .

odm:Class a owl:Class,
        linkml:ClassDefinition ;
    rdfs:label "Class" ;
    rdfs:subClassOf [ a owl:Restriction ;
            owl:allValuesFrom odm:SubClass ;
            owl:onProperty odm:SubClassRef ],
        [ a owl:Restriction ;
            owl:onClass odm:ItemGroupClass ;
            owl:onProperty odm:Name ;
            owl:qualifiedCardinality 1 ] ;
    skos:exactMatch odm:Class .

odm:ClinicalData a owl:Class,
        linkml:ClassDefinition ;
    rdfs:label "ClinicalData" ;
    rdfs:subClassOf [ a owl:Restriction ;
            owl:maxQualifiedCardinality 1 ;
            owl:onClass odm:Signature ;
            owl:onProperty odm:SignatureRefRef ],
        [ a owl:Restriction ;
            owl:allValuesFrom odm:Query ;
            owl:onProperty odm:QueryRef ],
        [ a owl:Restriction ;
            owl:allValuesFrom odm:ItemGroupData ;
            owl:onProperty odm:ItemGroupDataRef ],
        [ a owl:Restriction ;
            owl:maxQualifiedCardinality 1 ;
            owl:onClass odm:Annotation ;
            owl:onProperty odm:AnnotationRef ],
        [ a owl:Restriction ;
            owl:allValuesFrom odm:SubjectData ;
            owl:onProperty odm:SubjectDataRef ],
        [ a owl:Restriction ;
            owl:onClass odm:Oidref ;
            owl:onProperty odm:MetaDataVersionOID ;
            owl:qualifiedCardinality 1 ],
        [ a owl:Restriction ;
            owl:maxQualifiedCardinality 1 ;
            owl:onClass odm:AuditRecord ;
            owl:onProperty odm:AuditRecordRef ],
        [ a owl:Restriction ;
            owl:onClass odm:Oidref ;
            owl:onProperty odm:StudyOID ;
            owl:qualifiedCardinality 1 ] ;
    skos:definition "Clinical data for 1 or more subjects." ;
    skos:exactMatch odm:ClinicalData .

odm:Code a owl:Class,
        linkml:ClassDefinition ;
    rdfs:label "Code" ;
    rdfs:subClassOf [ a owl:Restriction ;
            owl:maxQualifiedCardinality 1 ;
            owl:onClass odm:String ;
            owl:onProperty odm:range ],
        [ a owl:Restriction ;
            owl:maxQualifiedCardinality 1 ;
            owl:onClass odm:ContentType ;
            owl:onProperty odm:_content ] ;
    skos:definition "Contains the source code that represents a FormalExpression in a given Context. The source code must be executable, and the MethodSignature defines the input parameters and return values for the code." ;
    skos:exactMatch odm:Code .

odm:CodeListItem a owl:Class,
        linkml:ClassDefinition ;
    rdfs:label "CodeListItem" ;
    rdfs:subClassOf [ a owl:Restriction ;
            owl:maxQualifiedCardinality 1 ;
            owl:onClass odm:Decode ;
            owl:onProperty odm:DecodeRef ],
        [ a owl:Restriction ;
            owl:onClass odm:Value ;
            owl:onProperty odm:CodedValue ;
            owl:qualifiedCardinality 1 ],
        [ a owl:Restriction ;
            owl:maxQualifiedCardinality 1 ;
            owl:onClass odm:Oidref ;
            owl:onProperty odm:CommentOID ],
        [ a owl:Restriction ;
            owl:allValuesFrom odm:Coding ;
            owl:onProperty odm:CodingRef ],
        [ a owl:Restriction ;
            owl:allValuesFrom odm:Alias ;
            owl:onProperty odm:AliasRef ],
        [ a owl:Restriction ;
            owl:maxQualifiedCardinality 1 ;
            owl:onClass odm:PositiveInteger ;
            owl:onProperty odm:OrderNumber ],
        [ a owl:Restriction ;
            owl:maxQualifiedCardinality 1 ;
            owl:onClass odm:Decimal ;
            owl:onProperty odm:Rank ],
        [ a owl:Restriction ;
            owl:maxQualifiedCardinality 1 ;
            owl:onClass odm:YesOnly ;
            owl:onProperty odm:ExtendedValue ],
        [ a owl:Restriction ;
            owl:maxQualifiedCardinality 1 ;
            owl:onClass odm:Description ;
            owl:onProperty odm:DescriptionRef ],
        [ a owl:Restriction ;
            owl:maxQualifiedCardinality 1 ;
            owl:onClass odm:YesOnly ;
            owl:onProperty odm:Other ] ;
    skos:definition "Defines an individual member value of a codelist. It may include a display value in the child Decode element" ;
    skos:exactMatch odm:CodeListItem .

odm:CodeListRef a owl:Class,
        linkml:ClassDefinition ;
    rdfs:label "CodeListRef" ;
    rdfs:subClassOf [ a owl:Restriction ;
            owl:onClass odm:Oidref ;
            owl:onProperty odm:CodeListOID ;
            owl:qualifiedCardinality 1 ] ;
    skos:definition "A reference to a CodeList definition." ;
    skos:exactMatch odm:CodeListRef .

odm:CollectionExceptionConditionOID a owl:ObjectProperty,
        linkml:SlotDefinition ;
    rdfs:label "CollectionExceptionConditionOID" ;
    rdfs:range odm:Oidref ;
    skos:definition "Reference to a ConditionDef" .

odm:Comment a owl:Class,
        linkml:ClassDefinition ;
    rdfs:label "Comment" ;
    rdfs:subClassOf [ a owl:Restriction ;
            owl:allValuesFrom odm:TranslatedText ;
            owl:onProperty odm:TranslatedTextRef ],
        [ a owl:Restriction ;
            owl:maxQualifiedCardinality 1 ;
            owl:onClass odm:CommentType ;
            owl:onProperty odm:SponsorOrSite ] ;
    skos:definition "A free-text (uninterpreted) comment about clinical data. The comment may have come from the sponsor or the clinical site." ;
    skos:exactMatch odm:Comment .

odm:CommentDef a owl:Class,
        linkml:ClassDefinition ;
    rdfs:label "CommentDef" ;
    rdfs:subClassOf [ a owl:Restriction ;
            owl:onClass odm:Oid ;
            owl:onProperty odm:OID ;
            owl:qualifiedCardinality 1 ],
        [ a owl:Restriction ;
            owl:maxQualifiedCardinality 1 ;
            owl:onClass odm:Description ;
            owl:onProperty odm:DescriptionRef ],
        [ a owl:Restriction ;
            owl:allValuesFrom odm:DocumentRef ;
            owl:onProperty odm:DocumentRefRef ] ;
    skos:definition "The Comment element allows referencing short comments self-contained in the XML document or long comments normally included in external documents. For comments included in external documents, the reference could include specific pages of a document where the comments are included." ;
    skos:exactMatch odm:CommentDef .

odm:CommentType a owl:Class,
        linkml:EnumDefinition ;
    rdfs:label "CommentType" ;
    owl:unionOf ( <http://www.cdisc.org/ns/odm/v2.0/CommentType#Sponsor> <http://www.cdisc.org/ns/odm/v2.0/CommentType#Site> ) ;
    linkml:permissible_values <http://www.cdisc.org/ns/odm/v2.0/CommentType#Site>,
        <http://www.cdisc.org/ns/odm/v2.0/CommentType#Sponsor> .

odm:ConditionDef a owl:Class,
        linkml:ClassDefinition ;
    rdfs:label "ConditionDef" ;
    rdfs:subClassOf [ a owl:Restriction ;
            owl:maxQualifiedCardinality 1 ;
            owl:onClass odm:Description ;
            owl:onProperty odm:DescriptionRef ],
        [ a owl:Restriction ;
            owl:maxQualifiedCardinality 1 ;
            owl:onClass odm:MethodSignature ;
            owl:onProperty odm:MethodSignatureRef ],
        [ a owl:Restriction ;
            owl:maxQualifiedCardinality 1 ;
            owl:onClass odm:Oidref ;
            owl:onProperty odm:CommentOID ],
        [ a owl:Restriction ;
            owl:onClass odm:Name ;
            owl:onProperty odm:Name ;
            owl:qualifiedCardinality 1 ],
        [ a owl:Restriction ;
            owl:onClass odm:Oid ;
            owl:onProperty odm:OID ;
            owl:qualifiedCardinality 1 ],
        [ a owl:Restriction ;
            owl:allValuesFrom odm:Alias ;
            owl:onProperty odm:AliasRef ],
        [ a owl:Restriction ;
            owl:allValuesFrom odm:FormalExpression ;
            owl:onProperty odm:FormalExpressionRef ] ;
    skos:definition "A ConditionDef defines a boolean condition." ;
    skos:exactMatch odm:ConditionDef .

odm:Context a owl:Class,
        linkml:EnumDefinition ;
    rdfs:label "Context" ;
    owl:unionOf ( <http://www.cdisc.org/ns/odm/v2.0/Context#Archive> <http://www.cdisc.org/ns/odm/v2.0/Context#Exchange> <http://www.cdisc.org/ns/odm/v2.0/Context#Submission> ) ;
    linkml:permissible_values <http://www.cdisc.org/ns/odm/v2.0/Context#Archive>,
        <http://www.cdisc.org/ns/odm/v2.0/Context#Exchange>,
        <http://www.cdisc.org/ns/odm/v2.0/Context#Submission> .

odm:Country a owl:Class,
        linkml:ClassDefinition ;
    rdfs:label "Country" ;
    rdfs:subClassOf [ a owl:Restriction ;
            owl:maxQualifiedCardinality 1 ;
            owl:onClass odm:ContentType ;
            owl:onProperty odm:_content ],
        [ a owl:Restriction ;
            owl:maxQualifiedCardinality 1 ;
            owl:onClass odm:String ;
            owl:onProperty odm:range ] ;
    skos:definition "The country name part of a user's postal address. For CDISC SDTM or trial registry applications, this must be represented by an ISO 3166 3-letter or US-GENC country code (e.g., FRA for France, JPN for Japan)." ;
    skos:exactMatch odm:Country .

odm:CriterionRef a owl:ObjectProperty,
        linkml:SlotDefinition ;
    rdfs:label "CriterionRef" ;
    rdfs:range odm:Criterion ;
    skos:definition "Criterion reference: The Criterion represents either an inclusion or an exclusion criterion, depending on the parent element (i.e., InclusionCriteria, ExclusionCriteria)." .

odm:DataTypeRef a owl:ObjectProperty,
        linkml:SlotDefinition ;
    rdfs:label "DataTypeRef" ;
    rdfs:range odm:String ;
    skos:definition """The DataType attribute specifies how the corresponding value
                    elements are to be interpreted for comparison and storage.""" .

odm:Decode a owl:Class,
        linkml:ClassDefinition ;
    rdfs:label "Decode" ;
    rdfs:subClassOf [ a owl:Restriction ;
            owl:allValuesFrom odm:TranslatedText ;
            owl:onProperty odm:TranslatedTextRef ] ;
    skos:definition "The displayed value relating to the CodeListItem/@CodedValue. This is often a label corresponding to a short name or alpha-numeric code. The actual Decode text is provided in a TranslatedText element so that it can be provided in different languages on a case report form or tabular data summary." ;
    skos:exactMatch odm:Decode .

odm:DefCoreType a owl:Class,
        linkml:EnumDefinition ;
    rdfs:label "DefCoreType" ;
    owl:unionOf ( <http://www.cdisc.org/ns/odm/v2.0/DefCoreType#Cond> <http://www.cdisc.org/ns/odm/v2.0/DefCoreType#Exp> <http://www.cdisc.org/ns/odm/v2.0/DefCoreType#Perm> <http://www.cdisc.org/ns/odm/v2.0/DefCoreType#Req> ) ;
    linkml:permissible_values <http://www.cdisc.org/ns/odm/v2.0/DefCoreType#Cond>,
        <http://www.cdisc.org/ns/odm/v2.0/DefCoreType#Exp>,
        <http://www.cdisc.org/ns/odm/v2.0/DefCoreType#Perm>,
        <http://www.cdisc.org/ns/odm/v2.0/DefCoreType#Req> .

odm:DefaultTransition a owl:Class,
        linkml:ClassDefinition ;
    rdfs:label "DefaultTransition" ;
    rdfs:subClassOf [ a owl:Restriction ;
            owl:onClass odm:Oidref ;
            owl:onProperty odm:TargetTransitionOID ;
            owl:qualifiedCardinality 1 ] ;
    skos:exactMatch odm:DefaultTransition .

odm:Definition a owl:Class,
        linkml:ClassDefinition ;
    rdfs:label "Definition" ;
    rdfs:subClassOf [ a owl:Restriction ;
            owl:allValuesFrom odm:TranslatedText ;
            owl:onProperty odm:TranslatedTextRef ] ;
    skos:definition "Definition of the item." ;
    skos:exactMatch odm:Definition .

odm:DurationTimingConstraint a owl:Class,
        linkml:ClassDefinition ;
    rdfs:label "DurationTimingConstraint" ;
    rdfs:subClassOf [ a owl:Restriction ;
            owl:onClass odm:Name ;
            owl:onProperty odm:Name ;
            owl:qualifiedCardinality 1 ],
        [ a owl:Restriction ;
            owl:onClass odm:Oidref ;
            owl:onProperty odm:StructuralElementOID ;
            owl:qualifiedCardinality 1 ],
        [ a owl:Restriction ;
            owl:maxQualifiedCardinality 1 ;
            owl:onClass odm:Description ;
            owl:onProperty odm:DescriptionRef ],
        [ a owl:Restriction ;
            owl:onClass odm:Oid ;
            owl:onProperty odm:OID ;
            owl:qualifiedCardinality 1 ],
        [ a owl:Restriction ;
            owl:onClass odm:DurationDatetime ;
            owl:onProperty odm:DurationTarget ;
            owl:qualifiedCardinality 1 ],
        [ a owl:Restriction ;
            owl:maxQualifiedCardinality 1 ;
            owl:onClass odm:DurationDatetime ;
            owl:onProperty odm:DurationPreWindow ],
        [ a owl:Restriction ;
            owl:maxQualifiedCardinality 1 ;
            owl:onClass odm:DurationDatetime ;
            owl:onProperty odm:DurationPostWindow ] ;
    skos:definition "The DurationTimingConstraint constrains the duration of an activity represented by a study, epoch, StudyEventGroupDef, StudyEventDef, ItemGroupDef, or ItemDef. It is used to constrain the duration of the visit, activity, or any other structural element." ;
    skos:exactMatch odm:DurationTimingConstraint .

odm:Epoch a owl:Class,
        linkml:ClassDefinition ;
    rdfs:label "Epoch" ;
    rdfs:subClassOf [ a owl:Restriction ;
            owl:onClass odm:Name ;
            owl:onProperty odm:Name ;
            owl:qualifiedCardinality 1 ],
        [ a owl:Restriction ;
            owl:onClass odm:Oid ;
            owl:onProperty odm:OID ;
            owl:qualifiedCardinality 1 ],
        [ a owl:Restriction ;
            owl:onClass odm:PositiveInteger ;
            owl:onProperty odm:SequenceNumber ;
            owl:qualifiedCardinality 1 ],
        [ a owl:Restriction ;
            owl:maxQualifiedCardinality 1 ;
            owl:onClass odm:Description ;
            owl:onProperty odm:DescriptionRef ] ;
    skos:definition "The planned period of subjects' participation in the trial is divided into sequential epochs. Each epoch is a period of time that serves a purpose in the trial as a whole. Epochs cannot overlap. The sequence of the epoch in the study is provided by the SequenceNumber attribute, the first epoch in the study being assigned the sequence number 1. Sequence numbers are subsequent." ;
    skos:exactMatch odm:Epoch .

odm:ErrorMessage a owl:Class,
        linkml:ClassDefinition ;
    rdfs:label "ErrorMessage" ;
    rdfs:subClassOf [ a owl:Restriction ;
            owl:allValuesFrom odm:TranslatedText ;
            owl:onProperty odm:TranslatedTextRef ] ;
    skos:definition "Error message provided to user when the range check fails." ;
    skos:exactMatch odm:ErrorMessage .

odm:EventType a owl:Class,
        linkml:EnumDefinition ;
    rdfs:label "EventType" ;
    owl:unionOf ( <http://www.cdisc.org/ns/odm/v2.0/EventType#Scheduled> <http://www.cdisc.org/ns/odm/v2.0/EventType#Unscheduled> <http://www.cdisc.org/ns/odm/v2.0/EventType#Common> ) ;
    linkml:permissible_values <http://www.cdisc.org/ns/odm/v2.0/EventType#Common>,
        <http://www.cdisc.org/ns/odm/v2.0/EventType#Scheduled>,
        <http://www.cdisc.org/ns/odm/v2.0/EventType#Unscheduled> .

odm:ExclusionCriteria a owl:Class,
        linkml:ClassDefinition ;
    rdfs:label "ExclusionCriteria" ;
    rdfs:subClassOf [ a owl:Restriction ;
            owl:allValuesFrom odm:Criterion ;
            owl:onProperty odm:CriterionRef ] ;
    skos:definition "The ExclusionCriteria is a container element for Criterion elements describing exclusion criteria for subjects in the study. When a list is provided, not meeting any of the criteria in the list may lead to exclusion of enrollment in the study." ;
    skos:exactMatch odm:ExclusionCriteria .

odm:ExternalCodeLib a owl:Class,
        linkml:ClassDefinition ;
    rdfs:label "ExternalCodeLib" ;
    rdfs:subClassOf [ a owl:Restriction ;
            owl:onClass odm:Name ;
            owl:onProperty odm:Library ;
            owl:qualifiedCardinality 1 ],
        [ a owl:Restriction ;
            owl:maxQualifiedCardinality 1 ;
            owl:onClass odm:Text ;
            owl:onProperty odm:ref ],
        [ a owl:Restriction ;
            owl:maxQualifiedCardinality 1 ;
            owl:onClass odm:Name ;
            owl:onProperty odm:Method ],
        [ a owl:Restriction ;
            owl:maxQualifiedCardinality 1 ;
            owl:onClass odm:Text ;
            owl:onProperty odm:Version ],
        [ a owl:Restriction ;
            owl:maxQualifiedCardinality 1 ;
            owl:onClass odm:Uriorcurie ;
            owl:onProperty odm:href ] ;
    skos:definition "The ExternalCodeLib element references a FormalExpression in an external code library, such as a file or GitHub. The intention is to make it possible to reference existing code libraries where the code is maintained as well as making it simpler to include longer, more complex FormalExpressions. The Library attribute provides the name of the external library, whereas ref or href provides a reference to the repository that can be used to retrieve the code. The Method attribute provides the name of the method in the file referenced for cases where multiple methods are provided in the source code file. The Version element provides the version of the external FormalExpression code referenced." ;
    skos:exactMatch odm:ExternalCodeLib .

odm:FamilyName a owl:Class,
        linkml:ClassDefinition ;
    rdfs:label "FamilyName" ;
    rdfs:subClassOf [ a owl:Restriction ;
            owl:maxQualifiedCardinality 1 ;
            owl:onClass odm:ContentType ;
            owl:onProperty odm:_content ],
        [ a owl:Restriction ;
            owl:maxQualifiedCardinality 1 ;
            owl:onClass odm:String ;
            owl:onProperty odm:range ] ;
    skos:definition "The user's surname (family name)." ;
    skos:exactMatch odm:FamilyName .

odm:FileType a owl:Class,
        linkml:EnumDefinition ;
    rdfs:label "FileType" ;
    owl:unionOf ( <http://www.cdisc.org/ns/odm/v2.0/FileType#Snapshot> <http://www.cdisc.org/ns/odm/v2.0/FileType#Transactional> ) ;
    linkml:permissible_values <http://www.cdisc.org/ns/odm/v2.0/FileType#Snapshot>,
        <http://www.cdisc.org/ns/odm/v2.0/FileType#Transactional> .

odm:Flag a owl:Class,
        linkml:ClassDefinition ;
    rdfs:label "Flag" ;
    rdfs:subClassOf [ a owl:Restriction ;
            owl:maxQualifiedCardinality 1 ;
            owl:onClass odm:FlagValue ;
            owl:onProperty odm:FlagValueRef ],
        [ a owl:Restriction ;
            owl:maxQualifiedCardinality 1 ;
            owl:onClass odm:FlagType ;
            owl:onProperty odm:FlagTypeRef ] ;
    skos:definition "A machine-processable annotation." ;
    skos:exactMatch odm:Flag .

odm:FlagType a owl:Class,
        linkml:ClassDefinition ;
    rdfs:label "FlagType" ;
    rdfs:subClassOf [ a owl:Restriction ;
            owl:onClass odm:Oidref ;
            owl:onProperty odm:CodeListOID ;
            owl:qualifiedCardinality 1 ],
        [ a owl:Restriction ;
            owl:maxQualifiedCardinality 1 ;
            owl:onClass odm:Name ;
            owl:onProperty odm:_content ] ;
    skos:definition "The type of flag. This determines the purpose and semantics of the flag." ;
    skos:exactMatch odm:FlagType .

odm:FlagValue a owl:Class,
        linkml:ClassDefinition ;
    rdfs:label "FlagValue" ;
    rdfs:subClassOf [ a owl:Restriction ;
            owl:maxQualifiedCardinality 1 ;
            owl:onClass odm:Name ;
            owl:onProperty odm:_content ],
        [ a owl:Restriction ;
            owl:onClass odm:Oidref ;
            owl:onProperty odm:CodeListOID ;
            owl:qualifiedCardinality 1 ] ;
    skos:definition "The value of the flag. The meaning of this value is typically dependent on the associated FlagType. The actual value must be a member of the referenced CodeList" ;
    skos:exactMatch odm:FlagValue .

odm:FullName a owl:Class,
        linkml:ClassDefinition ;
    rdfs:label "FullName" ;
    rdfs:subClassOf [ a owl:Restriction ;
            owl:maxQualifiedCardinality 1 ;
            owl:onClass odm:ContentType ;
            owl:onProperty odm:_content ],
        [ a owl:Restriction ;
            owl:maxQualifiedCardinality 1 ;
            owl:onClass odm:String ;
            owl:onProperty odm:range ] ;
    skos:definition "The user's full formal name. May be a combination of Prefix, GivenName, FamilyName & Suffix. Intended to be used for display." ;
    skos:exactMatch odm:FullName .

odm:GeoPosition a owl:Class,
        linkml:ClassDefinition ;
    rdfs:label "GeoPosition" ;
    rdfs:subClassOf [ a owl:Restriction ;
            owl:maxQualifiedCardinality 1 ;
            owl:onClass odm:Decimal ;
            owl:onProperty odm:Latitude ],
        [ a owl:Restriction ;
            owl:maxQualifiedCardinality 1 ;
            owl:onClass odm:Decimal ;
            owl:onProperty odm:Altitude ],
        [ a owl:Restriction ;
            owl:maxQualifiedCardinality 1 ;
            owl:onClass odm:Decimal ;
            owl:onProperty odm:Longitude ] ;
    skos:definition "The geographical position using the World Geodetic System WGS84." ;
    skos:exactMatch odm:GeoPosition .

odm:GivenName a owl:Class,
        linkml:ClassDefinition ;
    rdfs:label "GivenName" ;
    rdfs:subClassOf [ a owl:Restriction ;
            owl:maxQualifiedCardinality 1 ;
            owl:onClass odm:ContentType ;
            owl:onProperty odm:_content ],
        [ a owl:Restriction ;
            owl:maxQualifiedCardinality 1 ;
            owl:onClass odm:String ;
            owl:onProperty odm:range ] ;
    skos:definition "The user's initial given name or all given names." ;
    skos:exactMatch odm:GivenName .

odm:HouseNumber a owl:Class,
        linkml:ClassDefinition ;
    rdfs:label "HouseNumber" ;
    rdfs:subClassOf [ a owl:Restriction ;
            owl:maxQualifiedCardinality 1 ;
            owl:onClass odm:String ;
            owl:onProperty odm:range ],
        [ a owl:Restriction ;
            owl:maxQualifiedCardinality 1 ;
            owl:onClass odm:ContentType ;
            owl:onProperty odm:_content ] ;
    skos:definition "The house number part of a user's postal address." ;
    skos:exactMatch odm:HouseNumber .

odm:Image a owl:Class,
        linkml:ClassDefinition ;
    rdfs:label "Image" ;
    rdfs:subClassOf [ a owl:Restriction ;
            owl:maxQualifiedCardinality 1 ;
            owl:onClass odm:FileName ;
            owl:onProperty odm:ImageFileName ],
        [ a owl:Restriction ;
            owl:maxQualifiedCardinality 1 ;
            owl:onClass odm:Text ;
            owl:onProperty odm:MimeType ],
        [ a owl:Restriction ;
            owl:maxQualifiedCardinality 1 ;
            owl:onClass odm:Text ;
            owl:onProperty odm:href ] ;
    skos:definition "A visual depiction of the user." ;
    skos:exactMatch odm:Image .

odm:ImplementationNotes a owl:Class,
        linkml:ClassDefinition ;
    rdfs:label "ImplementationNotes" ;
    rdfs:subClassOf [ a owl:Restriction ;
            owl:allValuesFrom odm:TranslatedText ;
            owl:onProperty odm:TranslatedTextRef ] ;
    skos:definition "Further information, such as rationale and implementation instructions, on how to implement the CRF data collection fields." ;
    skos:exactMatch odm:ImplementationNotes .

odm:Include a owl:Class,
        linkml:ClassDefinition ;
    rdfs:label "Include" ;
    rdfs:subClassOf [ a owl:Restriction ;
            owl:maxQualifiedCardinality 1 ;
            owl:onClass odm:Uriorcurie ;
            owl:onProperty odm:href ],
        [ a owl:Restriction ;
            owl:onClass odm:Oidref ;
            owl:onProperty odm:StudyOID ;
            owl:qualifiedCardinality 1 ],
        [ a owl:Restriction ;
            owl:onClass odm:Oidref ;
            owl:onProperty odm:MetaDataVersionOID ;
            owl:qualifiedCardinality 1 ] ;
    skos:definition "The Include metadata element allows a reference to a prior metadata version." ;
    skos:exactMatch odm:Include .

odm:InclusionCriteria a owl:Class,
        linkml:ClassDefinition ;
    rdfs:label "InclusionCriteria" ;
    rdfs:subClassOf [ a owl:Restriction ;
            owl:allValuesFrom odm:Criterion ;
            owl:onProperty odm:CriterionRef ] ;
    skos:definition "The InclusionCriteria is a container element for Criterion elements describing inclusion criteria for subjects in the study. When a list is provided, subjects must meet each of the criteria in the list in order to enroll in the study." ;
    skos:exactMatch odm:InclusionCriteria .

odm:InclusionExclusionCriteria a owl:Class,
        linkml:ClassDefinition ;
    rdfs:label "InclusionExclusionCriteria" ;
    rdfs:subClassOf [ a owl:Restriction ;
            owl:maxQualifiedCardinality 1 ;
            owl:onClass odm:InclusionCriteria ;
            owl:onProperty odm:InclusionCriteriaRef ],
        [ a owl:Restriction ;
            owl:maxQualifiedCardinality 1 ;
            owl:onClass odm:ExclusionCriteria ;
            owl:onProperty odm:ExclusionCriteriaRef ] ;
    skos:definition "The InclusionExclusionCriteria element can contain 2 lists of Criterion elements, represented by the 2 elements InclusionCriteria and ExclusionCriteria. Together, these criteria determine the eligibility of a subject for the study. The actual condition to be evaluated is contained in an ODM ConditionDef, which is referenced by each Criterion‟s ConditionOID attribute." ;
    skos:exactMatch odm:InclusionExclusionCriteria .

odm:IntercurrentEvent a owl:Class,
        linkml:ClassDefinition ;
    rdfs:label "IntercurrentEvent" ;
    rdfs:subClassOf [ a owl:Restriction ;
            owl:maxQualifiedCardinality 1 ;
            owl:onClass odm:Description ;
            owl:onProperty odm:DescriptionRef ] ;
    skos:exactMatch odm:IntercurrentEvent .

odm:InvestigatorRef a owl:Class,
        linkml:ClassDefinition ;
    rdfs:label "InvestigatorRef" ;
    rdfs:subClassOf [ a owl:Restriction ;
            owl:onClass odm:Oidref ;
            owl:onProperty odm:UserOID ;
            owl:qualifiedCardinality 1 ] ;
    skos:definition "Provides a reference to the user who created the SubjectData record in the source system." ;
    skos:exactMatch odm:InvestigatorRef .

odm:ItemData a owl:Class,
        linkml:ClassDefinition ;
    rdfs:label "ItemData" ;
    rdfs:subClassOf [ a owl:Restriction ;
            owl:maxQualifiedCardinality 1 ;
            owl:onClass odm:TransactionType ;
            owl:onProperty odm:TransactionTypeRef ],
        [ a owl:Restriction ;
            owl:allValuesFrom odm:Value ;
            owl:onProperty odm:ValueRef ],
        [ a owl:Restriction ;
            owl:maxQualifiedCardinality 1 ;
            owl:onClass odm:AuditRecord ;
            owl:onProperty odm:AuditRecordRef ],
        [ a owl:Restriction ;
            owl:onClass odm:Oidref ;
            owl:onProperty odm:ItemOID ;
            owl:qualifiedCardinality 1 ],
        [ a owl:Restriction ;
            owl:maxQualifiedCardinality 1 ;
            owl:onClass odm:YesOnly ;
            owl:onProperty odm:IsNull ],
        [ a owl:Restriction ;
            owl:maxQualifiedCardinality 1 ;
            owl:onClass odm:Annotation ;
            owl:onProperty odm:AnnotationRef ],
        [ a owl:Restriction ;
            owl:allValuesFrom odm:Query ;
            owl:onProperty odm:QueryRef ],
        [ a owl:Restriction ;
            owl:maxQualifiedCardinality 1 ;
            owl:onClass odm:Signature ;
            owl:onProperty odm:SignatureRefRef ] ;
    skos:definition "The ItemData element is used for transmission of the clinical data for an item. The model does not support repeating items within a single item group." ;
    skos:exactMatch odm:ItemData .

odm:ItemDef a owl:Class,
        linkml:ClassDefinition ;
    rdfs:label "ItemDef" ;
    rdfs:subClassOf [ a owl:Restriction ;
            owl:onClass odm:Name ;
            owl:onProperty odm:Name ;
            owl:qualifiedCardinality 1 ],
        [ a owl:Restriction ;
            owl:maxQualifiedCardinality 1 ;
            owl:onClass odm:Definition ;
            owl:onProperty odm:DefinitionRef ],
        [ a owl:Restriction ;
            owl:maxQualifiedCardinality 1 ;
            owl:onClass odm:ImplementationNotes ;
            owl:onProperty odm:ImplementationNotesRef ],
        [ a owl:Restriction ;
            owl:maxQualifiedCardinality 1 ;
            owl:onClass odm:Text ;
            owl:onProperty odm:DisplayFormat ],
        [ a owl:Restriction ;
            owl:maxQualifiedCardinality 1 ;
            owl:onClass odm:CDISCNotes ;
            owl:onProperty odm:CDISCNotesRef ],
        [ a owl:Restriction ;
            owl:maxQualifiedCardinality 1 ;
            owl:onClass odm:Description ;
            owl:onProperty odm:DescriptionRef ],
        [ a owl:Restriction ;
            owl:maxQualifiedCardinality 1 ;
            owl:onClass odm:Text ;
            owl:onProperty odm:VariableSet ],
        [ a owl:Restriction ;
            owl:maxQualifiedCardinality 1 ;
            owl:onClass odm:CRFCompletionInstructions ;
            owl:onProperty odm:CRFCompletionInstructionsRef ],
        [ a owl:Restriction ;
            owl:onClass odm:DataType ;
            owl:onProperty odm:DataTypeRef ;
            owl:qualifiedCardinality 1 ],
        [ a owl:Restriction ;
            owl:allValuesFrom odm:Alias ;
            owl:onProperty odm:AliasRef ],
        [ a owl:Restriction ;
            owl:maxQualifiedCardinality 1 ;
            owl:onClass odm:CodeListRef ;
            owl:onProperty odm:CodeListRefRef ],
        [ a owl:Restriction ;
            owl:maxQualifiedCardinality 1 ;
            owl:onClass odm:Prompt ;
            owl:onProperty odm:PromptRef ],
        [ a owl:Restriction ;
            owl:maxQualifiedCardinality 1 ;
            owl:onClass odm:Question ;
            owl:onProperty odm:QuestionRef ],
        [ a owl:Restriction ;
            owl:onClass odm:Oid ;
            owl:onProperty odm:OID ;
            owl:qualifiedCardinality 1 ],
        [ a owl:Restriction ;
            owl:maxQualifiedCardinality 1 ;
            owl:onClass odm:PositiveInteger ;
            owl:onProperty odm:Length ],
        [ a owl:Restriction ;
            owl:allValuesFrom odm:Coding ;
            owl:onProperty odm:CodingRef ],
        [ a owl:Restriction ;
            owl:maxQualifiedCardinality 1 ;
            owl:onClass odm:ValueListRef ;
            owl:onProperty odm:ValueListRefRef ],
        [ a owl:Restriction ;
            owl:allValuesFrom odm:RangeCheck ;
            owl:onProperty odm:RangeCheckRef ],
        [ a owl:Restriction ;
            owl:maxQualifiedCardinality 1 ;
            owl:onClass odm:Oidref ;
            owl:onProperty odm:CommentOID ] ;
    skos:definition "An ItemDef describes a type of item that can occur within a study. Item properties include name, datatype, range, or codelist restrictions, and several other properties." ;
    skos:exactMatch odm:ItemDef .

odm:ItemGroupDataRef a owl:ObjectProperty,
        linkml:SlotDefinition ;
    rdfs:label "ItemGroupDataRef" ;
    rdfs:range odm:ItemGroupData ;
    skos:definition "ItemGroupData reference: Clinical data corresponding to an ItemGroupRef defined in the active MetaDataVersion." .

odm:ItemGroupDef a owl:Class,
        linkml:ClassDefinition ;
    rdfs:label "ItemGroupDef" ;
    rdfs:subClassOf [ a owl:Restriction ;
            owl:maxQualifiedCardinality 1 ;
            owl:onClass odm:YesOnly ;
            owl:onProperty odm:IsNonStandard ],
        [ a owl:Restriction ;
            owl:maxQualifiedCardinality 1 ;
            owl:onClass odm:Oidref ;
            owl:onProperty odm:ArchiveLocationID ],
        [ a owl:Restriction ;
            owl:allValuesFrom odm:ItemGroupRef ;
            owl:onProperty odm:ItemGroupRefRef ],
        [ a owl:Restriction ;
            owl:maxQualifiedCardinality 1 ;
            owl:onClass odm:Text ;
            owl:onProperty odm:Purpose ],
        [ a owl:Restriction ;
            owl:onClass odm:ItemGroupRepeatingType ;
            owl:onProperty odm:Repeating ;
            owl:qualifiedCardinality 1 ],
        [ a owl:Restriction ;
            owl:maxQualifiedCardinality 1 ;
            owl:onClass odm:YesOrNo ;
            owl:onProperty odm:IsReferenceData ],
        [ a owl:Restriction ;
            owl:maxQualifiedCardinality 1 ;
            owl:onClass odm:Leaf ;
            owl:onProperty odm:LeafRef ],
        [ a owl:Restriction ;
            owl:maxQualifiedCardinality 1 ;
            owl:onClass odm:Name ;
            owl:onProperty odm:DatasetName ],
        [ a owl:Restriction ;
            owl:maxQualifiedCardinality 1 ;
            owl:onClass odm:WorkflowRef ;
            owl:onProperty odm:WorkflowRefRef ],
        [ a owl:Restriction ;
            owl:allValuesFrom odm:ItemRef ;
            owl:onProperty odm:ItemRefRef ],
        [ a owl:Restriction ;
            owl:maxQualifiedCardinality 1 ;
            owl:onClass odm:Oidref ;
            owl:onProperty odm:StandardOID ],
        [ a owl:Restriction ;
            owl:maxQualifiedCardinality 1 ;
            owl:onClass odm:PositiveInteger ;
            owl:onProperty odm:RepeatingLimit ],
        [ a owl:Restriction ;
            owl:allValuesFrom odm:Alias ;
            owl:onProperty odm:AliasRef ],
        [ a owl:Restriction ;
            owl:maxQualifiedCardinality 1 ;
            owl:onClass odm:YesOnly ;
            owl:onProperty odm:HasNoData ],
        [ a owl:Restriction ;
            owl:onClass odm:Oid ;
            owl:onProperty odm:OID ;
            owl:qualifiedCardinality 1 ],
        [ a owl:Restriction ;
            owl:allValuesFrom odm:Coding ;
            owl:onProperty odm:CodingRef ],
        [ a owl:Restriction ;
            owl:maxQualifiedCardinality 1 ;
            owl:onClass odm:Class ;
            owl:onProperty odm:ClassRef ],
        [ a owl:Restriction ;
            owl:maxQualifiedCardinality 1 ;
            owl:onClass odm:Text ;
            owl:onProperty odm:Domain ],
        [ a owl:Restriction ;
            owl:onClass odm:Name ;
            owl:onProperty odm:Name ;
            owl:qualifiedCardinality 1 ],
        [ a owl:Restriction ;
            owl:allValuesFrom odm:Origin ;
            owl:onProperty odm:OriginRef ],
        [ a owl:Restriction ;
            owl:onClass odm:ItemGroupTypeType ;
            owl:onProperty odm:Type ;
            owl:qualifiedCardinality 1 ],
        [ a owl:Restriction ;
            owl:maxQualifiedCardinality 1 ;
            owl:onClass odm:Oidref ;
            owl:onProperty odm:CommentOID ],
        [ a owl:Restriction ;
            owl:maxQualifiedCardinality 1 ;
            owl:onClass odm:Description ;
            owl:onProperty odm:DescriptionRef ],
        [ a owl:Restriction ;
            owl:maxQualifiedCardinality 1 ;
            owl:onClass odm:Text ;
            owl:onProperty odm:Structure ] ;
    skos:definition "An ItemGroupDef describes a type of variable or field grouping that can occur within a study." ;
    skos:exactMatch odm:ItemGroupDef .

odm:ItemGroupOID a owl:ObjectProperty,
        linkml:SlotDefinition ;
    rdfs:label "ItemGroupOID" ;
    rdfs:range odm:Oidref ;
    skos:definition "Reference to the ItemGroupDef ." .

odm:KeySet a owl:Class,
        linkml:ClassDefinition ;
    rdfs:label "KeySet" ;
    rdfs:subClassOf [ a owl:Restriction ;
            owl:maxQualifiedCardinality 1 ;
            owl:onClass odm:Oidref ;
            owl:onProperty odm:MetaDataVersionOID ],
        [ a owl:Restriction ;
            owl:maxQualifiedCardinality 1 ;
            owl:onClass odm:Oidref ;
            owl:onProperty odm:StudyEventOID ],
        [ a owl:Restriction ;
            owl:maxQualifiedCardinality 1 ;
            owl:onClass odm:RepeatKey ;
            owl:onProperty odm:ItemGroupRepeatKey ],
        [ a owl:Restriction ;
            owl:maxQualifiedCardinality 1 ;
            owl:onClass odm:RepeatKey ;
            owl:onProperty odm:StudyEventRepeatKey ],
        [ a owl:Restriction ;
            owl:onClass odm:Oidref ;
            owl:onProperty odm:StudyOID ;
            owl:qualifiedCardinality 1 ],
        [ a owl:Restriction ;
            owl:maxQualifiedCardinality 1 ;
            owl:onClass odm:SubjectKey ;
            owl:onProperty odm:SubjectKey ],
        [ a owl:Restriction ;
            owl:maxQualifiedCardinality 1 ;
            owl:onClass odm:Oidref ;
            owl:onProperty odm:ItemOID ],
        [ a owl:Restriction ;
            owl:maxQualifiedCardinality 1 ;
            owl:onClass odm:Oidref ;
            owl:onProperty odm:ItemGroupOID ] ;
    skos:definition "A KeySet references a single entity (e.g., a study, a subject, a study event). Only those attributes needed to specify the particular entity are required, and all others must be omitted (see Section 2.7, Clinical Data Keys)." ;
    skos:exactMatch odm:KeySet .

odm:LegalReason a owl:Class,
        linkml:ClassDefinition ;
    rdfs:label "LegalReason" ;
    rdfs:subClassOf [ a owl:Restriction ;
            owl:maxQualifiedCardinality 1 ;
            owl:onClass odm:String ;
            owl:onProperty odm:range ],
        [ a owl:Restriction ;
            owl:maxQualifiedCardinality 1 ;
            owl:onClass odm:ContentType ;
            owl:onProperty odm:_content ] ;
    skos:definition "The responsibility statement associated with a signature (e.g., \"The signer accepts responsibility for the accuracy of this data.\")." ;
    skos:exactMatch odm:LegalReason .

odm:LocationOID a owl:ObjectProperty,
        linkml:SlotDefinition ;
    rdfs:label "LocationOID" ;
    rdfs:range odm:Oidref ;
    skos:definition "Reference to a Location element." .

odm:Mandatory a owl:ObjectProperty,
        linkml:SlotDefinition ;
    rdfs:label "Mandatory" ;
    rdfs:range odm:YesOrNo ;
    skos:definition "Indicator of whether this StudyEventGroup must appear in the study clinical data for each subject per the study protocol." .

odm:Meaning a owl:Class,
        linkml:ClassDefinition ;
    rdfs:label "Meaning" ;
    rdfs:subClassOf [ a owl:Restriction ;
            owl:maxQualifiedCardinality 1 ;
            owl:onClass odm:ContentType ;
            owl:onProperty odm:_content ],
        [ a owl:Restriction ;
            owl:maxQualifiedCardinality 1 ;
            owl:onClass odm:String ;
            owl:onProperty odm:range ] ;
    skos:definition "A short name or description for this signature. It should reflect the context of the signature and/or the text that appears when the signature is applied in the user interface." ;
    skos:exactMatch odm:Meaning .

odm:MetaDataVersionRef a owl:Class,
        linkml:ClassDefinition ;
    rdfs:label "MetaDataVersionRef" ;
    rdfs:subClassOf [ a owl:Restriction ;
            owl:onClass odm:Oidref ;
            owl:onProperty odm:StudyOID ;
            owl:qualifiedCardinality 1 ],
        [ a owl:Restriction ;
            owl:onClass odm:Oidref ;
            owl:onProperty odm:MetaDataVersionOID ;
            owl:qualifiedCardinality 1 ],
        [ a owl:Restriction ;
            owl:onClass odm:Date ;
            owl:onProperty odm:EffectiveDate ;
            owl:qualifiedCardinality 1 ] ;
    skos:definition "A reference to a MetaDataVersion used at the containing Location. The EffectiveDate reflects the possibility that the metadata may change over the course of the study." ;
    skos:exactMatch odm:MetaDataVersionRef .

odm:MethodDef a owl:Class,
        linkml:ClassDefinition ;
    rdfs:label "MethodDef" ;
    rdfs:subClassOf [ a owl:Restriction ;
            owl:allValuesFrom odm:FormalExpression ;
            owl:onProperty odm:FormalExpressionRef ],
        [ a owl:Restriction ;
            owl:maxQualifiedCardinality 1 ;
            owl:onClass odm:Oidref ;
            owl:onProperty odm:CommentOID ],
        [ a owl:Restriction ;
            owl:maxQualifiedCardinality 1 ;
            owl:onClass odm:MethodType ;
            owl:onProperty odm:Type ],
        [ a owl:Restriction ;
            owl:onClass odm:Name ;
            owl:onProperty odm:Name ;
            owl:qualifiedCardinality 1 ],
        [ a owl:Restriction ;
            owl:onClass odm:Oid ;
            owl:onProperty odm:OID ;
            owl:qualifiedCardinality 1 ],
        [ a owl:Restriction ;
            owl:allValuesFrom odm:DocumentRef ;
            owl:onProperty odm:DocumentRefRef ],
        [ a owl:Restriction ;
            owl:maxQualifiedCardinality 1 ;
            owl:onClass odm:Description ;
            owl:onProperty odm:DescriptionRef ],
        [ a owl:Restriction ;
            owl:allValuesFrom odm:Alias ;
            owl:onProperty odm:AliasRef ],
        [ a owl:Restriction ;
            owl:maxQualifiedCardinality 1 ;
            owl:onClass odm:MethodSignature ;
            owl:onProperty odm:MethodSignatureRef ] ;
    skos:definition "A MethodDef defines how a data value can be obtained from a collection of other data values." ;
    skos:exactMatch odm:MethodDef .

odm:Organization a owl:Class,
        linkml:ClassDefinition ;
    rdfs:label "Organization" ;
    rdfs:subClassOf [ a owl:Restriction ;
            owl:maxQualifiedCardinality 1 ;
            owl:onClass odm:Text ;
            owl:onProperty odm:Role ],
        [ a owl:Restriction ;
            owl:maxQualifiedCardinality 1 ;
            owl:onClass odm:Oidref ;
            owl:onProperty odm:PartOfOrganizationOID ],
        [ a owl:Restriction ;
            owl:onClass odm:Oid ;
            owl:onProperty odm:OID ;
            owl:qualifiedCardinality 1 ],
        [ a owl:Restriction ;
            owl:onClass odm:Name ;
            owl:onProperty odm:Name ;
            owl:qualifiedCardinality 1 ],
        [ a owl:Restriction ;
            owl:maxQualifiedCardinality 1 ;
            owl:onClass odm:Description ;
            owl:onProperty odm:DescriptionRef ],
        [ a owl:Restriction ;
            owl:onClass odm:OrganizationType ;
            owl:onProperty odm:Type ;
            owl:qualifiedCardinality 1 ],
        [ a owl:Restriction ;
            owl:allValuesFrom odm:Address ;
            owl:onProperty odm:AddressRef ],
        [ a owl:Restriction ;
            owl:allValuesFrom odm:Telecom ;
            owl:onProperty odm:TelecomRef ],
        [ a owl:Restriction ;
            owl:maxQualifiedCardinality 1 ;
            owl:onClass odm:Oidref ;
            owl:onProperty odm:LocationOID ] ;
    skos:definition "An organization can reference a parent organization. Users may be associated with an Organization. An Organization may be associated with a Location. A User, Location, or Organization may have an address." ;
    skos:exactMatch odm:Organization .

odm:OtherText a owl:Class,
        linkml:ClassDefinition ;
    rdfs:label "OtherText" ;
    rdfs:subClassOf [ a owl:Restriction ;
            owl:maxQualifiedCardinality 1 ;
            owl:onClass odm:String ;
            owl:onProperty odm:range ],
        [ a owl:Restriction ;
            owl:maxQualifiedCardinality 1 ;
            owl:onClass odm:ContentType ;
            owl:onProperty odm:_content ] ;
    skos:definition "Any other text needed as part of a user's postal address." ;
    skos:exactMatch odm:OtherText .

odm:PDFPageRef a owl:Class,
        linkml:ClassDefinition ;
    rdfs:label "PDFPageRef" ;
    rdfs:subClassOf [ a owl:Restriction ;
            owl:maxQualifiedCardinality 1 ;
            owl:onClass odm:PositiveInteger ;
            owl:onProperty odm:FirstPage ],
        [ a owl:Restriction ;
            owl:onClass odm:PDFPageType ;
            owl:onProperty odm:Type ;
            owl:qualifiedCardinality 1 ],
        [ a owl:Restriction ;
            owl:maxQualifiedCardinality 1 ;
            owl:onClass odm:Text ;
            owl:onProperty odm:Title ],
        [ a owl:Restriction ;
            owl:maxQualifiedCardinality 1 ;
            owl:onClass odm:Text ;
            owl:onProperty odm:PageRefs ],
        [ a owl:Restriction ;
            owl:maxQualifiedCardinality 1 ;
            owl:onClass odm:PositiveInteger ;
            owl:onProperty odm:LastPage ] ;
    skos:definition "This element is the container for CRF page references." ;
    skos:exactMatch odm:PDFPageRef .

odm:Parameter a owl:Class,
        linkml:ClassDefinition ;
    rdfs:label "Parameter" ;
    rdfs:subClassOf [ a owl:Restriction ;
            owl:onClass odm:Name ;
            owl:onProperty odm:Name ;
            owl:qualifiedCardinality 1 ],
        [ a owl:Restriction ;
            owl:maxQualifiedCardinality 1 ;
            owl:onClass odm:PositiveInteger ;
            owl:onProperty odm:OrderNumber ],
        [ a owl:Restriction ;
            owl:maxQualifiedCardinality 1 ;
            owl:onClass odm:Text ;
            owl:onProperty odm:DefinitionRef ],
        [ a owl:Restriction ;
            owl:onClass odm:DataType ;
            owl:onProperty odm:DataTypeRef ;
            owl:qualifiedCardinality 1 ] ;
    skos:definition "The Parameter element represents a method parameter used as part of a MethodSignature in MethodDef, ConditionDef, or RangeCheck." ;
    skos:exactMatch odm:Parameter .

odm:ParameterValue a owl:Class,
        linkml:ClassDefinition ;
    rdfs:label "ParameterValue" ;
    rdfs:subClassOf [ a owl:Restriction ;
            owl:onClass odm:Text ;
            owl:onProperty odm:ValueRef ;
            owl:qualifiedCardinality 1 ],
        [ a owl:Restriction ;
            owl:allValuesFrom odm:Coding ;
            owl:onProperty odm:CodingRef ] ;
    skos:definition "This element contains the value of the study parameter as text content." ;
    skos:exactMatch odm:ParameterValue .

odm:PostalCode a owl:Class,
        linkml:ClassDefinition ;
    rdfs:label "PostalCode" ;
    rdfs:subClassOf [ a owl:Restriction ;
            owl:maxQualifiedCardinality 1 ;
            owl:onClass odm:ContentType ;
            owl:onProperty odm:_content ],
        [ a owl:Restriction ;
            owl:maxQualifiedCardinality 1 ;
            owl:onClass odm:String ;
            owl:onProperty odm:range ] ;
    skos:definition "The postal code part of a user's postal address." ;
    skos:exactMatch odm:PostalCode .

odm:Prefix a owl:Class,
        linkml:ClassDefinition ;
    rdfs:label "Prefix" ;
    rdfs:subClassOf [ a owl:Restriction ;
            owl:maxQualifiedCardinality 1 ;
            owl:onClass odm:ContentType ;
            owl:onProperty odm:_content ],
        [ a owl:Restriction ;
            owl:maxQualifiedCardinality 1 ;
            owl:onClass odm:String ;
            owl:onProperty odm:range ] ;
    skos:definition "Title or other prefix. Maps to FHIR HumanName.prefix (https://www.hl7.org/fhir/datatypes.html#humanname)." ;
    skos:exactMatch odm:Prefix .

odm:Prompt a owl:Class,
        linkml:ClassDefinition ;
    rdfs:label "Prompt" ;
    rdfs:subClassOf [ a owl:Restriction ;
            owl:allValuesFrom odm:TranslatedText ;
            owl:onProperty odm:TranslatedTextRef ] ;
    skos:definition "A prompt text shown to a human user when prompted to provide data for an item on paper or on a screen. The Prompt is a short version of the question." ;
    skos:exactMatch odm:Prompt .

odm:Protocol a owl:Class,
        linkml:ClassDefinition ;
    rdfs:label "Protocol" ;
    rdfs:subClassOf [ a owl:Restriction ;
            owl:maxQualifiedCardinality 1 ;
            owl:onClass odm:StudyEndPoints ;
            owl:onProperty odm:StudyEndPointsRef ],
        [ a owl:Restriction ;
            owl:maxQualifiedCardinality 1 ;
            owl:onClass odm:WorkflowRef ;
            owl:onProperty odm:WorkflowRefRef ],
        [ a owl:Restriction ;
            owl:maxQualifiedCardinality 1 ;
            owl:onClass odm:StudyStructure ;
            owl:onProperty odm:StudyStructureRef ],
        [ a owl:Restriction ;
            owl:maxQualifiedCardinality 1 ;
            owl:onClass odm:StudyIndications ;
            owl:onProperty odm:StudyIndicationsRef ],
        [ a owl:Restriction ;
            owl:allValuesFrom odm:Alias ;
            owl:onProperty odm:AliasRef ],
        [ a owl:Restriction ;
            owl:maxQualifiedCardinality 1 ;
            owl:onClass odm:StudyInterventions ;
            owl:onProperty odm:StudyInterventionsRef ],
        [ a owl:Restriction ;
            owl:maxQualifiedCardinality 1 ;
            owl:onClass odm:StudySummary ;
            owl:onProperty odm:StudySummaryRef ],
        [ a owl:Restriction ;
            owl:allValuesFrom odm:StudyEventGroupRef ;
            owl:onProperty odm:StudyEventGroupRefRef ],
        [ a owl:Restriction ;
            owl:maxQualifiedCardinality 1 ;
            owl:onClass odm:Description ;
            owl:onProperty odm:DescriptionRef ],
        [ a owl:Restriction ;
            owl:maxQualifiedCardinality 1 ;
            owl:onClass odm:TrialPhase ;
            owl:onProperty odm:TrialPhaseRef ],
        [ a owl:Restriction ;
            owl:maxQualifiedCardinality 1 ;
            owl:onClass odm:StudyEstimands ;
            owl:onProperty odm:StudyEstimandsRef ],
        [ a owl:Restriction ;
            owl:maxQualifiedCardinality 1 ;
            owl:onClass odm:StudyTimings ;
            owl:onProperty odm:StudyTimingsRef ],
        [ a owl:Restriction ;
            owl:maxQualifiedCardinality 1 ;
            owl:onClass odm:InclusionExclusionCriteria ;
            owl:onProperty odm:InclusionExclusionCriteriaRef ],
        [ a owl:Restriction ;
            owl:maxQualifiedCardinality 1 ;
            owl:onClass odm:StudyObjectives ;
            owl:onProperty odm:StudyObjectivesRef ],
        [ a owl:Restriction ;
            owl:maxQualifiedCardinality 1 ;
            owl:onClass odm:StudyTargetPopulation ;
            owl:onProperty odm:StudyTargetPopulationRefRef ] ;
    skos:definition "The Protocol element lists the kinds of study events that can occur within a specific version of a study. All clinical data must occur within one of these study events." ;
    skos:exactMatch odm:Protocol .

odm:Question a owl:Class,
        linkml:ClassDefinition ;
    rdfs:label "Question" ;
    rdfs:subClassOf [ a owl:Restriction ;
            owl:allValuesFrom odm:TranslatedText ;
            owl:onProperty odm:TranslatedTextRef ] ;
    skos:definition "A label shown to a human user when prompted to provide data for an item on paper or on a screen." ;
    skos:exactMatch odm:Question .

odm:ReasonForChange a owl:Class,
        linkml:ClassDefinition ;
    rdfs:label "ReasonForChange" ;
    rdfs:subClassOf [ a owl:Restriction ;
            owl:maxQualifiedCardinality 1 ;
            owl:onClass odm:ContentType ;
            owl:onProperty odm:_content ],
        [ a owl:Restriction ;
            owl:maxQualifiedCardinality 1 ;
            owl:onClass odm:String ;
            owl:onProperty odm:range ] ;
    skos:definition "A user-supplied reason for a data change." ;
    skos:exactMatch odm:ReasonForChange .

odm:ReferenceData a owl:Class,
        linkml:ClassDefinition ;
    rdfs:label "ReferenceData" ;
    rdfs:subClassOf [ a owl:Restriction ;
            owl:onClass odm:Oidref ;
            owl:onProperty odm:StudyOID ;
            owl:qualifiedCardinality 1 ],
        [ a owl:Restriction ;
            owl:maxQualifiedCardinality 1 ;
            owl:onClass odm:AuditRecord ;
            owl:onProperty odm:AuditRecordRef ],
        [ a owl:Restriction ;
            owl:maxQualifiedCardinality 1 ;
            owl:onClass odm:Signature ;
            owl:onProperty odm:SignatureRefRef ],
        [ a owl:Restriction ;
            owl:allValuesFrom odm:ItemGroupData ;
            owl:onProperty odm:ItemGroupDataRef ],
        [ a owl:Restriction ;
            owl:maxQualifiedCardinality 1 ;
            owl:onClass odm:Annotation ;
            owl:onProperty odm:AnnotationRef ],
        [ a owl:Restriction ;
            owl:onClass odm:Oidref ;
            owl:onProperty odm:MetaDataVersionOID ;
            owl:qualifiedCardinality 1 ] ;
    skos:definition "Reference data provides information on how to interpret clinical data. For example, reference data might include lab normal ranges. For a study that uses CDISC standards, reference data might include SDTM Trial Design datasets." ;
    skos:exactMatch odm:ReferenceData .

odm:RelativeTimingConstraint a owl:Class,
        linkml:ClassDefinition ;
    rdfs:label "RelativeTimingConstraint" ;
    rdfs:subClassOf [ a owl:Restriction ;
            owl:maxQualifiedCardinality 1 ;
            owl:onClass odm:Description ;
            owl:onProperty odm:DescriptionRef ],
        [ a owl:Restriction ;
            owl:onClass odm:Name ;
            owl:onProperty odm:Name ;
            owl:qualifiedCardinality 1 ],
        [ a owl:Restriction ;
            owl:onClass odm:Oid ;
            owl:onProperty odm:OID ;
            owl:qualifiedCardinality 1 ],
        [ a owl:Restriction ;
            owl:maxQualifiedCardinality 1 ;
            owl:onClass odm:DurationDatetime ;
            owl:onProperty odm:TimepointPreWindow ],
        [ a owl:Restriction ;
            owl:maxQualifiedCardinality 1 ;
            owl:onClass odm:Oidref ;
            owl:onProperty odm:PredecessorOID ],
        [ a owl:Restriction ;
            owl:maxQualifiedCardinality 1 ;
            owl:onClass odm:Oidref ;
            owl:onProperty odm:SuccessorOID ],
        [ a owl:Restriction ;
            owl:maxQualifiedCardinality 1 ;
            owl:onClass odm:RelativeTimingConstraintType ;
            owl:onProperty odm:Type ],
        [ a owl:Restriction ;
            owl:maxQualifiedCardinality 1 ;
            owl:onClass odm:DurationDatetime ;
            owl:onProperty odm:TimepointPostWindow ],
        [ a owl:Restriction ;
            owl:onClass odm:DurationDatetime ;
            owl:onProperty odm:TimepointRelativeTarget ;
            owl:qualifiedCardinality 1 ] ;
    skos:definition "The RelativeTimingConstraint element describes a relative timing constraint between 2 activities or groups of activities, represented by StudyEventGroups, StudyEvents, ItemGroups, or Items." ;
    skos:exactMatch odm:RelativeTimingConstraint .

odm:Resource a owl:Class,
        linkml:ClassDefinition ;
    rdfs:label "Resource" ;
    rdfs:subClassOf [ a owl:Restriction ;
            owl:allValuesFrom odm:Selection ;
            owl:onProperty odm:SelectionRef ],
        [ a owl:Restriction ;
            owl:onClass odm:Text ;
            owl:onProperty odm:Type ;
            owl:qualifiedCardinality 1 ],
        [ a owl:Restriction ;
            owl:maxQualifiedCardinality 1 ;
            owl:onClass odm:Text ;
            owl:onProperty odm:Attribute ],
        [ a owl:Restriction ;
            owl:onClass odm:Name ;
            owl:onProperty odm:Name ;
            owl:qualifiedCardinality 1 ],
        [ a owl:Restriction ;
            owl:maxQualifiedCardinality 1 ;
            owl:onClass odm:Text ;
            owl:onProperty odm:Label ] ;
    skos:definition "Describes an external resource used as the source for the parent ItemGroup or Item." ;
    skos:exactMatch odm:Resource .

odm:ReturnValue a owl:Class,
        linkml:ClassDefinition ;
    rdfs:label "ReturnValue" ;
    rdfs:subClassOf [ a owl:Restriction ;
            owl:maxQualifiedCardinality 1 ;
            owl:onClass odm:Text ;
            owl:onProperty odm:DefinitionRef ],
        [ a owl:Restriction ;
            owl:onClass odm:DataType ;
            owl:onProperty odm:DataTypeRef ;
            owl:qualifiedCardinality 1 ],
        [ a owl:Restriction ;
            owl:onClass odm:Name ;
            owl:onProperty odm:Name ;
            owl:qualifiedCardinality 1 ],
        [ a owl:Restriction ;
            owl:maxQualifiedCardinality 1 ;
            owl:onClass odm:PositiveInteger ;
            owl:onProperty odm:OrderNumber ] ;
    skos:definition "The ReturnValue element represents a return value used as part of a MethodSignature in MethodDef, ConditionDef, or RangeCheck. A return value identifies values passed from the Method to the calling element. A ReturnValue may be computed by a FormalExpression." ;
    skos:exactMatch odm:ReturnValue .

odm:Selection a owl:Class,
        linkml:ClassDefinition ;
    rdfs:label "Selection" ;
    rdfs:subClassOf [ a owl:Restriction ;
            owl:onClass odm:Text ;
            owl:onProperty odm:Path ;
            owl:qualifiedCardinality 1 ] ;
    skos:definition "Template for machine-readable/executable expression for retrieving the data or information from an external resource." ;
    skos:exactMatch odm:Selection .

odm:SignMethod a owl:Class,
        linkml:EnumDefinition ;
    rdfs:label "SignMethod" ;
    owl:unionOf ( <http://www.cdisc.org/ns/odm/v2.0/SignMethod#Digital> <http://www.cdisc.org/ns/odm/v2.0/SignMethod#Electronic> ) ;
    linkml:permissible_values <http://www.cdisc.org/ns/odm/v2.0/SignMethod#Digital>,
        <http://www.cdisc.org/ns/odm/v2.0/SignMethod#Electronic> .

odm:SignatureDef a owl:Class,
        linkml:ClassDefinition ;
    rdfs:label "SignatureDef" ;
    rdfs:subClassOf [ a owl:Restriction ;
            owl:maxQualifiedCardinality 1 ;
            owl:onClass odm:SignMethod ;
            owl:onProperty odm:Methodology ],
        [ a owl:Restriction ;
            owl:maxQualifiedCardinality 1 ;
            owl:onClass odm:Meaning ;
            owl:onProperty odm:MeaningRef ],
        [ a owl:Restriction ;
            owl:maxQualifiedCardinality 1 ;
            owl:onClass odm:LegalReason ;
            owl:onProperty odm:LegalReasonRef ],
        [ a owl:Restriction ;
            owl:onClass odm:Oid ;
            owl:onProperty odm:OID ;
            owl:qualifiedCardinality 1 ] ;
    skos:definition "Provides Metadata for signatures included in the /ODM/ClinicalData." ;
    skos:exactMatch odm:SignatureDef .

odm:SignatureRef a owl:Class,
        linkml:ClassDefinition ;
    rdfs:label "SignatureRef" ;
    rdfs:subClassOf [ a owl:Restriction ;
            owl:onClass odm:Oidref ;
            owl:onProperty odm:SignatureOID ;
            owl:qualifiedCardinality 1 ] ;
    skos:exactMatch odm:SignatureRef .

odm:SiteRef a owl:Class,
        linkml:ClassDefinition ;
    rdfs:label "SiteRef" ;
    rdfs:subClassOf [ a owl:Restriction ;
            owl:onClass odm:Oidref ;
            owl:onProperty odm:LocationOID ;
            owl:qualifiedCardinality 1 ] ;
    skos:definition "lement NameSiteRefParent ElementsSubjectDataElement XPath(s)/ODM/ClinicalData/SubjectData/SiteRefElement Textual ValueNoneAttributesLocationOIDChild ElementsNoneUsage/Business RulesBusiness Rule(s):Must be provided when the /ODM/FileType is Transactional." ;
    skos:exactMatch odm:SiteRef .

odm:SoftOrHard a owl:Class,
        linkml:EnumDefinition ;
    rdfs:label "SoftOrHard" ;
    owl:unionOf ( <http://www.cdisc.org/ns/odm/v2.0/SoftOrHard#Soft> <http://www.cdisc.org/ns/odm/v2.0/SoftOrHard#Hard> ) ;
    linkml:permissible_values <http://www.cdisc.org/ns/odm/v2.0/SoftOrHard#Hard>,
        <http://www.cdisc.org/ns/odm/v2.0/SoftOrHard#Soft> .

odm:SourceID a owl:Class,
        linkml:ClassDefinition ;
    rdfs:label "SourceID" ;
    rdfs:subClassOf [ a owl:Restriction ;
            owl:maxQualifiedCardinality 1 ;
            owl:onClass odm:String ;
            owl:onProperty odm:range ],
        [ a owl:Restriction ;
            owl:maxQualifiedCardinality 1 ;
            owl:onClass odm:ContentType ;
            owl:onProperty odm:_content ] ;
    skos:definition "Information that identifies the source of the data within an originating system." ;
    skos:exactMatch odm:SourceID .

odm:SourceItem a owl:Class,
        linkml:ClassDefinition ;
    rdfs:label "SourceItem" ;
    rdfs:subClassOf [ a owl:Restriction ;
            owl:onClass odm:Oidref ;
            owl:onProperty odm:leafID ;
            owl:qualifiedCardinality 1 ],
        [ a owl:Restriction ;
            owl:maxQualifiedCardinality 1 ;
            owl:onClass odm:Oidref ;
            owl:onProperty odm:ItemOID ],
        [ a owl:Restriction ;
            owl:maxQualifiedCardinality 1 ;
            owl:onClass odm:Oidref ;
            owl:onProperty odm:ItemGroupOID ],
        [ a owl:Restriction ;
            owl:maxQualifiedCardinality 1 ;
            owl:onClass odm:Oidref ;
            owl:onProperty odm:StudyOID ],
        [ a owl:Restriction ;
            owl:allValuesFrom odm:Coding ;
            owl:onProperty odm:CodingRef ],
        [ a owl:Restriction ;
            owl:maxQualifiedCardinality 1 ;
            owl:onClass odm:Oidref ;
            owl:onProperty odm:MetaDataVersionOID ],
        [ a owl:Restriction ;
            owl:allValuesFrom odm:Resource ;
            owl:onProperty odm:ResourceRef ],
        [ a owl:Restriction ;
            owl:maxQualifiedCardinality 1 ;
            owl:onClass odm:Name ;
            owl:onProperty odm:Name ] ;
    skos:definition "Provides the information needed to identify the source metadata." ;
    skos:exactMatch odm:SourceItem .

odm:SourceItems a owl:Class,
        linkml:ClassDefinition ;
    rdfs:label "SourceItems" ;
    rdfs:subClassOf [ a owl:Restriction ;
            owl:allValuesFrom odm:Coding ;
            owl:onProperty odm:CodingRef ],
        [ a owl:Restriction ;
            owl:allValuesFrom odm:SourceItem ;
            owl:onProperty odm:SourceItemRef ] ;
    skos:definition "Identifies source items as needed to support automated data capture and end-to-end traceability." ;
    skos:exactMatch odm:SourceItems .

odm:Standard a owl:Class,
        linkml:ClassDefinition ;
    rdfs:label "Standard" ;
    rdfs:subClassOf [ a owl:Restriction ;
            owl:maxQualifiedCardinality 1 ;
            owl:onClass odm:Oidref ;
            owl:onProperty odm:CommentOID ],
        [ a owl:Restriction ;
            owl:onClass odm:StandardType ;
            owl:onProperty odm:Type ;
            owl:qualifiedCardinality 1 ],
        [ a owl:Restriction ;
            owl:maxQualifiedCardinality 1 ;
            owl:onClass odm:StandardPublishingSet ;
            owl:onProperty odm:PublishingSet ],
        [ a owl:Restriction ;
            owl:onClass odm:StandardStatus ;
            owl:onProperty odm:Status ;
            owl:qualifiedCardinality 1 ],
        [ a owl:Restriction ;
            owl:onClass odm:Oid ;
            owl:onProperty odm:OID ;
            owl:qualifiedCardinality 1 ],
        [ a owl:Restriction ;
            owl:onClass odm:StandardName ;
            owl:onProperty odm:Name ;
            owl:qualifiedCardinality 1 ],
        [ a owl:Restriction ;
            owl:onClass odm:Text ;
            owl:onProperty odm:Version ;
            owl:qualifiedCardinality 1 ] ;
    skos:definition "The Standard element describes each standard used within the MetaDataVersion element." ;
    skos:exactMatch odm:Standard .

odm:Standards a owl:Class,
        linkml:ClassDefinition ;
    rdfs:label "Standards" ;
    rdfs:subClassOf [ a owl:Restriction ;
            owl:allValuesFrom odm:Standard ;
            owl:onProperty odm:StandardRef ] ;
    skos:definition "The Standards element provides a container for the list of Standard elements referenced in the MetaDataVersion for the Study.." ;
    skos:exactMatch odm:Standards .

odm:StateProv a owl:Class,
        linkml:ClassDefinition ;
    rdfs:label "StateProv" ;
    rdfs:subClassOf [ a owl:Restriction ;
            owl:maxQualifiedCardinality 1 ;
            owl:onClass odm:String ;
            owl:onProperty odm:range ],
        [ a owl:Restriction ;
            owl:maxQualifiedCardinality 1 ;
            owl:onClass odm:ContentType ;
            owl:onProperty odm:_content ] ;
    skos:definition "The state or province name part of a user's postal address." ;
    skos:exactMatch odm:StateProv .

odm:StreetName a owl:Class,
        linkml:ClassDefinition ;
    rdfs:label "StreetName" ;
    rdfs:subClassOf [ a owl:Restriction ;
            owl:maxQualifiedCardinality 1 ;
            owl:onClass odm:ContentType ;
            owl:onProperty odm:_content ],
        [ a owl:Restriction ;
            owl:maxQualifiedCardinality 1 ;
            owl:onClass odm:String ;
            owl:onProperty odm:range ] ;
    skos:definition "The street name part of a user's postal address." ;
    skos:exactMatch odm:StreetName .

odm:Study a owl:Class,
        linkml:ClassDefinition ;
    rdfs:label "Study" ;
    rdfs:subClassOf [ a owl:Restriction ;
            owl:maxQualifiedCardinality 1 ;
            owl:onClass odm:Name ;
            owl:onProperty odm:Status ],
        [ a owl:Restriction ;
            owl:maxQualifiedCardinality 1 ;
            owl:onClass odm:Name ;
            owl:onProperty odm:VersionID ],
        [ a owl:Restriction ;
            owl:maxQualifiedCardinality 1 ;
            owl:onClass odm:Name ;
            owl:onProperty odm:VersionName ],
        [ a owl:Restriction ;
            owl:allValuesFrom odm:MetaDataVersion ;
            owl:onProperty odm:MetaDataVersionRefRef ],
        [ a owl:Restriction ;
            owl:onClass odm:Name ;
            owl:onProperty odm:StudyName ;
            owl:qualifiedCardinality 1 ],
        [ a owl:Restriction ;
            owl:onClass odm:Name ;
            owl:onProperty odm:ProtocolName ;
            owl:qualifiedCardinality 1 ],
        [ a owl:Restriction ;
            owl:maxQualifiedCardinality 1 ;
            owl:onClass odm:Description ;
            owl:onProperty odm:DescriptionRef ],
        [ a owl:Restriction ;
            owl:onClass odm:Oid ;
            owl:onProperty odm:OID ;
            owl:qualifiedCardinality 1 ] ;
    skos:definition "This element collects static structural information about an individual study." ;
    skos:exactMatch odm:Study .

odm:StudyEndPoints a owl:Class,
        linkml:ClassDefinition ;
    rdfs:label "StudyEndPoints" ;
    rdfs:subClassOf [ a owl:Restriction ;
            owl:allValuesFrom odm:StudyEndPoint ;
            owl:onProperty odm:StudyEndPointRefRef ] ;
    skos:definition "Go to start of metadata" ;
    skos:exactMatch odm:StudyEndPoints .

odm:StudyEstimand a owl:Class,
        linkml:ClassDefinition ;
    rdfs:label "StudyEstimand" ;
    rdfs:subClassOf [ a owl:Restriction ;
            owl:onClass odm:Name ;
            owl:onProperty odm:Name ;
            owl:qualifiedCardinality 1 ],
        [ a owl:Restriction ;
            owl:maxQualifiedCardinality 1 ;
            owl:onClass odm:StudyTargetPopulationRef ;
            owl:onProperty odm:StudyTargetPopulationRefRef ],
        [ a owl:Restriction ;
            owl:maxQualifiedCardinality 1 ;
            owl:onClass odm:StudyInterventionRef ;
            owl:onProperty odm:StudyInterventionRefRef ],
        [ a owl:Restriction ;
            owl:allValuesFrom odm:IntercurrentEvent ;
            owl:onProperty odm:IntercurrentEventRef ],
        [ a owl:Restriction ;
            owl:maxQualifiedCardinality 1 ;
            owl:onClass odm:StudyEstimandLevel ;
            owl:onProperty odm:Level ],
        [ a owl:Restriction ;
            owl:onClass odm:Oid ;
            owl:onProperty odm:OID ;
            owl:qualifiedCardinality 1 ],
        [ a owl:Restriction ;
            owl:maxQualifiedCardinality 1 ;
            owl:onClass odm:Description ;
            owl:onProperty odm:DescriptionRef ],
        [ a owl:Restriction ;
            owl:maxQualifiedCardinality 1 ;
            owl:onClass odm:SummaryMeasure ;
            owl:onProperty odm:SummaryMeasureRef ],
        [ a owl:Restriction ;
            owl:maxQualifiedCardinality 1 ;
            owl:onClass odm:StudyEndPointRef ;
            owl:onProperty odm:StudyEndPointRefRef ] ;
    skos:exactMatch odm:StudyEstimand .

odm:StudyEstimands a owl:Class,
        linkml:ClassDefinition ;
    rdfs:label "StudyEstimands" ;
    rdfs:subClassOf [ a owl:Restriction ;
            owl:allValuesFrom odm:StudyEstimand ;
            owl:onProperty odm:StudyEstimandRef ] ;
    skos:exactMatch odm:StudyEstimands .

odm:StudyEventData a owl:Class,
        linkml:ClassDefinition ;
    rdfs:label "StudyEventData" ;
    rdfs:subClassOf [ a owl:Restriction ;
            owl:maxQualifiedCardinality 1 ;
            owl:onClass odm:Signature ;
            owl:onProperty odm:SignatureRefRef ],
        [ a owl:Restriction ;
            owl:maxQualifiedCardinality 1 ;
            owl:onClass odm:Annotation ;
            owl:onProperty odm:AnnotationRef ],
        [ a owl:Restriction ;
            owl:allValuesFrom odm:ItemGroupData ;
            owl:onProperty odm:ItemGroupDataRef ],
        [ a owl:Restriction ;
            owl:maxQualifiedCardinality 1 ;
            owl:onClass odm:RepeatKey ;
            owl:onProperty odm:StudyEventRepeatKey ],
        [ a owl:Restriction ;
            owl:onClass odm:Oidref ;
            owl:onProperty odm:StudyEventOID ;
            owl:qualifiedCardinality 1 ],
        [ a owl:Restriction ;
            owl:allValuesFrom odm:Query ;
            owl:onProperty odm:QueryRef ],
        [ a owl:Restriction ;
            owl:maxQualifiedCardinality 1 ;
            owl:onClass odm:AuditRecord ;
            owl:onProperty odm:AuditRecordRef ],
        [ a owl:Restriction ;
            owl:maxQualifiedCardinality 1 ;
            owl:onClass odm:TransactionType ;
            owl:onProperty odm:TransactionTypeRef ] ;
    skos:definition "Clinical data for a study event (visit). The model supports repeating study events (e.g., when the same set of information is collected for a series of patient visits)." ;
    skos:exactMatch odm:StudyEventData .

odm:StudyEventDef a owl:Class,
        linkml:ClassDefinition ;
    rdfs:label "StudyEventDef" ;
    rdfs:subClassOf [ a owl:Restriction ;
            owl:maxQualifiedCardinality 1 ;
            owl:onClass odm:Oidref ;
            owl:onProperty odm:CommentOID ],
        [ a owl:Restriction ;
            owl:onClass odm:Oid ;
            owl:onProperty odm:OID ;
            owl:qualifiedCardinality 1 ],
        [ a owl:Restriction ;
            owl:maxQualifiedCardinality 1 ;
            owl:onClass odm:WorkflowRef ;
            owl:onProperty odm:WorkflowRefRef ],
        [ a owl:Restriction ;
            owl:allValuesFrom odm:Coding ;
            owl:onProperty odm:CodingRef ],
        [ a owl:Restriction ;
            owl:onClass odm:Name ;
            owl:onProperty odm:Name ;
            owl:qualifiedCardinality 1 ],
        [ a owl:Restriction ;
            owl:maxQualifiedCardinality 1 ;
            owl:onClass odm:Text ;
            owl:onProperty odm:Category ],
        [ a owl:Restriction ;
            owl:allValuesFrom odm:Alias ;
            owl:onProperty odm:AliasRef ],
        [ a owl:Restriction ;
            owl:allValuesFrom odm:ItemGroupRef ;
            owl:onProperty odm:ItemGroupRefRef ],
        [ a owl:Restriction ;
            owl:onClass odm:YesOrNo ;
            owl:onProperty odm:Repeating ;
            owl:qualifiedCardinality 1 ],
        [ a owl:Restriction ;
            owl:onClass odm:EventType ;
            owl:onProperty odm:Type ;
            owl:qualifiedCardinality 1 ],
        [ a owl:Restriction ;
            owl:maxQualifiedCardinality 1 ;
            owl:onClass odm:Description ;
            owl:onProperty odm:DescriptionRef ] ;
    skos:definition "StudyEventDef represents the definition of an activity in a study where data is collected. For example, a study event may represent a set of item groups that represent data collection instruments to be completed for a subject during a visit in a study. The visit occurs as part of a study workflow, and the workflow is referenced in the study event." ;
    skos:exactMatch odm:StudyEventDef .

odm:StudyEventGroupDef a owl:Class,
        linkml:ClassDefinition ;
    rdfs:label "StudyEventGroupDef" ;
    rdfs:subClassOf [ a owl:Restriction ;
            owl:allValuesFrom odm:Coding ;
            owl:onProperty odm:CodingRef ],
        [ a owl:Restriction ;
            owl:maxQualifiedCardinality 1 ;
            owl:onClass odm:Description ;
            owl:onProperty odm:DescriptionRef ],
        [ a owl:Restriction ;
            owl:allValuesFrom odm:StudyEventGroupRef ;
            owl:onProperty odm:StudyEventGroupRefRef ],
        [ a owl:Restriction ;
            owl:onClass odm:Name ;
            owl:onProperty odm:Name ;
            owl:qualifiedCardinality 1 ],
        [ a owl:Restriction ;
            owl:maxQualifiedCardinality 1 ;
            owl:onClass odm:Oidref ;
            owl:onProperty odm:CommentOID ],
        [ a owl:Restriction ;
            owl:maxQualifiedCardinality 1 ;
            owl:onClass odm:Oidref ;
            owl:onProperty odm:ArmOID ],
        [ a owl:Restriction ;
            owl:allValuesFrom odm:StudyEventRef ;
            owl:onProperty odm:StudyEventRefRef ],
        [ a owl:Restriction ;
            owl:maxQualifiedCardinality 1 ;
            owl:onClass odm:Oidref ;
            owl:onProperty odm:EpochOID ],
        [ a owl:Restriction ;
            owl:onClass odm:Oid ;
            owl:onProperty odm:OID ;
            owl:qualifiedCardinality 1 ],
        [ a owl:Restriction ;
            owl:maxQualifiedCardinality 1 ;
            owl:onClass odm:WorkflowRef ;
            owl:onProperty odm:WorkflowRefRef ] ;
    skos:definition "StudyEventGroupDef is a study building block that groups a number of smaller building blocks, which can themselves be StudyEventGroups or StudyEvents. It thus allows nesting of building blocks." ;
    skos:exactMatch odm:StudyEventGroupDef .

odm:StudyEventOID a owl:ObjectProperty,
        linkml:SlotDefinition ;
    rdfs:label "StudyEventOID" ;
    rdfs:range odm:Oidref ;
    skos:definition "Reference to the StudyEventDef ." .

odm:StudyIndication a owl:Class,
        linkml:ClassDefinition ;
    rdfs:label "StudyIndication" ;
    rdfs:subClassOf [ a owl:Restriction ;
            owl:maxQualifiedCardinality 1 ;
            owl:onClass odm:Description ;
            owl:onProperty odm:DescriptionRef ],
        [ a owl:Restriction ;
            owl:onClass odm:Oid ;
            owl:onProperty odm:OID ;
            owl:qualifiedCardinality 1 ],
        [ a owl:Restriction ;
            owl:allValuesFrom odm:Coding ;
            owl:onProperty odm:CodingRef ] ;
    skos:definition "This element describes a study indication (e.g., condition, disease) for the clinical study. The human-readable description is provided in the Description element. The Coding element can be used to provide a machine-readable code for the indication (e.g., SNOMED-CT code 26929004 for \"Alzheimer's disease\")." ;
    skos:exactMatch odm:StudyIndication .

odm:StudyIndications a owl:Class,
        linkml:ClassDefinition ;
    rdfs:label "StudyIndications" ;
    rdfs:subClassOf [ a owl:Restriction ;
            owl:allValuesFrom odm:StudyIndication ;
            owl:onProperty odm:StudyIndicationRef ] ;
    skos:definition "StudyIndications is a container element for individual StudyIndication elements." ;
    skos:exactMatch odm:StudyIndications .

odm:StudyInterventionRef a owl:Class,
        linkml:ClassDefinition ;
    rdfs:label "StudyInterventionRef" ;
    rdfs:subClassOf [ a owl:Restriction ;
            owl:onClass odm:Oidref ;
            owl:onProperty odm:StudyInterventionOID ;
            owl:qualifiedCardinality 1 ] ;
    skos:exactMatch odm:StudyInterventionRef .

odm:StudyInterventions a owl:Class,
        linkml:ClassDefinition ;
    rdfs:label "StudyInterventions" ;
    rdfs:subClassOf [ a owl:Restriction ;
            owl:allValuesFrom odm:StudyIntervention ;
            owl:onProperty odm:StudyInterventionRefRef ] ;
    skos:definition "The StudyInterventions element is a container element for individual StudyIntervention elements." ;
    skos:exactMatch odm:StudyInterventions .

odm:StudyObjective a owl:Class,
        linkml:ClassDefinition ;
    rdfs:label "StudyObjective" ;
    rdfs:subClassOf [ a owl:Restriction ;
            owl:allValuesFrom odm:StudyEndPointRef ;
            owl:onProperty odm:StudyEndPointRefRef ],
        [ a owl:Restriction ;
            owl:maxQualifiedCardinality 1 ;
            owl:onClass odm:StudyObjectiveLevel ;
            owl:onProperty odm:Level ],
        [ a owl:Restriction ;
            owl:maxQualifiedCardinality 1 ;
            owl:onClass odm:Description ;
            owl:onProperty odm:DescriptionRef ],
        [ a owl:Restriction ;
            owl:onClass odm:Name ;
            owl:onProperty odm:Name ;
            owl:qualifiedCardinality 1 ],
        [ a owl:Restriction ;
            owl:onClass odm:Oid ;
            owl:onProperty odm:OID ;
            owl:qualifiedCardinality 1 ] ;
    skos:exactMatch odm:StudyObjective .

odm:StudyObjectiveLevel a owl:Class,
        linkml:EnumDefinition ;
    rdfs:label "StudyObjectiveLevel" ;
    owl:unionOf ( <http://www.cdisc.org/ns/odm/v2.0/StudyObjectiveLevel#Primary> <http://www.cdisc.org/ns/odm/v2.0/StudyObjectiveLevel#Secondary> <http://www.cdisc.org/ns/odm/v2.0/StudyObjectiveLevel#Exploratory> ) ;
    linkml:permissible_values <http://www.cdisc.org/ns/odm/v2.0/StudyObjectiveLevel#Exploratory>,
        <http://www.cdisc.org/ns/odm/v2.0/StudyObjectiveLevel#Primary>,
        <http://www.cdisc.org/ns/odm/v2.0/StudyObjectiveLevel#Secondary> .

odm:StudyObjectives a owl:Class,
        linkml:ClassDefinition ;
    rdfs:label "StudyObjectives" ;
    rdfs:subClassOf [ a owl:Restriction ;
            owl:allValuesFrom odm:StudyObjective ;
            owl:onProperty odm:StudyObjectiveRef ] ;
    skos:definition "The StudyObjectives is a container element for individual StudyObjective elements." ;
    skos:exactMatch odm:StudyObjectives .

odm:StudyParameter a owl:Class,
        linkml:ClassDefinition ;
    rdfs:label "StudyParameter" ;
    rdfs:subClassOf [ a owl:Restriction ;
            owl:maxQualifiedCardinality 1 ;
            owl:onClass odm:ParameterValue ;
            owl:onProperty odm:ParameterValueRef ],
        [ a owl:Restriction ;
            owl:onClass odm:Oid ;
            owl:onProperty odm:OID ;
            owl:qualifiedCardinality 1 ],
        [ a owl:Restriction ;
            owl:allValuesFrom odm:Coding ;
            owl:onProperty odm:CodingRef ],
        [ a owl:Restriction ;
            owl:onClass odm:Name ;
            owl:onProperty odm:Term ;
            owl:qualifiedCardinality 1 ],
        [ a owl:Restriction ;
            owl:maxQualifiedCardinality 1 ;
            owl:onClass odm:Name ;
            owl:onProperty odm:ShortName ] ;
    skos:definition "A StudyParameter defines a study design parameter for which the value or values are delivered in the ParameterValue child element or elements." ;
    skos:exactMatch odm:StudyParameter .

odm:StudyStructure a owl:Class,
        linkml:ClassDefinition ;
    rdfs:label "StudyStructure" ;
    rdfs:subClassOf [ a owl:Restriction ;
            owl:allValuesFrom odm:Arm ;
            owl:onProperty odm:ArmRef ],
        [ a owl:Restriction ;
            owl:maxQualifiedCardinality 1 ;
            owl:onClass odm:Description ;
            owl:onProperty odm:DescriptionRef ],
        [ a owl:Restriction ;
            owl:allValuesFrom odm:Epoch ;
            owl:onProperty odm:EpochRef ],
        [ a owl:Restriction ;
            owl:maxQualifiedCardinality 1 ;
            owl:onClass odm:WorkflowRef ;
            owl:onProperty odm:WorkflowRefRef ] ;
    skos:definition "The StudyStructure element describes the general structure of a clinical study with arms, epochs, and workflows." ;
    skos:exactMatch odm:StudyStructure .

odm:StudySummary a owl:Class,
        linkml:ClassDefinition ;
    rdfs:label "StudySummary" ;
    rdfs:subClassOf [ a owl:Restriction ;
            owl:allValuesFrom odm:StudyParameter ;
            owl:onProperty odm:StudyParameterRef ] ;
    skos:definition "The StudyParameter element allows to provide a set of study design parameters such as anticipated number of subjects, minimum and maximum age of the participants, or planned number of arms." ;
    skos:exactMatch odm:StudySummary .

odm:StudyTargetPopulationRef a owl:Class,
        linkml:ClassDefinition ;
    rdfs:label "StudyTargetPopulationRef" ;
    rdfs:subClassOf [ a owl:Restriction ;
            owl:onClass odm:Oidref ;
            owl:onProperty odm:StudyTargetPopulationOID ;
            owl:qualifiedCardinality 1 ] ;
    skos:exactMatch odm:StudyTargetPopulationRef .

odm:StudyTiming a owl:Class,
        linkml:ClassDefinition ;
    rdfs:label "StudyTiming" ;
    rdfs:subClassOf [ a owl:Restriction ;
            owl:allValuesFrom odm:TransitionTimingConstraint ;
            owl:onProperty odm:TransitionTimingConstraintRef ],
        [ a owl:Restriction ;
            owl:onClass odm:Oid ;
            owl:onProperty odm:OID ;
            owl:qualifiedCardinality 1 ],
        [ a owl:Restriction ;
            owl:allValuesFrom odm:AbsoluteTimingConstraint ;
            owl:onProperty odm:AbsoluteTimingConstraintRef ],
        [ a owl:Restriction ;
            owl:onClass odm:Name ;
            owl:onProperty odm:Name ;
            owl:qualifiedCardinality 1 ],
        [ a owl:Restriction ;
            owl:allValuesFrom odm:RelativeTimingConstraint ;
            owl:onProperty odm:RelativeTimingConstraintRef ],
        [ a owl:Restriction ;
            owl:allValuesFrom odm:DurationTimingConstraint ;
            owl:onProperty odm:DurationTimingConstraintRef ] ;
    skos:definition "The StudyTiming element defines a timing constraint within the study, which can be an absolute timing constraint (e.g., start of the screening visit must be between 1 January 2022 and 31 December 2022), a relative timing constraint (e.g., visit 2 must be within 30 days after visit 1 with a window of +/- 1 week), a transition timing constraint (i.e., timing constraint on a transition within a defined workflow), or a duration timing constraint (e.g., the duration of visit 2 is planned to take hours with a window of 30 minutes)." ;
    skos:exactMatch odm:StudyTiming .

odm:StudyTimings a owl:Class,
        linkml:ClassDefinition ;
    rdfs:label "StudyTimings" ;
    rdfs:subClassOf [ a owl:Restriction ;
            owl:allValuesFrom odm:StudyTiming ;
            owl:onProperty odm:StudyTimingRef ] ;
    skos:definition "The StudyTimings element is a container element for individual StudyTiming elements." ;
    skos:exactMatch odm:StudyTimings .

odm:SubClass a owl:Class,
        linkml:ClassDefinition ;
    rdfs:label "SubClass" ;
    rdfs:subClassOf [ a owl:Restriction ;
            owl:maxQualifiedCardinality 1 ;
            owl:onClass odm:ItemGroupClassSubClass ;
            owl:onProperty odm:ParentClass ],
        [ a owl:Restriction ;
            owl:onClass odm:ItemGroupSubClass ;
            owl:onProperty odm:Name ;
            owl:qualifiedCardinality 1 ] ;
    skos:definition "This element contains SubClass definitions." ;
    skos:exactMatch odm:SubClass .

odm:SubjectData a owl:Class,
        linkml:ClassDefinition ;
    rdfs:label "SubjectData" ;
    rdfs:subClassOf [ a owl:Restriction ;
            owl:allValuesFrom odm:StudyEventData ;
            owl:onProperty odm:StudyEventDataRef ],
        [ a owl:Restriction ;
            owl:maxQualifiedCardinality 1 ;
            owl:onClass odm:Annotation ;
            owl:onProperty odm:AnnotationRef ],
        [ a owl:Restriction ;
            owl:onClass odm:SubjectKey ;
            owl:onProperty odm:SubjectKey ;
            owl:qualifiedCardinality 1 ],
        [ a owl:Restriction ;
            owl:maxQualifiedCardinality 1 ;
            owl:onClass odm:TransactionType ;
            owl:onProperty odm:TransactionTypeRef ],
        [ a owl:Restriction ;
            owl:maxQualifiedCardinality 1 ;
            owl:onClass odm:InvestigatorRef ;
            owl:onProperty odm:InvestigatorRefRef ],
        [ a owl:Restriction ;
            owl:maxQualifiedCardinality 1 ;
            owl:onClass odm:SiteRef ;
            owl:onProperty odm:SiteRefRef ],
        [ a owl:Restriction ;
            owl:allValuesFrom odm:Query ;
            owl:onProperty odm:QueryRef ],
        [ a owl:Restriction ;
            owl:maxQualifiedCardinality 1 ;
            owl:onClass odm:AuditRecord ;
            owl:onProperty odm:AuditRecordRef ],
        [ a owl:Restriction ;
            owl:maxQualifiedCardinality 1 ;
            owl:onClass odm:Signature ;
            owl:onProperty odm:SignatureRefRef ] ;
    skos:definition "Clinical data for a single subject." ;
    skos:exactMatch odm:SubjectData .

odm:Suffix a owl:Class,
        linkml:ClassDefinition ;
    rdfs:label "Suffix" ;
    rdfs:subClassOf [ a owl:Restriction ;
            owl:maxQualifiedCardinality 1 ;
            owl:onClass odm:ContentType ;
            owl:onProperty odm:_content ],
        [ a owl:Restriction ;
            owl:maxQualifiedCardinality 1 ;
            owl:onClass odm:String ;
            owl:onProperty odm:range ] ;
    skos:definition "This element may include credentials, or suffixes (e.g., Jr., III)." ;
    skos:exactMatch odm:Suffix .

odm:SummaryMeasure a owl:Class,
        linkml:ClassDefinition ;
    rdfs:label "SummaryMeasure" ;
    rdfs:subClassOf [ a owl:Restriction ;
            owl:maxQualifiedCardinality 1 ;
            owl:onClass odm:Description ;
            owl:onProperty odm:DescriptionRef ] ;
    skos:exactMatch odm:SummaryMeasure .

odm:SupplementalDoc a owl:Class,
        linkml:ClassDefinition ;
    rdfs:label "SupplementalDoc" ;
    rdfs:subClassOf [ a owl:Restriction ;
            owl:allValuesFrom odm:DocumentRef ;
            owl:onProperty odm:DocumentRefRef ] ;
    skos:definition "Supplemental data definitions" ;
    skos:exactMatch odm:SupplementalDoc .

odm:TargetTransition a owl:Class,
        linkml:ClassDefinition ;
    rdfs:label "TargetTransition" ;
    rdfs:subClassOf [ a owl:Restriction ;
            owl:onClass odm:Oidref ;
            owl:onProperty odm:TargetTransitionOID ;
            owl:qualifiedCardinality 1 ],
        [ a owl:Restriction ;
            owl:maxQualifiedCardinality 1 ;
            owl:onClass odm:Oidref ;
            owl:onProperty odm:ConditionOID ] ;
    skos:definition "Provides a reference to a Transition element." ;
    skos:exactMatch odm:TargetTransition .

odm:Transition a owl:Class,
        linkml:ClassDefinition ;
    rdfs:label "Transition" ;
    rdfs:subClassOf [ a owl:Restriction ;
            owl:maxQualifiedCardinality 1 ;
            owl:onClass odm:Oidref ;
            owl:onProperty odm:EndConditionOID ],
        [ a owl:Restriction ;
            owl:onClass odm:Oidref ;
            owl:onProperty odm:SourceOID ;
            owl:qualifiedCardinality 1 ],
        [ a owl:Restriction ;
            owl:onClass odm:Oid ;
            owl:onProperty odm:OID ;
            owl:qualifiedCardinality 1 ],
        [ a owl:Restriction ;
            owl:onClass odm:Name ;
            owl:onProperty odm:Name ;
            owl:qualifiedCardinality 1 ],
        [ a owl:Restriction ;
            owl:onClass odm:Oidref ;
            owl:onProperty odm:TargetOID ;
            owl:qualifiedCardinality 1 ],
        [ a owl:Restriction ;
            owl:maxQualifiedCardinality 1 ;
            owl:onClass odm:Oidref ;
            owl:onProperty odm:StartConditionOID ] ;
    skos:definition "A Transition defines a link between 2 structural elements in a workflow. When the execution of the transition is dependent upon a timing constraint that is either directly defined or calculated, a TransitionTimingConstraint must be defined, referencing the current Transition." ;
    skos:exactMatch odm:Transition .

odm:TransitionTimingConstraint a owl:Class,
        linkml:ClassDefinition ;
    rdfs:label "TransitionTimingConstraint" ;
    rdfs:subClassOf [ a owl:Restriction ;
            owl:onClass odm:DurationDatetime ;
            owl:onProperty odm:TimepointTarget ;
            owl:qualifiedCardinality 1 ],
        [ a owl:Restriction ;
            owl:maxQualifiedCardinality 1 ;
            owl:onClass odm:Description ;
            owl:onProperty odm:DescriptionRef ],
        [ a owl:Restriction ;
            owl:maxQualifiedCardinality 1 ;
            owl:onClass odm:RelativeTimingConstraintType ;
            owl:onProperty odm:Type ],
        [ a owl:Restriction ;
            owl:maxQualifiedCardinality 1 ;
            owl:onClass odm:Oidref ;
            owl:onProperty odm:MethodOID ],
        [ a owl:Restriction ;
            owl:maxQualifiedCardinality 1 ;
            owl:onClass odm:DurationDatetime ;
            owl:onProperty odm:TimepointPostWindow ],
        [ a owl:Restriction ;
            owl:onClass odm:Oidref ;
            owl:onProperty odm:TransitionOID ;
            owl:qualifiedCardinality 1 ],
        [ a owl:Restriction ;
            owl:maxQualifiedCardinality 1 ;
            owl:onClass odm:DurationDatetime ;
            owl:onProperty odm:TimepointPreWindow ],
        [ a owl:Restriction ;
            owl:onClass odm:Name ;
            owl:onProperty odm:Name ;
            owl:qualifiedCardinality 1 ],
        [ a owl:Restriction ;
            owl:onClass odm:Oid ;
            owl:onProperty odm:OID ;
            owl:qualifiedCardinality 1 ] ;
    skos:definition "The TransitionTimingConstraint element defines a timing constraint on a transition between structural elements as defined in a workflow. As such, it is a non-blocking constraint. This means that the transition is set on hold as long as the timing condition is not fulfilled, and is executed as soon as the timing condition is fulfilled." ;
    skos:exactMatch odm:TransitionTimingConstraint .

odm:TrialPhase a owl:Class,
        linkml:ClassDefinition ;
    rdfs:label "TrialPhase" ;
    rdfs:subClassOf [ a owl:Restriction ;
            owl:maxQualifiedCardinality 1 ;
            owl:onClass odm:Description ;
            owl:onProperty odm:DescriptionRef ],
        [ a owl:Restriction ;
            owl:onClass odm:TrialPhaseType ;
            owl:onProperty odm:ValueRef ;
            owl:qualifiedCardinality 1 ] ;
    skos:definition "The TrialPhase element designates the phase of the study in the clinical trial." ;
    skos:exactMatch odm:TrialPhase .

odm:UserName a owl:Class,
        linkml:ClassDefinition ;
    rdfs:label "UserName" ;
    rdfs:subClassOf [ a owl:Restriction ;
            owl:maxQualifiedCardinality 1 ;
            owl:onClass odm:ContentType ;
            owl:onProperty odm:_content ],
        [ a owl:Restriction ;
            owl:maxQualifiedCardinality 1 ;
            owl:onClass odm:String ;
            owl:onProperty odm:range ] ;
    skos:definition "The user's login identification in the sender's system." ;
    skos:exactMatch odm:UserName .

odm:ValueListDef a owl:Class,
        linkml:ClassDefinition ;
    rdfs:label "ValueListDef" ;
    rdfs:subClassOf [ a owl:Restriction ;
            owl:maxQualifiedCardinality 1 ;
            owl:onClass odm:Description ;
            owl:onProperty odm:DescriptionRef ],
        [ a owl:Restriction ;
            owl:onClass odm:Oid ;
            owl:onProperty odm:OID ;
            owl:qualifiedCardinality 1 ],
        [ a owl:Restriction ;
            owl:allValuesFrom odm:ItemRef ;
            owl:onProperty odm:ItemRefRef ] ;
    skos:definition "The following table specifies the XML structure for valuelist metadata. The ValueListDef element contains ItemRef elements that reference ItemDef elements that provide the value-level metadata details" ;
    skos:exactMatch odm:ValueListDef .

odm:ValueListRef a owl:Class,
        linkml:ClassDefinition ;
    rdfs:label "ValueListRef" ;
    rdfs:subClassOf [ a owl:Restriction ;
            owl:onClass odm:Oidref ;
            owl:onProperty odm:ValueListOID ;
            owl:qualifiedCardinality 1 ] ;
    skos:definition "The ValueListRef element is the OID of the ValueListDef that contains the valuelist definition associated with the variable. If value-level metadata is required for a variable, a ValueListRef element should be provided as a child element on the ItemDef for the variable definition." ;
    skos:exactMatch odm:ValueListRef .

odm:WhereClauseDef a owl:Class,
        linkml:ClassDefinition ;
    rdfs:label "WhereClauseDef" ;
    rdfs:subClassOf [ a owl:Restriction ;
            owl:onClass odm:Oid ;
            owl:onProperty odm:OID ;
            owl:qualifiedCardinality 1 ],
        [ a owl:Restriction ;
            owl:maxQualifiedCardinality 1 ;
            owl:onClass odm:Oidref ;
            owl:onProperty odm:CommentOID ],
        [ a owl:Restriction ;
            owl:allValuesFrom odm:RangeCheck ;
            owl:onProperty odm:RangeCheckRef ] ;
    skos:definition "The WhereClauseDef element specifies a condition." ;
    skos:exactMatch odm:WhereClauseDef .

odm:WhereClauseRef a owl:Class,
        linkml:ClassDefinition ;
    rdfs:label "WhereClauseRef" ;
    rdfs:subClassOf [ a owl:Restriction ;
            owl:onClass odm:Oidref ;
            owl:onProperty odm:WhereClauseOID ;
            owl:qualifiedCardinality 1 ] ;
    skos:definition "The WhereClauseRef references the WhereClauseDef element that describes the conditions under which the variable values are defined by the referenced ItemDef." ;
    skos:exactMatch odm:WhereClauseRef .

odm:WorkflowDef a owl:Class,
        linkml:ClassDefinition ;
    rdfs:label "WorkflowDef" ;
    rdfs:subClassOf [ a owl:Restriction ;
            owl:onClass odm:Name ;
            owl:onProperty odm:Name ;
            owl:qualifiedCardinality 1 ],
        [ a owl:Restriction ;
            owl:allValuesFrom odm:WorkflowEnd ;
            owl:onProperty odm:WorkflowEndRef ],
        [ a owl:Restriction ;
            owl:maxQualifiedCardinality 1 ;
            owl:onClass odm:WorkflowStart ;
            owl:onProperty odm:WorkflowStartRef ],
        [ a owl:Restriction ;
            owl:onClass odm:Oid ;
            owl:onProperty odm:OID ;
            owl:qualifiedCardinality 1 ],
        [ a owl:Restriction ;
            owl:allValuesFrom odm:Transition ;
            owl:onProperty odm:TransitionRef ],
        [ a owl:Restriction ;
            owl:allValuesFrom odm:Branching ;
            owl:onProperty odm:BranchingRef ],
        [ a owl:Restriction ;
            owl:maxQualifiedCardinality 1 ;
            owl:onClass odm:Description ;
            owl:onProperty odm:DescriptionRef ] ;
    skos:definition "A WorkflowDef defines an automated workflow for a study." ;
    skos:exactMatch odm:WorkflowDef .

odm:WorkflowEnd a owl:Class,
        linkml:ClassDefinition ;
    rdfs:label "WorkflowEnd" ;
    rdfs:subClassOf [ a owl:Restriction ;
            owl:onClass odm:Oidref ;
            owl:onProperty odm:EndOID ;
            owl:qualifiedCardinality 1 ],
        [ a owl:Restriction ;
            owl:maxQualifiedCardinality 1 ;
            owl:onClass odm:Text ;
            owl:onProperty odm:_content ] ;
    skos:definition "A WorkflowEnd references a structural element with which the workflows ends." ;
    skos:exactMatch odm:WorkflowEnd .

odm:WorkflowStart a owl:Class,
        linkml:ClassDefinition ;
    rdfs:label "WorkflowStart" ;
    rdfs:subClassOf [ a owl:Restriction ;
            owl:onClass odm:Oidref ;
            owl:onProperty odm:StartOID ;
            owl:qualifiedCardinality 1 ] ;
    skos:definition "WorkflowStart references a structural element that begins the automated workflow." ;
    skos:exactMatch odm:WorkflowStart .

odm:CLDataType a owl:Class,
        linkml:EnumDefinition ;
    rdfs:label "CLDataType" ;
    owl:unionOf ( <http://www.cdisc.org/ns/odm/v2.0/CLDataType#integer> <http://www.cdisc.org/ns/odm/v2.0/CLDataType#decimal> <http://www.cdisc.org/ns/odm/v2.0/CLDataType#text> <http://www.cdisc.org/ns/odm/v2.0/CLDataType#string> ) ;
    linkml:permissible_values <http://www.cdisc.org/ns/odm/v2.0/CLDataType#decimal>,
        <http://www.cdisc.org/ns/odm/v2.0/CLDataType#integer>,
        <http://www.cdisc.org/ns/odm/v2.0/CLDataType#string>,
        <http://www.cdisc.org/ns/odm/v2.0/CLDataType#text> .

odm:DateTimeStamp a owl:Class,
        linkml:ClassDefinition ;
    rdfs:label "DateTimeStamp" ;
    rdfs:subClassOf [ a owl:Restriction ;
            owl:maxQualifiedCardinality 1 ;
            owl:onClass odm:ContentType ;
            owl:onProperty odm:_content ],
        [ a owl:Restriction ;
            owl:maxQualifiedCardinality 1 ;
            owl:onClass odm:String ;
            owl:onProperty odm:range ] ;
    skos:exactMatch odm:DateTimeStamp .

odm:DocumentRefRef a owl:ObjectProperty,
        linkml:SlotDefinition ;
    rdfs:label "DocumentRefRef" ;
    rdfs:range odm:DocumentRef ;
    skos:definition "The DocumentRef element is a container for page references in a PDF file." .

odm:EditPointType a owl:Class,
        linkml:EnumDefinition ;
    rdfs:label "EditPointType" ;
    owl:unionOf ( <http://www.cdisc.org/ns/odm/v2.0/EditPointType#Monitoring> <http://www.cdisc.org/ns/odm/v2.0/EditPointType#DataManagement> <http://www.cdisc.org/ns/odm/v2.0/EditPointType#DBAudit> ) ;
    linkml:permissible_values <http://www.cdisc.org/ns/odm/v2.0/EditPointType#DBAudit>,
        <http://www.cdisc.org/ns/odm/v2.0/EditPointType#DataManagement>,
        <http://www.cdisc.org/ns/odm/v2.0/EditPointType#Monitoring> .

odm:FormalExpressionRef a owl:ObjectProperty,
        linkml:SlotDefinition ;
    rdfs:label "FormalExpressionRef" ;
    rdfs:range odm:FormalExpression ;
    skos:definition "FormalExpression reference: A FormalExpression used within a ConditionDef or a RangeCheck must evaluate to True or False. A FormalExpression referenced within a MethodDef having Type Imputation, Computation, or Transpose must evaluate to the correct DataType for an Item that may be imputed or computed using the Method. A FormalExpression gets parameter and return value definitions from the MethodSignature element. The data types in the MethodSignature parameters and return values must match the corresponding data types in the FormalExpression." .

odm:ItemGroupRef a owl:Class,
        linkml:ClassDefinition ;
    rdfs:label "ItemGroupRef" ;
    rdfs:subClassOf [ a owl:Restriction ;
            owl:maxQualifiedCardinality 1 ;
            owl:onClass odm:PositiveInteger ;
            owl:onProperty odm:OrderNumber ],
        [ a owl:Restriction ;
            owl:maxQualifiedCardinality 1 ;
            owl:onClass odm:Oidref ;
            owl:onProperty odm:MethodOID ],
        [ a owl:Restriction ;
            owl:onClass odm:Oidref ;
            owl:onProperty odm:ItemGroupOID ;
            owl:qualifiedCardinality 1 ],
        [ a owl:Restriction ;
            owl:onClass odm:YesOrNo ;
            owl:onProperty odm:Mandatory ;
            owl:qualifiedCardinality 1 ],
        [ a owl:Restriction ;
            owl:maxQualifiedCardinality 1 ;
            owl:onClass odm:Oidref ;
            owl:onProperty odm:CollectionExceptionConditionOID ] ;
    skos:definition "ItemGroupRef references an ItemGroupDef as it occurs within a specific StudyEventDef or ItemGroupDef. The list of ItemGroupRefs identifies the types of item groups that are allowed to occur within this type of studyevent or (nested) item group. The ItemGroupRefs within a single StudyEventDef or ItemGroupDef must not have duplicate ItemGroupOID or OrderNumber attribute values." ;
    skos:exactMatch odm:ItemGroupRef .

odm:ItemGroupRepeatingType a owl:Class,
        linkml:EnumDefinition ;
    rdfs:label "ItemGroupRepeatingType" ;
    owl:unionOf ( <http://www.cdisc.org/ns/odm/v2.0/ItemGroupRepeatingType#No> <http://www.cdisc.org/ns/odm/v2.0/ItemGroupRepeatingType#Simple> <http://www.cdisc.org/ns/odm/v2.0/ItemGroupRepeatingType#Dynamic> <http://www.cdisc.org/ns/odm/v2.0/ItemGroupRepeatingType#Static> ) ;
    linkml:permissible_values <http://www.cdisc.org/ns/odm/v2.0/ItemGroupRepeatingType#Dynamic>,
        <http://www.cdisc.org/ns/odm/v2.0/ItemGroupRepeatingType#No>,
        <http://www.cdisc.org/ns/odm/v2.0/ItemGroupRepeatingType#Simple>,
        <http://www.cdisc.org/ns/odm/v2.0/ItemGroupRepeatingType#Static> .

odm:ItemGroupSubClass a owl:Class,
        linkml:EnumDefinition ;
    rdfs:label "ItemGroupSubClass" ;
    owl:unionOf ( <http://ncicb.nci.nih.gov/xml/odm/EVS/CDISCExtCodeID:C176265> <http://ncicb.nci.nih.gov/xml/odm/EVS/CDISCExtCodeID:C177920> <http://ncicb.nci.nih.gov/xml/odm/EVS/CDISCExtCodeID:C172452> <http://ncicb.nci.nih.gov/xml/odm/EVS/CDISCExtCodeID:C165637> ) ;
    linkml:permissible_values <http://ncicb.nci.nih.gov/xml/odm/EVS/CDISCExtCodeID:C165637>,
        <http://ncicb.nci.nih.gov/xml/odm/EVS/CDISCExtCodeID:C172452>,
        <http://ncicb.nci.nih.gov/xml/odm/EVS/CDISCExtCodeID:C176265>,
        <http://ncicb.nci.nih.gov/xml/odm/EVS/CDISCExtCodeID:C177920> .

odm:ItemOID a owl:ObjectProperty,
        linkml:SlotDefinition ;
    rdfs:label "ItemOID" ;
    rdfs:range odm:Oidref ;
    skos:definition "Reference to the ItemDef ." .

odm:ItemRef a owl:Class,
        linkml:ClassDefinition ;
    rdfs:label "ItemRef" ;
    rdfs:subClassOf [ a owl:Restriction ;
            owl:maxQualifiedCardinality 1 ;
            owl:onClass odm:PositiveInteger ;
            owl:onProperty odm:KeySequence ],
        [ a owl:Restriction ;
            owl:maxQualifiedCardinality 1 ;
            owl:onClass odm:Text ;
            owl:onProperty odm:Role ],
        [ a owl:Restriction ;
            owl:onClass odm:YesOrNo ;
            owl:onProperty odm:Mandatory ;
            owl:qualifiedCardinality 1 ],
        [ a owl:Restriction ;
            owl:onClass odm:Oidref ;
            owl:onProperty odm:ItemOID ;
            owl:qualifiedCardinality 1 ],
        [ a owl:Restriction ;
            owl:maxQualifiedCardinality 1 ;
            owl:onClass odm:Oidref ;
            owl:onProperty odm:CollectionExceptionConditionOID ],
        [ a owl:Restriction ;
            owl:allValuesFrom odm:WhereClauseRef ;
            owl:onProperty odm:WhereClauseRefRef ],
        [ a owl:Restriction ;
            owl:maxQualifiedCardinality 1 ;
            owl:onClass odm:YesOnly ;
            owl:onProperty odm:IsNonStandard ],
        [ a owl:Restriction ;
            owl:maxQualifiedCardinality 1 ;
            owl:onClass odm:Oidref ;
            owl:onProperty odm:UnitsItemOID ],
        [ a owl:Restriction ;
            owl:maxQualifiedCardinality 1 ;
            owl:onClass odm:Oidref ;
            owl:onProperty odm:RoleCodeListOID ],
        [ a owl:Restriction ;
            owl:maxQualifiedCardinality 1 ;
            owl:onClass odm:YesOnly ;
            owl:onProperty odm:Repeat ],
        [ a owl:Restriction ;
            owl:maxQualifiedCardinality 1 ;
            owl:onClass odm:YesOnly ;
            owl:onProperty odm:Other ],
        [ a owl:Restriction ;
            owl:maxQualifiedCardinality 1 ;
            owl:onClass odm:Text ;
            owl:onProperty odm:PreSpecifiedValue ],
        [ a owl:Restriction ;
            owl:allValuesFrom odm:Origin ;
            owl:onProperty odm:OriginRef ],
        [ a owl:Restriction ;
            owl:maxQualifiedCardinality 1 ;
            owl:onClass odm:PositiveInteger ;
            owl:onProperty odm:OrderNumber ],
        [ a owl:Restriction ;
            owl:maxQualifiedCardinality 1 ;
            owl:onClass odm:Oidref ;
            owl:onProperty odm:MethodOID ],
        [ a owl:Restriction ;
            owl:maxQualifiedCardinality 1 ;
            owl:onClass odm:CoreType ;
            owl:onProperty odm:Core ],
        [ a owl:Restriction ;
            owl:maxQualifiedCardinality 1 ;
            owl:onClass odm:YesOnly ;
            owl:onProperty odm:HasNoData ] ;
    skos:definition "A reference to an ItemDef as it occurs within a specific ItemGroupDef. The list of ItemRefs identifies the types of items that are allowed to occur within this type of item group." ;
    skos:exactMatch odm:ItemRef .

odm:Leaf a owl:Class,
        linkml:ClassDefinition ;
    rdfs:label "Leaf" ;
    rdfs:subClassOf [ a owl:Restriction ;
            owl:onClass odm:Uriorcurie ;
            owl:onProperty odm:href ;
            owl:qualifiedCardinality 1 ],
        [ a owl:Restriction ;
            owl:onClass odm:Oid ;
            owl:onProperty odm:ID ;
            owl:qualifiedCardinality 1 ],
        [ a owl:Restriction ;
            owl:maxQualifiedCardinality 1 ;
            owl:onClass odm:Text ;
            owl:onProperty odm:Title ] ;
    skos:definition "Contains the XLink information referenced by DocumentRef or ArchiveLocationID" ;
    skos:exactMatch odm:Leaf .

odm:LocationRef a owl:Class,
        linkml:ClassDefinition ;
    rdfs:label "LocationRef" ;
    rdfs:subClassOf [ a owl:Restriction ;
            owl:onClass odm:Oidref ;
            owl:onProperty odm:LocationOID ;
            owl:qualifiedCardinality 1 ] ;
    skos:definition "A reference to the user's physical location." ;
    skos:exactMatch odm:LocationRef .

odm:MethodType a owl:Class,
        linkml:EnumDefinition ;
    rdfs:label "MethodType" ;
    owl:unionOf ( <http://www.cdisc.org/ns/odm/v2.0/MethodType#Computation> <http://www.cdisc.org/ns/odm/v2.0/MethodType#Imputation> <http://www.cdisc.org/ns/odm/v2.0/MethodType#Preload> <http://www.cdisc.org/ns/odm/v2.0/MethodType#Transpose> ) ;
    linkml:permissible_values <http://www.cdisc.org/ns/odm/v2.0/MethodType#Computation>,
        <http://www.cdisc.org/ns/odm/v2.0/MethodType#Imputation>,
        <http://www.cdisc.org/ns/odm/v2.0/MethodType#Preload>,
        <http://www.cdisc.org/ns/odm/v2.0/MethodType#Transpose> .

odm:Origin a owl:Class,
        linkml:ClassDefinition ;
    rdfs:label "Origin" ;
    rdfs:subClassOf [ a owl:Restriction ;
            owl:maxQualifiedCardinality 1 ;
            owl:onClass odm:SourceItems ;
            owl:onProperty odm:SourceItemsRef ],
        [ a owl:Restriction ;
            owl:maxQualifiedCardinality 1 ;
            owl:onClass odm:Description ;
            owl:onProperty odm:DescriptionRef ],
        [ a owl:Restriction ;
            owl:maxQualifiedCardinality 1 ;
            owl:onClass odm:OriginSource ;
            owl:onProperty odm:Source ],
        [ a owl:Restriction ;
            owl:allValuesFrom odm:DocumentRef ;
            owl:onProperty odm:DocumentRefRef ],
        [ a owl:Restriction ;
            owl:onClass odm:OriginType ;
            owl:onProperty odm:Type ;
            owl:qualifiedCardinality 1 ],
        [ a owl:Restriction ;
            owl:allValuesFrom odm:Coding ;
            owl:onProperty odm:CodingRef ] ;
    skos:definition "Origin defines the source metadata, where applicable, for ODM ItemRefs or ItemGroupRefs. Origin as a child element replaces the Origin attribute in ODM v1.3 that exists for the ItemDef and ItemGroupDef elements.The Origin element is based on the def:Origin element in Define-XML v2.1 with the Trace-XML v1.0 extension." ;
    skos:exactMatch odm:Origin .

odm:OriginSource a owl:Class,
        linkml:EnumDefinition ;
    rdfs:label "OriginSource" ;
    owl:unionOf ( <http://ncicb.nci.nih.gov/xml/odm/EVS/CDISCExtCodeID:C25936> <http://ncicb.nci.nih.gov/xml/odm/EVS/CDISCExtCodeID:C70793> <http://ncicb.nci.nih.gov/xml/odm/EVS/CDISCExtCodeID:C41189> <http://ncicb.nci.nih.gov/xml/odm/EVS/CDISCExtCodeID:C68608> ) ;
    linkml:permissible_values <http://ncicb.nci.nih.gov/xml/odm/EVS/CDISCExtCodeID:C25936>,
        <http://ncicb.nci.nih.gov/xml/odm/EVS/CDISCExtCodeID:C41189>,
        <http://ncicb.nci.nih.gov/xml/odm/EVS/CDISCExtCodeID:C68608>,
        <http://ncicb.nci.nih.gov/xml/odm/EVS/CDISCExtCodeID:C70793> .

odm:RangeCheck a owl:Class,
        linkml:ClassDefinition ;
    rdfs:label "RangeCheck" ;
    rdfs:subClassOf [ a owl:Restriction ;
            owl:allValuesFrom odm:FormalExpression ;
            owl:onProperty odm:FormalExpressionRef ],
        [ a owl:Restriction ;
            owl:maxQualifiedCardinality 1 ;
            owl:onClass odm:SoftOrHard ;
            owl:onProperty odm:SoftHard ],
        [ a owl:Restriction ;
            owl:maxQualifiedCardinality 1 ;
            owl:onClass odm:MethodSignature ;
            owl:onProperty odm:MethodSignatureRef ],
        [ a owl:Restriction ;
            owl:maxQualifiedCardinality 1 ;
            owl:onClass odm:ErrorMessage ;
            owl:onProperty odm:ErrorMessageRef ],
        [ a owl:Restriction ;
            owl:allValuesFrom odm:CheckValue ;
            owl:onProperty odm:CheckValueRef ],
        [ a owl:Restriction ;
            owl:maxQualifiedCardinality 1 ;
            owl:onClass odm:Oidref ;
            owl:onProperty odm:ItemOID ],
        [ a owl:Restriction ;
            owl:maxQualifiedCardinality 1 ;
            owl:onClass odm:Comparator ;
            owl:onProperty odm:ComparatorRef ] ;
    skos:definition "A RangeCheck defines a constraint on the value of the enclosing item. It represents an expression that evaluates to True when the ItemData value is valid or False when the ItemData value is invalid. The expression is specified using either Comparator and CheckValue or using FormalExpressions." ;
    skos:exactMatch odm:RangeCheck .

odm:StudyEndPointRef a owl:Class,
        linkml:ClassDefinition ;
    rdfs:label "StudyEndPointRef" ;
    rdfs:subClassOf [ a owl:Restriction ;
            owl:maxQualifiedCardinality 1 ;
            owl:onClass odm:PositiveInteger ;
            owl:onProperty odm:OrderNumber ],
        [ a owl:Restriction ;
            owl:onClass odm:Oidref ;
            owl:onProperty odm:StudyEndPointOID ;
            owl:qualifiedCardinality 1 ] ;
    skos:definition "Go to start of metadata" ;
    skos:exactMatch odm:StudyEndPointRef .

odm:StudyEndPointType a owl:Class,
        linkml:EnumDefinition ;
    rdfs:label "StudyEndPointType" ;
    owl:unionOf ( <http://www.cdisc.org/ns/odm/v2.0/StudyEndPointType#Simple> <http://www.cdisc.org/ns/odm/v2.0/StudyEndPointType#Humane> <http://www.cdisc.org/ns/odm/v2.0/StudyEndPointType#Surrogate> <http://www.cdisc.org/ns/odm/v2.0/StudyEndPointType#Composite> ) ;
    linkml:permissible_values <http://www.cdisc.org/ns/odm/v2.0/StudyEndPointType#Composite>,
        <http://www.cdisc.org/ns/odm/v2.0/StudyEndPointType#Humane>,
        <http://www.cdisc.org/ns/odm/v2.0/StudyEndPointType#Simple>,
        <http://www.cdisc.org/ns/odm/v2.0/StudyEndPointType#Surrogate> .

odm:StudyEstimandLevel a owl:Class,
        linkml:EnumDefinition ;
    rdfs:label "StudyEstimandLevel" ;
    owl:unionOf ( <http://www.cdisc.org/ns/odm/v2.0/StudyEstimandLevel#Primary> <http://www.cdisc.org/ns/odm/v2.0/StudyEstimandLevel#Secondary> <http://www.cdisc.org/ns/odm/v2.0/StudyEstimandLevel#Exploratory> ) ;
    linkml:permissible_values <http://www.cdisc.org/ns/odm/v2.0/StudyEstimandLevel#Exploratory>,
        <http://www.cdisc.org/ns/odm/v2.0/StudyEstimandLevel#Primary>,
        <http://www.cdisc.org/ns/odm/v2.0/StudyEstimandLevel#Secondary> .

odm:StudyEventRef a owl:Class,
        linkml:ClassDefinition ;
    rdfs:label "StudyEventRef" ;
    rdfs:subClassOf [ a owl:Restriction ;
            owl:maxQualifiedCardinality 1 ;
            owl:onClass odm:Oidref ;
            owl:onProperty odm:CollectionExceptionConditionOID ],
        [ a owl:Restriction ;
            owl:onClass odm:Oidref ;
            owl:onProperty odm:StudyEventOID ;
            owl:qualifiedCardinality 1 ],
        [ a owl:Restriction ;
            owl:maxQualifiedCardinality 1 ;
            owl:onClass odm:PositiveInteger ;
            owl:onProperty odm:OrderNumber ],
        [ a owl:Restriction ;
            owl:onClass odm:YesOrNo ;
            owl:onProperty odm:Mandatory ;
            owl:qualifiedCardinality 1 ] ;
    skos:definition "This element references a StudyEventDef as it occurs within a specific version of a study. The list of StudyEventRefs identifies the types of study events that are allowed to occur within the study." ;
    skos:exactMatch odm:StudyEventRef .

odm:SubjectKey a owl:Class,
        owl:ObjectProperty,
        linkml:SlotDefinition,
        linkml:TypeDefinition ;
    rdfs:label "SubjectKey",
        "subjectKey" ;
    rdfs:range odm:SubjectKey ;
    rdfs:subClassOf [ a owl:Restriction ;
            owl:onDataRange odm:subjectKey ;
            owl:onProperty linkml:topValue ;
            owl:qualifiedCardinality 1 ] ;
    skos:definition "Unique identifier for the Subject." .

odm:TransactionTypeRef a owl:ObjectProperty,
        linkml:SlotDefinition ;
    rdfs:label "TransactionTypeRef" ;
    rdfs:range odm:TransactionType ;
    skos:definition "Identifies the transaction type when /ODM/@FileType is Transactional and there is no child element." .

odm:UserRef a owl:Class,
        linkml:ClassDefinition ;
    rdfs:label "UserRef" ;
    rdfs:subClassOf [ a owl:Restriction ;
            owl:onClass odm:Oidref ;
            owl:onProperty odm:UserOID ;
            owl:qualifiedCardinality 1 ] ;
    skos:exactMatch odm:UserRef .

odm:ValueRef a owl:ObjectProperty,
        linkml:SlotDefinition ;
    rdfs:label "ValueRef" ;
    rdfs:range odm:Value ;
    skos:definition "Human-readable designation of the trial phase." .

odm:href a owl:ObjectProperty,
        linkml:SlotDefinition ;
    rdfs:label "href" ;
    rdfs:range odm:String ;
    skos:definition "URL that can be used to identify the location of a document or dataset file relative to the folder containing the ODM file." .

<http://ncicb.nci.nih.gov/xml/odm/EVS/CDISCExtCodeID:C163415> a odm:DictionaryNameTypeEnum,
        odm:StandardName,
        odm:StandardType,
        owl:Class ;
    rdfs:label "CDISC CT",
        "CDISC/NCI",
        "CT" .

odm:Address a owl:Class,
        linkml:ClassDefinition ;
    rdfs:label "Address" ;
    rdfs:subClassOf [ a owl:Restriction ;
            owl:maxQualifiedCardinality 1 ;
            owl:onClass odm:City ;
            owl:onProperty odm:CityRef ],
        [ a owl:Restriction ;
            owl:maxQualifiedCardinality 1 ;
            owl:onClass odm:OtherText ;
            owl:onProperty odm:OtherTextRef ],
        [ a owl:Restriction ;
            owl:maxQualifiedCardinality 1 ;
            owl:onClass odm:HouseNumber ;
            owl:onProperty odm:HouseNumberRef ],
        [ a owl:Restriction ;
            owl:maxQualifiedCardinality 1 ;
            owl:onClass odm:StreetName ;
            owl:onProperty odm:StreetNameRef ],
        [ a owl:Restriction ;
            owl:maxQualifiedCardinality 1 ;
            owl:onClass odm:StateProv ;
            owl:onProperty odm:StateProvRef ],
        [ a owl:Restriction ;
            owl:maxQualifiedCardinality 1 ;
            owl:onClass odm:PostalCode ;
            owl:onProperty odm:PostalCodeRef ],
        [ a owl:Restriction ;
            owl:maxQualifiedCardinality 1 ;
            owl:onClass odm:Country ;
            owl:onProperty odm:CountryRef ],
        [ a owl:Restriction ;
            owl:maxQualifiedCardinality 1 ;
            owl:onClass odm:GeoPosition ;
            owl:onProperty odm:GeoPositionRef ] ;
    skos:definition "The postal address for a user, location, or organization." ;
    skos:exactMatch odm:Address .

odm:Datetime a owl:Class,
        linkml:TypeDefinition ;
    rdfs:label "datetime" ;
    rdfs:subClassOf [ a owl:Restriction ;
            owl:onDataRange xsd:dateTime ;
            owl:onProperty linkml:topValue ;
            owl:qualifiedCardinality 1 ] .

odm:MethodSignature a owl:Class,
        linkml:ClassDefinition ;
    rdfs:label "MethodSignature" ;
    rdfs:subClassOf [ a owl:Restriction ;
            owl:allValuesFrom odm:ReturnValue ;
            owl:onProperty odm:ReturnValueRef ],
        [ a owl:Restriction ;
            owl:allValuesFrom odm:Parameter ;
            owl:onProperty odm:ParameterRef ] ;
    skos:definition "A MethodSignature defines the parameters and return values for a method. The MethodSignature improves traceability while enhancing the ability for automation engines to execute a MethodDef's FormalExpression. Most Methods use one or more input parameters and return one or more values." ;
    skos:exactMatch odm:MethodSignature .

odm:QueryRef a owl:ObjectProperty,
        linkml:SlotDefinition ;
    rdfs:label "QueryRef" ;
    rdfs:range odm:Query ;
    skos:definition "Query reference: The Query element represents a request for clarification on a data item collected for a clinical trial, specifically a request from a sponsor or sponsor’s representative to an investigator to resolve an error or inconsistency discovered during data review. Queries can be created manually by individuals such as site monitors or data managers or automatically by systems. The full text of the Query exists in the Value child element. The optional Name attribute provide the means to provide a short identifier that can be included in listing or user interfaces." .

odm:QuerySourceType a owl:Class,
        linkml:EnumDefinition ;
    rdfs:label "QuerySourceType" ;
    owl:unionOf ( <http://www.cdisc.org/ns/odm/v2.0/QuerySourceType#System> <http://www.cdisc.org/ns/odm/v2.0/QuerySourceType#Data+Management> <http://www.cdisc.org/ns/odm/v2.0/QuerySourceType#Site+Monitor> <http://www.cdisc.org/ns/odm/v2.0/QuerySourceType#Coding+System> <http://www.cdisc.org/ns/odm/v2.0/QuerySourceType#Safety+Reviewer> ) ;
    linkml:permissible_values <http://www.cdisc.org/ns/odm/v2.0/QuerySourceType#Coding+System>,
        <http://www.cdisc.org/ns/odm/v2.0/QuerySourceType#Data+Management>,
        <http://www.cdisc.org/ns/odm/v2.0/QuerySourceType#Safety+Reviewer>,
        <http://www.cdisc.org/ns/odm/v2.0/QuerySourceType#Site+Monitor>,
        <http://www.cdisc.org/ns/odm/v2.0/QuerySourceType#System> .

odm:RelativeTimingConstraintType a owl:Class,
        linkml:EnumDefinition ;
    rdfs:label "RelativeTimingConstraintType" ;
    owl:unionOf ( <http://www.cdisc.org/ns/odm/v2.0/RelativeTimingConstraintType#StartToStart> <http://www.cdisc.org/ns/odm/v2.0/RelativeTimingConstraintType#StartToFinish> <http://www.cdisc.org/ns/odm/v2.0/RelativeTimingConstraintType#FinishToStart> <http://www.cdisc.org/ns/odm/v2.0/RelativeTimingConstraintType#FinishToFinish> ) ;
    linkml:permissible_values <http://www.cdisc.org/ns/odm/v2.0/RelativeTimingConstraintType#FinishToFinish>,
        <http://www.cdisc.org/ns/odm/v2.0/RelativeTimingConstraintType#FinishToStart>,
        <http://www.cdisc.org/ns/odm/v2.0/RelativeTimingConstraintType#StartToFinish>,
        <http://www.cdisc.org/ns/odm/v2.0/RelativeTimingConstraintType#StartToStart> .

odm:RepeatKey a owl:Class,
        linkml:TypeDefinition ;
    rdfs:label "repeatKey" ;
    rdfs:subClassOf [ a owl:Restriction ;
            owl:onDataRange odm:repeatKey ;
            owl:onProperty linkml:topValue ;
            owl:qualifiedCardinality 1 ] .

odm:StudyEventGroupRef a owl:Class,
        linkml:ClassDefinition ;
    rdfs:label "StudyEventGroupRef" ;
    rdfs:subClassOf [ a owl:Restriction ;
            owl:onClass odm:Oidref ;
            owl:onProperty odm:StudyEventGroupOID ;
            owl:qualifiedCardinality 1 ],
        [ a owl:Restriction ;
            owl:maxQualifiedCardinality 1 ;
            owl:onClass odm:Oidref ;
            owl:onProperty odm:CollectionExceptionConditionOID ],
        [ a owl:Restriction ;
            owl:maxQualifiedCardinality 1 ;
            owl:onClass odm:PositiveInteger ;
            owl:onProperty odm:OrderNumber ],
        [ a owl:Restriction ;
            owl:maxQualifiedCardinality 1 ;
            owl:onClass odm:Description ;
            owl:onProperty odm:DescriptionRef ],
        [ a owl:Restriction ;
            owl:onClass odm:YesOrNo ;
            owl:onProperty odm:Mandatory ;
            owl:qualifiedCardinality 1 ] ;
    skos:definition "This element references a StudyEventGroupDef as it occurs within a specific version of a study. The list of StudyEventGroupRefs identifies the types of study group events that are allowed to occur within the study." ;
    skos:exactMatch odm:StudyEventGroupRef .

odm:Telecom a owl:Class,
        linkml:ClassDefinition ;
    rdfs:label "Telecom" ;
    rdfs:subClassOf [ a owl:Restriction ;
            owl:onClass odm:Text ;
            owl:onProperty odm:ValueRef ;
            owl:qualifiedCardinality 1 ],
        [ a owl:Restriction ;
            owl:onClass odm:TelecomTypeType ;
            owl:onProperty odm:TelecomType ;
            owl:qualifiedCardinality 1 ] ;
    skos:definition "The telecommunication contacts points of a user, a location, or an organization. The Type attribute designates the type of contact." ;
    skos:exactMatch odm:Telecom .

odm:AnnotationRef a owl:ObjectProperty,
        linkml:SlotDefinition ;
    rdfs:label "AnnotationRef" ;
    rdfs:range odm:Annotation ;
    skos:definition "Annotation reference: A general note about clinical data. If an annotation has both a comment and flags, the flags should be related to the comment." .

odm:AuditRecordRef a owl:ObjectProperty,
        linkml:SlotDefinition ;
    rdfs:label "AuditRecordRef" ;
    rdfs:range odm:AuditRecord ;
    skos:definition "AuditRecord reference: An AuditRecord carries information pertaining to the creation, deletion, or modification of clinical data. This information includes who performed that action, and where, when, and why that action was performed.AuditRecord information describes a change to clinical data, but is not itself clinical data. The value of some clinical data can always be changed by a subsequent transaction, but history cannot be changed, only added to." .

odm:Criterion a owl:Class,
        linkml:ClassDefinition ;
    rdfs:label "Criterion" ;
    rdfs:subClassOf [ a owl:Restriction ;
            owl:onClass odm:Oidref ;
            owl:onProperty odm:ConditionOID ;
            owl:qualifiedCardinality 1 ],
        [ a owl:Restriction ;
            owl:maxQualifiedCardinality 1 ;
            owl:onClass odm:Description ;
            owl:onProperty odm:DescriptionRef ],
        [ a owl:Restriction ;
            owl:onClass odm:Oid ;
            owl:onProperty odm:OID ;
            owl:qualifiedCardinality 1 ],
        [ a owl:Restriction ;
            owl:onClass odm:Name ;
            owl:onProperty odm:Name ;
            owl:qualifiedCardinality 1 ],
        [ a owl:Restriction ;
            owl:allValuesFrom odm:Coding ;
            owl:onProperty odm:CodingRef ] ;
    skos:definition "The Criterion represents either an inclusion or an exclusion criterion, depending on the parent element (i.e., InclusionCriteria, ExclusionCriteria)." ;
    skos:exactMatch odm:Criterion .

odm:ItemGroupData a owl:Class,
        linkml:ClassDefinition ;
    rdfs:label "ItemGroupData" ;
    rdfs:subClassOf [ a owl:Restriction ;
            owl:onClass odm:Oidref ;
            owl:onProperty odm:ItemGroupOID ;
            owl:qualifiedCardinality 1 ],
        [ a owl:Restriction ;
            owl:maxQualifiedCardinality 1 ;
            owl:onClass odm:Signature ;
            owl:onProperty odm:SignatureRefRef ],
        [ a owl:Restriction ;
            owl:maxQualifiedCardinality 1 ;
            owl:onClass odm:PositiveInteger ;
            owl:onProperty odm:ItemGroupDataSeq ],
        [ a owl:Restriction ;
            owl:maxQualifiedCardinality 1 ;
            owl:onClass odm:AuditRecord ;
            owl:onProperty odm:AuditRecordRef ],
        [ a owl:Restriction ;
            owl:allValuesFrom odm:Query ;
            owl:onProperty odm:QueryRef ],
        [ a owl:Restriction ;
            owl:allValuesFrom odm:ItemData ;
            owl:onProperty odm:ItemDataRef ],
        [ a owl:Restriction ;
            owl:maxQualifiedCardinality 1 ;
            owl:onClass odm:TransactionType ;
            owl:onProperty odm:TransactionTypeRef ],
        [ a owl:Restriction ;
            owl:maxQualifiedCardinality 1 ;
            owl:onClass odm:Annotation ;
            owl:onProperty odm:AnnotationRef ],
        [ a owl:Restriction ;
            owl:maxQualifiedCardinality 1 ;
            owl:onClass odm:RepeatKey ;
            owl:onProperty odm:ItemGroupRepeatKey ],
        [ a owl:Restriction ;
            owl:allValuesFrom odm:ItemGroupData ;
            owl:onProperty odm:ItemGroupDataRef ] ;
    skos:definition "Clinical data corresponding to an ItemGroupRef defined in the active MetaDataVersion." ;
    skos:exactMatch odm:ItemGroupData .

odm:MetaDataVersionOID a owl:ObjectProperty,
        linkml:SlotDefinition ;
    rdfs:label "MetaDataVersionOID" ;
    rdfs:range odm:Oidref ;
    skos:definition "References a prior MetaDataVersion within the Study referenced by the StudyOID attribute." .

odm:OrganizationType a owl:Class,
        linkml:EnumDefinition ;
    rdfs:label "OrganizationType" ;
    owl:unionOf ( <http://www.cdisc.org/ns/odm/v2.0/OrganizationType#Sponsor> <http://www.cdisc.org/ns/odm/v2.0/OrganizationType#Site> <http://www.cdisc.org/ns/odm/v2.0/OrganizationType#CRO> <http://www.cdisc.org/ns/odm/v2.0/OrganizationType#Lab> <http://www.cdisc.org/ns/odm/v2.0/OrganizationType#Other> <http://www.cdisc.org/ns/odm/v2.0/OrganizationType#TechnologyProvider> ) ;
    linkml:permissible_values <http://www.cdisc.org/ns/odm/v2.0/OrganizationType#CRO>,
        <http://www.cdisc.org/ns/odm/v2.0/OrganizationType#Lab>,
        <http://www.cdisc.org/ns/odm/v2.0/OrganizationType#Other>,
        <http://www.cdisc.org/ns/odm/v2.0/OrganizationType#Site>,
        <http://www.cdisc.org/ns/odm/v2.0/OrganizationType#Sponsor>,
        <http://www.cdisc.org/ns/odm/v2.0/OrganizationType#TechnologyProvider> .

odm:SignatureRefRef a owl:ObjectProperty,
        linkml:SlotDefinition ;
    rdfs:label "SignatureRefRef" ;
    rdfs:range odm:SignatureRef ;
    skos:definition "SignatureRef reference: None" .

odm:StandardPublishingSet a owl:Class,
        linkml:EnumDefinition ;
    rdfs:label "StandardPublishingSet" ;
    owl:unionOf ( <http://ncicb.nci.nih.gov/xml/odm/EVS/CDISCExtCodeID:C180548> <http://ncicb.nci.nih.gov/xml/odm/EVS/CDISCExtCodeID:C180549> <http://ncicb.nci.nih.gov/xml/odm/EVS/CDISCExtCodeID:C180550> <http://ncicb.nci.nih.gov/xml/odm/EVS/CDISCExtCodeID:C180551> <http://ncicb.nci.nih.gov/xml/odm/EVS/CDISCExtCodeID:C180552> ) ;
    linkml:permissible_values <http://ncicb.nci.nih.gov/xml/odm/EVS/CDISCExtCodeID:C180548>,
        <http://ncicb.nci.nih.gov/xml/odm/EVS/CDISCExtCodeID:C180549>,
        <http://ncicb.nci.nih.gov/xml/odm/EVS/CDISCExtCodeID:C180550>,
        <http://ncicb.nci.nih.gov/xml/odm/EVS/CDISCExtCodeID:C180551>,
        <http://ncicb.nci.nih.gov/xml/odm/EVS/CDISCExtCodeID:C180552> .

odm:Uriorcurie a owl:Class,
        linkml:TypeDefinition ;
    rdfs:label "uriorcurie" ;
    rdfs:subClassOf [ a owl:Restriction ;
            owl:onDataRange xsd:anyURI ;
            owl:onProperty linkml:topValue ;
            owl:qualifiedCardinality 1 ] .

odm:Value a owl:Class,
        linkml:ClassDefinition,
        linkml:TypeDefinition ;
    rdfs:label "Value",
        "value" ;
    rdfs:subClassOf [ a owl:Restriction ;
            owl:onDataRange odm:value ;
            owl:onProperty linkml:topValue ;
            owl:qualifiedCardinality 1 ],
        [ a owl:Restriction ;
            owl:maxQualifiedCardinality 1 ;
            owl:onClass odm:Text ;
            owl:onProperty odm:_content ],
        [ a owl:Restriction ;
            owl:maxQualifiedCardinality 1 ;
            owl:onClass odm:PositiveInteger ;
            owl:onProperty odm:SeqNum ] ;
    skos:definition "The data collected for an item. This data is represented according to DataType attribute of the ItemDef referenced by the ItemOID attribute in the parent ItemData element." ;
    skos:exactMatch odm:Value .

odm:WorkflowRefRef a owl:ObjectProperty,
        linkml:SlotDefinition ;
    rdfs:label "WorkflowRefRef" ;
    rdfs:range odm:WorkflowRef ;
    skos:definition "WorkflowRef reference: The WorkflowRef references a workflow definition" .

odm:AliasRef a owl:ObjectProperty,
        linkml:SlotDefinition ;
    rdfs:label "AliasRef" ;
    rdfs:range odm:Alias ;
    skos:definition "Alias reference: An Alias provides an additional name for an element. The Context attribute specifies the application domain in which this additional name is relevant." .

odm:Decimal a owl:Class,
        linkml:TypeDefinition ;
    rdfs:label "decimal" ;
    rdfs:subClassOf [ a owl:Restriction ;
            owl:onDataRange xsd:decimal ;
            owl:onProperty linkml:topValue ;
            owl:qualifiedCardinality 1 ] .

odm:DocumentRef a owl:Class,
        linkml:ClassDefinition ;
    rdfs:label "DocumentRef" ;
    rdfs:subClassOf [ a owl:Restriction ;
            owl:onClass odm:Oid ;
            owl:onProperty odm:LeafID ;
            owl:qualifiedCardinality 1 ],
        [ a owl:Restriction ;
            owl:allValuesFrom odm:PDFPageRef ;
            owl:onProperty odm:PDFPageRefRef ] ;
    skos:definition "Links to a leaf element with the location of the document." ;
    skos:exactMatch odm:DocumentRef .

odm:FormalExpression a owl:Class,
        linkml:ClassDefinition ;
    rdfs:label "FormalExpression" ;
    rdfs:subClassOf [ a owl:Restriction ;
            owl:maxQualifiedCardinality 1 ;
            owl:onClass odm:Text ;
            owl:onProperty odm:ContextRef ],
        [ a owl:Restriction ;
            owl:maxQualifiedCardinality 1 ;
            owl:onClass odm:ExternalCodeLib ;
            owl:onProperty odm:ExternalCodeLibRef ],
        [ a owl:Restriction ;
            owl:maxQualifiedCardinality 1 ;
            owl:onClass odm:Code ;
            owl:onProperty odm:CodeRef ] ;
    skos:definition "A FormalExpression used within a ConditionDef or a RangeCheck must evaluate to True or False. A FormalExpression referenced within a MethodDef having Type Imputation, Computation, or Transpose must evaluate to the correct DataType for an Item that may be imputed or computed using the Method. A FormalExpression gets parameter and return value definitions from the MethodSignature element. The data types in the MethodSignature parameters and return values must match the corresponding data types in the FormalExpression." ;
    skos:exactMatch odm:FormalExpression .

odm:OrderNumber a owl:ObjectProperty,
        linkml:SlotDefinition ;
    rdfs:label "OrderNumber" ;
    rdfs:range odm:PositiveInteger ;
    skos:definition "Indicates the order in which this StudyEventGroup appears in Metadata displays or data entry applications." .

odm:QueryStateType a owl:Class,
        linkml:EnumDefinition ;
    rdfs:label "QueryStateType" ;
    owl:unionOf ( <http://www.cdisc.org/ns/odm/v2.0/QueryStateType#Candidate> <http://www.cdisc.org/ns/odm/v2.0/QueryStateType#Open> <http://www.cdisc.org/ns/odm/v2.0/QueryStateType#Answered> <http://www.cdisc.org/ns/odm/v2.0/QueryStateType#Closed> <http://www.cdisc.org/ns/odm/v2.0/QueryStateType#Cancelled> <http://www.cdisc.org/ns/odm/v2.0/QueryStateType#Resolved> ) ;
    linkml:permissible_values <http://www.cdisc.org/ns/odm/v2.0/QueryStateType#Answered>,
        <http://www.cdisc.org/ns/odm/v2.0/QueryStateType#Cancelled>,
        <http://www.cdisc.org/ns/odm/v2.0/QueryStateType#Candidate>,
        <http://www.cdisc.org/ns/odm/v2.0/QueryStateType#Closed>,
        <http://www.cdisc.org/ns/odm/v2.0/QueryStateType#Open>,
        <http://www.cdisc.org/ns/odm/v2.0/QueryStateType#Resolved> .

odm:Signature a owl:Class,
        linkml:ClassDefinition ;
    rdfs:label "Signature" ;
    rdfs:subClassOf [ a owl:Restriction ;
            owl:maxQualifiedCardinality 1 ;
            owl:onClass odm:SignatureRef ;
            owl:onProperty odm:SignatureRefRef ],
        [ a owl:Restriction ;
            owl:maxQualifiedCardinality 1 ;
            owl:onClass odm:DateTimeStamp ;
            owl:onProperty odm:DateTimeStampRef ],
        [ a owl:Restriction ;
            owl:onClass odm:Oid ;
            owl:onProperty odm:ID ;
            owl:qualifiedCardinality 1 ],
        [ a owl:Restriction ;
            owl:maxQualifiedCardinality 1 ;
            owl:onClass odm:UserRef ;
            owl:onProperty odm:UserRefRef ],
        [ a owl:Restriction ;
            owl:maxQualifiedCardinality 1 ;
            owl:onClass odm:LocationRef ;
            owl:onProperty odm:LocationRefRef ] ;
    skos:definition "An electronic signature applies to a collection of clinical data. This indicates that some user accepts legal responsibility for that data. See 21 CFR Part 11. The signature identifies the person signing, the location of signing, the signature meaning (via the referenced SignatureDef), the date and time of signing, and (in the case of a digital signature) an encrypted hash of the included data." ;
    skos:exactMatch odm:Signature .

odm:StudyOID a owl:ObjectProperty,
        linkml:SlotDefinition ;
    rdfs:label "StudyOID" ;
    rdfs:range odm:Oidref ;
    skos:definition "References the Study that provides a prior metadata version. This attribute allows an Include element to reference a metadata version in another study. Thus, it is possible for many studies to share a set of common metadata definitions" .

odm:Granularity a owl:Class,
        linkml:EnumDefinition ;
    rdfs:label "Granularity" ;
    owl:unionOf ( <http://www.cdisc.org/ns/odm/v2.0/Granularity#All> <http://www.cdisc.org/ns/odm/v2.0/Granularity#Metadata> <http://www.cdisc.org/ns/odm/v2.0/Granularity#AdminData> <http://www.cdisc.org/ns/odm/v2.0/Granularity#ReferenceData> <http://www.cdisc.org/ns/odm/v2.0/Granularity#AllClinicalData> <http://www.cdisc.org/ns/odm/v2.0/Granularity#SingleSite> <http://www.cdisc.org/ns/odm/v2.0/Granularity#SingleSubject> ) ;
    linkml:permissible_values <http://www.cdisc.org/ns/odm/v2.0/Granularity#AdminData>,
        <http://www.cdisc.org/ns/odm/v2.0/Granularity#All>,
        <http://www.cdisc.org/ns/odm/v2.0/Granularity#AllClinicalData>,
        <http://www.cdisc.org/ns/odm/v2.0/Granularity#Metadata>,
        <http://www.cdisc.org/ns/odm/v2.0/Granularity#ReferenceData>,
        <http://www.cdisc.org/ns/odm/v2.0/Granularity#SingleSite>,
        <http://www.cdisc.org/ns/odm/v2.0/Granularity#SingleSubject> .

odm:OriginType a owl:Class,
        linkml:EnumDefinition ;
    rdfs:label "OriginType" ;
    owl:unionOf ( <http://ncicb.nci.nih.gov/xml/odm/EVS/CDISCExtCodeID:C170547> <http://ncicb.nci.nih.gov/xml/odm/EVS/CDISCExtCodeID:C170548> <http://ncicb.nci.nih.gov/xml/odm/EVS/CDISCExtCodeID:C170549> <http://www.cdisc.org/ns/odm/v2.0/OriginType#EHR> <http://ncicb.nci.nih.gov/xml/odm/EVS/CDISCExtCodeID:C126101> <http://ncicb.nci.nih.gov/xml/odm/EVS/CDISCExtCodeID:C17649> <http://ncicb.nci.nih.gov/xml/odm/EVS/CDISCExtCodeID:C170550> <http://ncicb.nci.nih.gov/xml/odm/EVS/CDISCExtCodeID:C170551> ) ;
    linkml:permissible_values <http://ncicb.nci.nih.gov/xml/odm/EVS/CDISCExtCodeID:C126101>,
        <http://ncicb.nci.nih.gov/xml/odm/EVS/CDISCExtCodeID:C170547>,
        <http://ncicb.nci.nih.gov/xml/odm/EVS/CDISCExtCodeID:C170548>,
        <http://ncicb.nci.nih.gov/xml/odm/EVS/CDISCExtCodeID:C170549>,
        <http://ncicb.nci.nih.gov/xml/odm/EVS/CDISCExtCodeID:C170550>,
        <http://ncicb.nci.nih.gov/xml/odm/EVS/CDISCExtCodeID:C170551>,
        <http://ncicb.nci.nih.gov/xml/odm/EVS/CDISCExtCodeID:C17649>,
        <http://www.cdisc.org/ns/odm/v2.0/OriginType#EHR> .

odm:Query a owl:Class,
        linkml:ClassDefinition ;
    rdfs:label "Query" ;
    rdfs:subClassOf [ a owl:Restriction ;
            owl:maxQualifiedCardinality 1 ;
            owl:onClass odm:Name ;
            owl:onProperty odm:Name ],
        [ a owl:Restriction ;
            owl:maxQualifiedCardinality 1 ;
            owl:onClass odm:Text ;
            owl:onProperty odm:Target ],
        [ a owl:Restriction ;
            owl:onClass odm:QuerySourceType ;
            owl:onProperty odm:Source ;
            owl:qualifiedCardinality 1 ],
        [ a owl:Restriction ;
            owl:onClass odm:Oid ;
            owl:onProperty odm:OID ;
            owl:qualifiedCardinality 1 ],
        [ a owl:Restriction ;
            owl:allValuesFrom odm:AuditRecord ;
            owl:onProperty odm:AuditRecordRef ],
        [ a owl:Restriction ;
            owl:maxQualifiedCardinality 1 ;
            owl:onClass odm:Value ;
            owl:onProperty odm:ValueRef ],
        [ a owl:Restriction ;
            owl:maxQualifiedCardinality 1 ;
            owl:onClass odm:QueryType ;
            owl:onProperty odm:Type ],
        [ a owl:Restriction ;
            owl:onClass odm:QueryStateType ;
            owl:onProperty odm:State ;
            owl:qualifiedCardinality 1 ],
        [ a owl:Restriction ;
            owl:onClass odm:Datetime ;
            owl:onProperty odm:LastUpdateDatetime ;
            owl:qualifiedCardinality 1 ] ;
    skos:definition "The Query element represents a request for clarification on a data item collected for a clinical trial, specifically a request from a sponsor or sponsor’s representative to an investigator to resolve an error or inconsistency discovered during data review. Queries can be created manually by individuals such as site monitors or data managers or automatically by systems. The full text of the Query exists in the Value child element. The optional Name attribute provide the means to provide a short identifier that can be included in listing or user interfaces." ;
    skos:exactMatch odm:Query .

odm:StandardName a owl:Class,
        linkml:EnumDefinition ;
    rdfs:label "StandardName" ;
    owl:unionOf ( <http://ncicb.nci.nih.gov/xml/odm/EVS/CDISCExtCodeID:C170552> <http://ncicb.nci.nih.gov/xml/odm/EVS/CDISCExtCodeID:C163415> <http://ncicb.nci.nih.gov/xml/odm/EVS/CDISCExtCodeID:C170455> <http://ncicb.nci.nih.gov/xml/odm/EVS/CDISCExtCodeID:C170553> <http://ncicb.nci.nih.gov/xml/odm/EVS/CDISCExtCodeID:C170554> <http://ncicb.nci.nih.gov/xml/odm/EVS/CDISCExtCodeID:C170456> <http://ncicb.nci.nih.gov/xml/odm/EVS/CDISCExtCodeID:C181230> <http://ncicb.nci.nih.gov/xml/odm/EVS/CDISCExtCodeID:C170556> ) ;
    linkml:permissible_values <http://ncicb.nci.nih.gov/xml/odm/EVS/CDISCExtCodeID:C163415>,
        <http://ncicb.nci.nih.gov/xml/odm/EVS/CDISCExtCodeID:C170455>,
        <http://ncicb.nci.nih.gov/xml/odm/EVS/CDISCExtCodeID:C170456>,
        <http://ncicb.nci.nih.gov/xml/odm/EVS/CDISCExtCodeID:C170552>,
        <http://ncicb.nci.nih.gov/xml/odm/EVS/CDISCExtCodeID:C170553>,
        <http://ncicb.nci.nih.gov/xml/odm/EVS/CDISCExtCodeID:C170554>,
        <http://ncicb.nci.nih.gov/xml/odm/EVS/CDISCExtCodeID:C170556>,
        <http://ncicb.nci.nih.gov/xml/odm/EVS/CDISCExtCodeID:C181230> .

odm:TelecomTypeType a owl:Class,
        linkml:EnumDefinition ;
    rdfs:label "TelecomTypeType" ;
    owl:unionOf ( <http://www.cdisc.org/ns/odm/v2.0/TelecomTypeType#Email> <http://www.cdisc.org/ns/odm/v2.0/TelecomTypeType#Pager> <http://www.cdisc.org/ns/odm/v2.0/TelecomTypeType#Phone> <http://www.cdisc.org/ns/odm/v2.0/TelecomTypeType#Fax> <http://www.cdisc.org/ns/odm/v2.0/TelecomTypeType#SMS> <http://www.cdisc.org/ns/odm/v2.0/TelecomTypeType#URL> <http://www.cdisc.org/ns/odm/v2.0/TelecomTypeType#Other> ) ;
    linkml:permissible_values <http://www.cdisc.org/ns/odm/v2.0/TelecomTypeType#Email>,
        <http://www.cdisc.org/ns/odm/v2.0/TelecomTypeType#Fax>,
        <http://www.cdisc.org/ns/odm/v2.0/TelecomTypeType#Other>,
        <http://www.cdisc.org/ns/odm/v2.0/TelecomTypeType#Pager>,
        <http://www.cdisc.org/ns/odm/v2.0/TelecomTypeType#Phone>,
        <http://www.cdisc.org/ns/odm/v2.0/TelecomTypeType#SMS>,
        <http://www.cdisc.org/ns/odm/v2.0/TelecomTypeType#URL> .

odm:Annotation a owl:Class,
        linkml:ClassDefinition ;
    rdfs:label "Annotation" ;
    rdfs:subClassOf [ a owl:Restriction ;
            owl:maxQualifiedCardinality 1 ;
            owl:onClass odm:TransactionType ;
            owl:onProperty odm:TransactionTypeRef ],
        [ a owl:Restriction ;
            owl:maxQualifiedCardinality 1 ;
            owl:onClass odm:Comment ;
            owl:onProperty odm:CommentRef ],
        [ a owl:Restriction ;
            owl:allValuesFrom odm:Flag ;
            owl:onProperty odm:FlagRef ],
        [ a owl:Restriction ;
            owl:onClass odm:PositiveInteger ;
            owl:onProperty odm:SeqNum ;
            owl:qualifiedCardinality 1 ],
        [ a owl:Restriction ;
            owl:allValuesFrom odm:Coding ;
            owl:onProperty odm:CodingRef ],
        [ a owl:Restriction ;
            owl:onClass odm:Oid ;
            owl:onProperty odm:ID ;
            owl:qualifiedCardinality 1 ] ;
    skos:definition "A general note about clinical data. If an annotation has both a comment and flags, the flags should be related to the comment." ;
    skos:exactMatch odm:Annotation .

odm:AuditRecord a owl:Class,
        linkml:ClassDefinition ;
    rdfs:label "AuditRecord" ;
    rdfs:subClassOf [ a owl:Restriction ;
            owl:maxQualifiedCardinality 1 ;
            owl:onClass odm:UserRef ;
            owl:onProperty odm:UserRefRef ],
        [ a owl:Restriction ;
            owl:maxQualifiedCardinality 1 ;
            owl:onClass odm:EditPointType ;
            owl:onProperty odm:EditPoint ],
        [ a owl:Restriction ;
            owl:maxQualifiedCardinality 1 ;
            owl:onClass odm:LocationRef ;
            owl:onProperty odm:LocationRefRef ],
        [ a owl:Restriction ;
            owl:maxQualifiedCardinality 1 ;
            owl:onClass odm:YesOrNo ;
            owl:onProperty odm:UsedMethod ],
        [ a owl:Restriction ;
            owl:maxQualifiedCardinality 1 ;
            owl:onClass odm:DateTimeStamp ;
            owl:onProperty odm:DateTimeStampRef ],
        [ a owl:Restriction ;
            owl:maxQualifiedCardinality 1 ;
            owl:onClass odm:SourceID ;
            owl:onProperty odm:SourceIDRef ],
        [ a owl:Restriction ;
            owl:maxQualifiedCardinality 1 ;
            owl:onClass odm:ReasonForChange ;
            owl:onProperty odm:ReasonForChangeRef ] ;
    skos:definition "An AuditRecord carries information pertaining to the creation, deletion, or modification of clinical data. This information includes who performed that action, and where, when, and why that action was performed.AuditRecord information describes a change to clinical data, but is not itself clinical data. The value of some clinical data can always be changed by a subsequent transaction, but history cannot be changed, only added to." ;
    skos:exactMatch odm:AuditRecord .

odm:Comparator a owl:Class,
        linkml:EnumDefinition ;
    rdfs:label "Comparator" ;
    owl:unionOf ( <http://www.cdisc.org/ns/odm/v2.0/Comparator#LT> <http://www.cdisc.org/ns/odm/v2.0/Comparator#LE> <http://www.cdisc.org/ns/odm/v2.0/Comparator#GT> <http://www.cdisc.org/ns/odm/v2.0/Comparator#GE> <http://www.cdisc.org/ns/odm/v2.0/Comparator#EQ> <http://www.cdisc.org/ns/odm/v2.0/Comparator#NE> <http://www.cdisc.org/ns/odm/v2.0/Comparator#IN> <http://www.cdisc.org/ns/odm/v2.0/Comparator#NOTIN> ) ;
    linkml:permissible_values <http://www.cdisc.org/ns/odm/v2.0/Comparator#EQ>,
        <http://www.cdisc.org/ns/odm/v2.0/Comparator#GE>,
        <http://www.cdisc.org/ns/odm/v2.0/Comparator#GT>,
        <http://www.cdisc.org/ns/odm/v2.0/Comparator#IN>,
        <http://www.cdisc.org/ns/odm/v2.0/Comparator#LE>,
        <http://www.cdisc.org/ns/odm/v2.0/Comparator#LT>,
        <http://www.cdisc.org/ns/odm/v2.0/Comparator#NE>,
        <http://www.cdisc.org/ns/odm/v2.0/Comparator#NOTIN> .

odm:TranslatedTextRef a owl:ObjectProperty,
        linkml:SlotDefinition ;
    rdfs:label "TranslatedTextRef" ;
    rdfs:range odm:TranslatedText ;
    skos:definition "TranslatedText reference: Human-readable text that is appropriate for a particular language. TranslatedText elements typically occur in a series, presenting a set of alternative textual renditions for different languages and types." .

odm:WorkflowRef a owl:Class,
        linkml:ClassDefinition ;
    rdfs:label "WorkflowRef" ;
    rdfs:subClassOf [ a owl:Restriction ;
            owl:onClass odm:Oidref ;
            owl:onProperty odm:WorkflowOID ;
            owl:qualifiedCardinality 1 ] ;
    skos:definition "The WorkflowRef references a workflow definition" ;
    skos:exactMatch odm:WorkflowRef .

odm:Alias a owl:Class,
        linkml:ClassDefinition ;
    rdfs:label "Alias" ;
    rdfs:subClassOf [ a owl:Restriction ;
            owl:onClass odm:Text ;
            owl:onProperty odm:ContextRef ;
            owl:qualifiedCardinality 1 ],
        [ a owl:Restriction ;
            owl:onClass odm:Text ;
            owl:onProperty odm:Name ;
            owl:qualifiedCardinality 1 ] ;
    skos:definition "An Alias provides an additional name for an element. The Context attribute specifies the application domain in which this additional name is relevant." ;
    skos:exactMatch odm:Alias .

odm:TransactionType a owl:Class,
        linkml:EnumDefinition ;
    rdfs:label "TransactionType" ;
    owl:unionOf ( <http://www.cdisc.org/ns/odm/v2.0/TransactionType#Insert> <http://www.cdisc.org/ns/odm/v2.0/TransactionType#Update> <http://www.cdisc.org/ns/odm/v2.0/TransactionType#Remove> <http://www.cdisc.org/ns/odm/v2.0/TransactionType#Upsert> <http://www.cdisc.org/ns/odm/v2.0/TransactionType#Context> ) ;
    linkml:permissible_values <http://www.cdisc.org/ns/odm/v2.0/TransactionType#Context>,
        <http://www.cdisc.org/ns/odm/v2.0/TransactionType#Insert>,
        <http://www.cdisc.org/ns/odm/v2.0/TransactionType#Remove>,
        <http://www.cdisc.org/ns/odm/v2.0/TransactionType#Update>,
        <http://www.cdisc.org/ns/odm/v2.0/TransactionType#Upsert> .

odm:UserType a owl:Class,
        linkml:EnumDefinition ;
    rdfs:label "UserType" ;
    owl:unionOf ( <http://www.cdisc.org/ns/odm/v2.0/UserType#Sponsor> <http://www.cdisc.org/ns/odm/v2.0/UserType#Investigator> <http://www.cdisc.org/ns/odm/v2.0/UserType#Lab> <http://www.cdisc.org/ns/odm/v2.0/UserType#Other> <http://www.cdisc.org/ns/odm/v2.0/UserType#Subject> <http://www.cdisc.org/ns/odm/v2.0/UserType#Monitor> <http://www.cdisc.org/ns/odm/v2.0/UserType#Data+analyst> <http://www.cdisc.org/ns/odm/v2.0/UserType#Care+provider> <http://www.cdisc.org/ns/odm/v2.0/UserType#Assessor> ) ;
    linkml:permissible_values <http://www.cdisc.org/ns/odm/v2.0/UserType#Assessor>,
        <http://www.cdisc.org/ns/odm/v2.0/UserType#Care+provider>,
        <http://www.cdisc.org/ns/odm/v2.0/UserType#Data+analyst>,
        <http://www.cdisc.org/ns/odm/v2.0/UserType#Investigator>,
        <http://www.cdisc.org/ns/odm/v2.0/UserType#Lab>,
        <http://www.cdisc.org/ns/odm/v2.0/UserType#Monitor>,
        <http://www.cdisc.org/ns/odm/v2.0/UserType#Other>,
        <http://www.cdisc.org/ns/odm/v2.0/UserType#Sponsor>,
        <http://www.cdisc.org/ns/odm/v2.0/UserType#Subject> .

odm:CommentOID a owl:ObjectProperty,
        linkml:SlotDefinition ;
    rdfs:label "CommentOID" ;
    rdfs:range odm:String ;
    skos:definition """The Comment identifier that this value refers to. Needed when the WhereClause references Items across different domains.
                The Comment would define any join assumptions.""" .

odm:YesOrNo a owl:Class,
        linkml:EnumDefinition ;
    rdfs:label "YesOrNo" ;
    owl:unionOf ( <http://www.cdisc.org/ns/odm/v2.0/YesOrNo#Yes> <http://www.cdisc.org/ns/odm/v2.0/YesOrNo#No> ) ;
    linkml:permissible_values <http://www.cdisc.org/ns/odm/v2.0/YesOrNo#No>,
        <http://www.cdisc.org/ns/odm/v2.0/YesOrNo#Yes> .

odm:DictionaryNameTypeEnum a owl:Class,
        linkml:EnumDefinition ;
    rdfs:label "DictionaryNameTypeEnum" ;
    owl:unionOf ( <http://ncicb.nci.nih.gov/xml/odm/EVS/CDISCExtCodeID:C163415> <http://ncicb.nci.nih.gov/xml/odm/EVS/CDISCExtCodeID:C49471> <http://ncicb.nci.nih.gov/xml/odm/EVS/CDISCExtCodeID:C49704> <http://ncicb.nci.nih.gov/xml/odm/EVS/CDISCExtCodeID:C134003> <http://ncicb.nci.nih.gov/xml/odm/EVS/CDISCExtCodeID:C49474> <http://ncicb.nci.nih.gov/xml/odm/EVS/CDISCExtCodeID:C49476> <http://ncicb.nci.nih.gov/xml/odm/EVS/CDISCExtCodeID:C163416> <http://ncicb.nci.nih.gov/xml/odm/EVS/CDISCExtCodeID:C43820> <http://ncicb.nci.nih.gov/xml/odm/EVS/CDISCExtCodeID:C53489> <http://ncicb.nci.nih.gov/xml/odm/EVS/CDISCExtCodeID:C163417> <http://ncicb.nci.nih.gov/xml/odm/EVS/CDISCExtCodeID:C154331> <http://ncicb.nci.nih.gov/xml/odm/EVS/CDISCExtCodeID:C49468> <http://ncicb.nci.nih.gov/xml/odm/EVS/CDISCExtCodeID:C49475> ) ;
    linkml:permissible_values <http://ncicb.nci.nih.gov/xml/odm/EVS/CDISCExtCodeID:C134003>,
        <http://ncicb.nci.nih.gov/xml/odm/EVS/CDISCExtCodeID:C154331>,
        <http://ncicb.nci.nih.gov/xml/odm/EVS/CDISCExtCodeID:C163415>,
        <http://ncicb.nci.nih.gov/xml/odm/EVS/CDISCExtCodeID:C163416>,
        <http://ncicb.nci.nih.gov/xml/odm/EVS/CDISCExtCodeID:C163417>,
        <http://ncicb.nci.nih.gov/xml/odm/EVS/CDISCExtCodeID:C43820>,
        <http://ncicb.nci.nih.gov/xml/odm/EVS/CDISCExtCodeID:C49468>,
        <http://ncicb.nci.nih.gov/xml/odm/EVS/CDISCExtCodeID:C49471>,
        <http://ncicb.nci.nih.gov/xml/odm/EVS/CDISCExtCodeID:C49474>,
        <http://ncicb.nci.nih.gov/xml/odm/EVS/CDISCExtCodeID:C49475>,
        <http://ncicb.nci.nih.gov/xml/odm/EVS/CDISCExtCodeID:C49476>,
        <http://ncicb.nci.nih.gov/xml/odm/EVS/CDISCExtCodeID:C49704>,
        <http://ncicb.nci.nih.gov/xml/odm/EVS/CDISCExtCodeID:C53489> .

odm:TranslatedText a owl:Class,
        linkml:ClassDefinition ;
    rdfs:label "TranslatedText" ;
    rdfs:subClassOf [ a owl:Restriction ;
            owl:onClass odm:Text ;
            owl:onProperty odm:Type ;
            owl:qualifiedCardinality 1 ],
        [ a owl:Restriction ;
            owl:maxQualifiedCardinality 1 ;
            owl:onClass odm:ContentType ;
            owl:onProperty odm:_content ],
        [ a owl:Restriction ;
            owl:maxQualifiedCardinality 1 ;
            owl:onClass odm:LanguageType ;
            owl:onProperty odm:_language ] ;
    skos:definition "Human-readable text that is appropriate for a particular language. TranslatedText elements typically occur in a series, presenting a set of alternative textual renditions for different languages and types." ;
    skos:exactMatch odm:TranslatedText .

odm:TrialPhaseTypeEnum a owl:Class,
        linkml:EnumDefinition ;
    rdfs:label "TrialPhaseTypeEnum" ;
    owl:unionOf ( <http://ncicb.nci.nih.gov/xml/odm/EVS/CDISCExtCodeID:C48660> <http://ncicb.nci.nih.gov/xml/odm/EVS/CDISCExtCodeID:C54721> <http://ncicb.nci.nih.gov/xml/odm/EVS/CDISCExtCodeID:C15600> <http://ncicb.nci.nih.gov/xml/odm/EVS/CDISCExtCodeID:C15693> <http://ncicb.nci.nih.gov/xml/odm/EVS/CDISCExtCodeID:C15601> <http://ncicb.nci.nih.gov/xml/odm/EVS/CDISCExtCodeID:C15694> <http://ncicb.nci.nih.gov/xml/odm/EVS/CDISCExtCodeID:C49686> <http://ncicb.nci.nih.gov/xml/odm/EVS/CDISCExtCodeID:C49688> <http://ncicb.nci.nih.gov/xml/odm/EVS/CDISCExtCodeID:C15602> <http://ncicb.nci.nih.gov/xml/odm/EVS/CDISCExtCodeID:C49687> <http://ncicb.nci.nih.gov/xml/odm/EVS/CDISCExtCodeID:C49689> <http://ncicb.nci.nih.gov/xml/odm/EVS/CDISCExtCodeID:C15603> <http://ncicb.nci.nih.gov/xml/odm/EVS/CDISCExtCodeID:C47865> ) ;
    linkml:permissible_values <http://ncicb.nci.nih.gov/xml/odm/EVS/CDISCExtCodeID:C15600>,
        <http://ncicb.nci.nih.gov/xml/odm/EVS/CDISCExtCodeID:C15601>,
        <http://ncicb.nci.nih.gov/xml/odm/EVS/CDISCExtCodeID:C15602>,
        <http://ncicb.nci.nih.gov/xml/odm/EVS/CDISCExtCodeID:C15603>,
        <http://ncicb.nci.nih.gov/xml/odm/EVS/CDISCExtCodeID:C15693>,
        <http://ncicb.nci.nih.gov/xml/odm/EVS/CDISCExtCodeID:C15694>,
        <http://ncicb.nci.nih.gov/xml/odm/EVS/CDISCExtCodeID:C47865>,
        <http://ncicb.nci.nih.gov/xml/odm/EVS/CDISCExtCodeID:C48660>,
        <http://ncicb.nci.nih.gov/xml/odm/EVS/CDISCExtCodeID:C49686>,
        <http://ncicb.nci.nih.gov/xml/odm/EVS/CDISCExtCodeID:C49687>,
        <http://ncicb.nci.nih.gov/xml/odm/EVS/CDISCExtCodeID:C49688>,
        <http://ncicb.nci.nih.gov/xml/odm/EVS/CDISCExtCodeID:C49689>,
        <http://ncicb.nci.nih.gov/xml/odm/EVS/CDISCExtCodeID:C54721> .

odm:Type a owl:ObjectProperty,
        linkml:SlotDefinition ;
    rdfs:label "Type" ;
    rdfs:range odm:String ;
    skos:definition "Type of page for page references indicated in the PageRefs attribute." .

odm:CodingRef a owl:ObjectProperty,
        linkml:SlotDefinition ;
    rdfs:label "CodingRef" ;
    rdfs:range odm:Coding ;
    skos:definition "Coding reference: Coding references a symbol from a defined code system. It uses a code defined in a terminology system to associate semantics with a given term, codelist, variable, or group of variables. The presence of a Coding element associates a meaning to its parent element. Including multiple Coding elements for a given parent indicates synonymous meanings provided by different code systems or code system versions." .

odm:ItemGroupClass a owl:Class,
        linkml:EnumDefinition ;
    rdfs:label "ItemGroupClass" ;
    owl:unionOf ( <http://ncicb.nci.nih.gov/xml/odm/EVS/CDISCExtCodeID:C103375> <http://ncicb.nci.nih.gov/xml/odm/EVS/CDISCExtCodeID:C103371> <http://ncicb.nci.nih.gov/xml/odm/EVS/CDISCExtCodeID:C177921> <http://ncicb.nci.nih.gov/xml/odm/EVS/CDISCExtCodeID:C103372> <http://ncicb.nci.nih.gov/xml/odm/EVS/CDISCExtCodeID:C103373> <http://ncicb.nci.nih.gov/xml/odm/EVS/CDISCExtCodeID:C135396> <http://ncicb.nci.nih.gov/xml/odm/EVS/CDISCExtCodeID:C103374> <http://ncicb.nci.nih.gov/xml/odm/EVS/CDISCExtCodeID:C177922> <http://ncicb.nci.nih.gov/xml/odm/EVS/CDISCExtCodeID:C177923> <http://ncicb.nci.nih.gov/xml/odm/EVS/CDISCExtCodeID:C123454> <http://ncicb.nci.nih.gov/xml/odm/EVS/CDISCExtCodeID:C103376> <http://ncicb.nci.nih.gov/xml/odm/EVS/CDISCExtCodeID:C103377> <http://ncicb.nci.nih.gov/xml/odm/EVS/CDISCExtCodeID:C147271> <http://ncicb.nci.nih.gov/xml/odm/EVS/CDISCExtCodeID:C103378> <http://ncicb.nci.nih.gov/xml/odm/EVS/CDISCExtCodeID:C103379> ) ;
    linkml:permissible_values <http://ncicb.nci.nih.gov/xml/odm/EVS/CDISCExtCodeID:C103371>,
        <http://ncicb.nci.nih.gov/xml/odm/EVS/CDISCExtCodeID:C103372>,
        <http://ncicb.nci.nih.gov/xml/odm/EVS/CDISCExtCodeID:C103373>,
        <http://ncicb.nci.nih.gov/xml/odm/EVS/CDISCExtCodeID:C103374>,
        <http://ncicb.nci.nih.gov/xml/odm/EVS/CDISCExtCodeID:C103375>,
        <http://ncicb.nci.nih.gov/xml/odm/EVS/CDISCExtCodeID:C103376>,
        <http://ncicb.nci.nih.gov/xml/odm/EVS/CDISCExtCodeID:C103377>,
        <http://ncicb.nci.nih.gov/xml/odm/EVS/CDISCExtCodeID:C103378>,
        <http://ncicb.nci.nih.gov/xml/odm/EVS/CDISCExtCodeID:C103379>,
        <http://ncicb.nci.nih.gov/xml/odm/EVS/CDISCExtCodeID:C123454>,
        <http://ncicb.nci.nih.gov/xml/odm/EVS/CDISCExtCodeID:C135396>,
        <http://ncicb.nci.nih.gov/xml/odm/EVS/CDISCExtCodeID:C147271>,
        <http://ncicb.nci.nih.gov/xml/odm/EVS/CDISCExtCodeID:C177921>,
        <http://ncicb.nci.nih.gov/xml/odm/EVS/CDISCExtCodeID:C177922>,
        <http://ncicb.nci.nih.gov/xml/odm/EVS/CDISCExtCodeID:C177923> .

odm:YesOnly a owl:Class,
        linkml:EnumDefinition ;
    rdfs:label "YesOnly" ;
    owl:unionOf [ rdf:rest () ] .

odm:DurationDatetime a owl:Class,
        linkml:TypeDefinition ;
    rdfs:label "durationDatetime" ;
    rdfs:subClassOf [ a owl:Restriction ;
            owl:onDataRange odm:durationDatetime ;
            owl:onProperty linkml:topValue ;
            owl:qualifiedCardinality 1 ] .

odm:Coding a owl:Class,
        linkml:ClassDefinition ;
    rdfs:label "Coding" ;
    rdfs:subClassOf [ a owl:Restriction ;
            owl:maxQualifiedCardinality 1 ;
            owl:onClass odm:Uriorcurie ;
            owl:onProperty odm:href ],
        [ a owl:Restriction ;
            owl:onClass odm:Uriorcurie ;
            owl:onProperty odm:System ;
            owl:qualifiedCardinality 1 ],
        [ a owl:Restriction ;
            owl:maxQualifiedCardinality 1 ;
            owl:onClass odm:Text ;
            owl:onProperty odm:CommentOID ],
        [ a owl:Restriction ;
            owl:maxQualifiedCardinality 1 ;
            owl:onClass odm:Text ;
            owl:onProperty odm:CodeRef ],
        [ a owl:Restriction ;
            owl:maxQualifiedCardinality 1 ;
            owl:onClass odm:Text ;
            owl:onProperty odm:Label ],
        [ a owl:Restriction ;
            owl:maxQualifiedCardinality 1 ;
            owl:onClass odm:Uriorcurie ;
            owl:onProperty odm:ref ],
        [ a owl:Restriction ;
            owl:maxQualifiedCardinality 1 ;
            owl:onClass odm:Text ;
            owl:onProperty odm:SystemVersion ],
        [ a owl:Restriction ;
            owl:maxQualifiedCardinality 1 ;
            owl:onClass odm:Text ;
            owl:onProperty odm:SystemName ] ;
    skos:definition "Coding references a symbol from a defined code system. It uses a code defined in a terminology system to associate semantics with a given term, codelist, variable, or group of variables. The presence of a Coding element associates a meaning to its parent element. Including multiple Coding elements for a given parent indicates synonymous meanings provided by different code systems or code system versions." ;
    skos:exactMatch odm:Coding .

odm:range a owl:ObjectProperty,
        linkml:SlotDefinition ;
    rdfs:label "range" ;
    rdfs:range odm:String .

odm:ContentType a owl:Class,
        linkml:TypeDefinition ;
    rdfs:label "_contentType" ;
    rdfs:subClassOf [ a owl:Restriction ;
            owl:onDataRange xhtml:div ;
            owl:onProperty linkml:topValue ;
            owl:qualifiedCardinality 1 ] .

odm:_content a owl:ObjectProperty,
        linkml:SlotDefinition ;
    rdfs:label "_content" ;
    rdfs:range odm:ContentType ;
    skos:definition "multi-line text content from between XML tags" .

odm:DataType a owl:Class,
        linkml:EnumDefinition ;
    rdfs:label "DataType" ;
    owl:unionOf ( <http://www.cdisc.org/ns/odm/v2.0/DataType#integer> <http://www.cdisc.org/ns/odm/v2.0/DataType#decimal> <http://www.cdisc.org/ns/odm/v2.0/DataType#float> <http://www.cdisc.org/ns/odm/v2.0/DataType#double> <http://www.cdisc.org/ns/odm/v2.0/DataType#date> <http://www.cdisc.org/ns/odm/v2.0/DataType#datetime> <http://www.cdisc.org/ns/odm/v2.0/DataType#time> <http://www.cdisc.org/ns/odm/v2.0/DataType#text> <http://www.cdisc.org/ns/odm/v2.0/DataType#string> <http://www.cdisc.org/ns/odm/v2.0/DataType#URI> <http://www.cdisc.org/ns/odm/v2.0/DataType#boolean> <http://www.cdisc.org/ns/odm/v2.0/DataType#hexBinary> <http://www.cdisc.org/ns/odm/v2.0/DataType#base64Binary> <http://www.cdisc.org/ns/odm/v2.0/DataType#hexFloat> <http://www.cdisc.org/ns/odm/v2.0/DataType#base64Float> <http://www.cdisc.org/ns/odm/v2.0/DataType#partialDate> <http://www.cdisc.org/ns/odm/v2.0/DataType#partialTime> <http://www.cdisc.org/ns/odm/v2.0/DataType#partialDatetime> <http://www.cdisc.org/ns/odm/v2.0/DataType#durationDatetime> <http://www.cdisc.org/ns/odm/v2.0/DataType#intervalDatetime> <http://www.cdisc.org/ns/odm/v2.0/DataType#incompleteDatetime> <http://www.cdisc.org/ns/odm/v2.0/DataType#incompleteDate> <http://www.cdisc.org/ns/odm/v2.0/DataType#incompleteTime> ) ;
    linkml:permissible_values <http://www.cdisc.org/ns/odm/v2.0/DataType#URI>,
        <http://www.cdisc.org/ns/odm/v2.0/DataType#base64Binary>,
        <http://www.cdisc.org/ns/odm/v2.0/DataType#base64Float>,
        <http://www.cdisc.org/ns/odm/v2.0/DataType#boolean>,
        <http://www.cdisc.org/ns/odm/v2.0/DataType#date>,
        <http://www.cdisc.org/ns/odm/v2.0/DataType#datetime>,
        <http://www.cdisc.org/ns/odm/v2.0/DataType#decimal>,
        <http://www.cdisc.org/ns/odm/v2.0/DataType#double>,
        <http://www.cdisc.org/ns/odm/v2.0/DataType#durationDatetime>,
        <http://www.cdisc.org/ns/odm/v2.0/DataType#float>,
        <http://www.cdisc.org/ns/odm/v2.0/DataType#hexBinary>,
        <http://www.cdisc.org/ns/odm/v2.0/DataType#hexFloat>,
        <http://www.cdisc.org/ns/odm/v2.0/DataType#incompleteDate>,
        <http://www.cdisc.org/ns/odm/v2.0/DataType#incompleteDatetime>,
        <http://www.cdisc.org/ns/odm/v2.0/DataType#incompleteTime>,
        <http://www.cdisc.org/ns/odm/v2.0/DataType#integer>,
        <http://www.cdisc.org/ns/odm/v2.0/DataType#intervalDatetime>,
        <http://www.cdisc.org/ns/odm/v2.0/DataType#partialDate>,
        <http://www.cdisc.org/ns/odm/v2.0/DataType#partialDatetime>,
        <http://www.cdisc.org/ns/odm/v2.0/DataType#partialTime>,
        <http://www.cdisc.org/ns/odm/v2.0/DataType#string>,
        <http://www.cdisc.org/ns/odm/v2.0/DataType#text>,
        <http://www.cdisc.org/ns/odm/v2.0/DataType#time> .

odm:PositiveInteger a owl:Class,
        linkml:TypeDefinition ;
    rdfs:label "positiveInteger" ;
    rdfs:subClassOf [ a owl:Restriction ;
            owl:onDataRange odm:positiveInteger ;
            owl:onProperty linkml:topValue ;
            owl:qualifiedCardinality 1 ] .

odm:String a owl:Class,
        linkml:TypeDefinition ;
    rdfs:label "string" ;
    rdfs:subClassOf [ a owl:Restriction ;
            owl:onDataRange xsd:string ;
            owl:onProperty linkml:topValue ;
            owl:qualifiedCardinality 1 ] .

odm:DescriptionRef a owl:ObjectProperty,
        linkml:SlotDefinition ;
    rdfs:label "DescriptionRef" ;
    rdfs:range odm:Description ;
    skos:definition "Description reference: A free-text description of the containing metadata component, unless restricted by Business Rules." .

odm:OID a owl:ObjectProperty,
        linkml:SlotDefinition ;
    rdfs:label "OID" ;
    rdfs:range odm:Oid ;
    skos:definition "Unique identifier of the version within the XML document." .

odm:Description a owl:Class,
        linkml:ClassDefinition ;
    rdfs:label "Description" ;
    rdfs:subClassOf [ a owl:Restriction ;
            owl:allValuesFrom odm:TranslatedText ;
            owl:onProperty odm:TranslatedTextRef ] ;
    skos:definition "A free-text description of the containing metadata component, unless restricted by Business Rules." ;
    skos:exactMatch odm:Description .

odm:Oid a owl:Class,
        linkml:TypeDefinition ;
    rdfs:label "oid" ;
    rdfs:subClassOf [ a owl:Restriction ;
            owl:onDataRange odm:oid ;
            owl:onProperty linkml:topValue ;
            owl:qualifiedCardinality 1 ] .

linkml:TypeDefinition a owl:Class .

linkml:topValue a owl:DatatypeProperty ;
    rdfs:label "value" .

odm:Text a owl:Class,
        linkml:TypeDefinition ;
    rdfs:label "text" ;
    rdfs:subClassOf [ a owl:Restriction ;
            owl:onDataRange odm:text ;
            owl:onProperty linkml:topValue ;
            owl:qualifiedCardinality 1 ] .

odm:Name a owl:Class,
        owl:ObjectProperty,
        linkml:SlotDefinition,
        linkml:TypeDefinition ;
    rdfs:label "Name",
        "name" ;
    rdfs:range odm:String ;
    rdfs:subClassOf [ a owl:Restriction ;
            owl:onDataRange odm:name ;
            owl:onProperty linkml:topValue ;
            owl:qualifiedCardinality 1 ] ;
    skos:definition "General observation Sub Class." .

odm:Oidref a owl:Class,
        linkml:TypeDefinition ;
    rdfs:label "oidref" ;
    rdfs:subClassOf [ a owl:Restriction ;
            owl:onDataRange odm:oidref ;
            owl:onProperty linkml:topValue ;
            owl:qualifiedCardinality 1 ] .

linkml:ClassDefinition a owl:Class .

linkml:SlotDefinition a owl:Class .


